@prefix fhir:  <http://hl7.org/fhir/> .
@prefix rdf:   <http://www.w3.org/1999/02/22-rdf-syntax-ns#> .
@prefix owl:   <http://www.w3.org/2002/07/owl#> .
@prefix v3-substanceAdminSubstitution: <http://hl7.org/fhir/v3/substanceAdminSubstitution/> .
@prefix xsd:   <http://www.w3.org/2001/XMLSchema#> .
@prefix rdfs:  <http://www.w3.org/2000/01/rdf-schema#> .
@prefix w5:    <http://hl7.org/fhir/w5#> .

v3-substanceAdminSubstitution:BC
        a                owl:Class ;
        rdfs:label       "brand composition" ;
        rdfs:subClassOf  v3-substanceAdminSubstitution:EC ;
        <http://www.w3.org/2004/02/skos/core#definition>
                "Description: \n                        \r\n\n                        Substitution occurred or is permitted between equivalent Brands but not Generics\r\n\n                        \n                           Examples: \n                        \r\n\n                        \n                           Zestril  for Prinivil\n                           Coumadin for Jantoven" ;
        <http://www.w3.org/2004/02/skos/core#prefLabel>
                "brand composition" .

v3-substanceAdminSubstitution:TE
        a                owl:Class ;
        rdfs:label       "therapeutic alternative" ;
        rdfs:subClassOf  v3-substanceAdminSubstitution:E ;
        <http://www.w3.org/2004/02/skos/core#definition>
                "Description: Substitution occurred or is permitted with another product having the same therapeutic objective and safety profile.\r\n\n                        \n                           Examples: \n                        \r\n\n                        \n                           ranitidine for Tagamet" ;
        <http://www.w3.org/2004/02/skos/core#prefLabel>
                "therapeutic alternative" .

v3-substanceAdminSubstitution:
        a                owl:Ontology ;
        rdfs:comment     " Identifies what sort of change is permitted or has occurred between the therapy that was ordered and the therapy that was/will be provided." ;
        rdfs:label       "v3 Code System substanceAdminSubstitution" ;
        owl:versionIRI   "http://hl7.org/fhir/v3/substanceAdminSubstitution/2016-11-11" ;
        owl:versionInfo  "v3 Code System substanceAdminSubstitution(2016-11-11)" .

v3-substanceAdminSubstitution:F
        a                owl:Class ;
        rdfs:label       "formulary" ;
        rdfs:subClassOf  v3-substanceAdminSubstitution:_ActSubstanceAdminSubstitutionCode ;
        <http://www.w3.org/2004/02/skos/core#definition>
                "Description: This substitution was performed or is permitted based on formulary guidelines." ;
        <http://www.w3.org/2004/02/skos/core#prefLabel>
                "formulary" .

v3-substanceAdminSubstitution:N
        a                owl:Class ;
        rdfs:label       "none" ;
        rdfs:subClassOf  v3-substanceAdminSubstitution:_ActSubstanceAdminSubstitutionCode ;
        <http://www.w3.org/2004/02/skos/core#definition>
                "No substitution occurred or is permitted." ;
        <http://www.w3.org/2004/02/skos/core#prefLabel>
                "none" .

v3-substanceAdminSubstitution:_ActSubstanceAdminSubstitutionCode
        a           owl:Class ;
        rdfs:label  "ActSubstanceAdminSubstitutionCode" ;
        <http://www.w3.org/2004/02/skos/core#definition>
                "Description: Substitution occurred or is permitted with another product that may potentially have different ingredients, but having the same biological and therapeutic effects." ;
        <http://www.w3.org/2004/02/skos/core#prefLabel>
                "ActSubstanceAdminSubstitutionCode" .

v3-substanceAdminSubstitution:G
        a                owl:Class ;
        rdfs:label       "generic composition" ;
        rdfs:subClassOf  v3-substanceAdminSubstitution:EC ;
        <http://www.w3.org/2004/02/skos/core#definition>
                "Description: Substitution occurred or is permitted between equivalent Generics but not Brands\r\n\n                        \n                           Examples: \n                        \r\n\n                        \n                           Lisnopril (Lupin Corp) for Lisnopril (Wockhardt Corp)" ;
        <http://www.w3.org/2004/02/skos/core#prefLabel>
                "generic composition" .

v3-substanceAdminSubstitution:EC
        a                owl:Class ;
        rdfs:label       "equivalent composition" ;
        rdfs:subClassOf  v3-substanceAdminSubstitution:E ;
        <http://www.w3.org/2004/02/skos/core#definition>
                "Description: \n                        \r\n\n                        Substitution occurred or is permitted with another product that is a:\r\n\n                        \n                           pharmaceutical alternative containing the same active ingredient but is formulated with different salt, ester\n                           pharmaceutical equivalent that has the same active ingredient, strength, dosage form and route of administration\n                        \n                        \n                           Examples: \n                        \r\n\n                        \n                           \n                              Pharmaceutical alternative: Erythromycin Ethylsuccinate for Erythromycin Stearate\n                           \n                              Pharmaceutical equivalent: Lisonpril for Zestril" ;
        <http://www.w3.org/2004/02/skos/core#prefLabel>
                "equivalent composition" .

v3-substanceAdminSubstitution:E
        a                owl:Class ;
        rdfs:label       "equivalent" ;
        rdfs:subClassOf  v3-substanceAdminSubstitution:_ActSubstanceAdminSubstitutionCode ;
        <http://www.w3.org/2004/02/skos/core#definition>
                "Description: Substitution occurred or is permitted with another bioequivalent and therapeutically equivalent product." ;
        <http://www.w3.org/2004/02/skos/core#prefLabel>
                "equivalent" .

v3-substanceAdminSubstitution:TB
        a                owl:Class ;
        rdfs:label       "therapeutic brand" ;
        rdfs:subClassOf  v3-substanceAdminSubstitution:TE ;
        <http://www.w3.org/2004/02/skos/core#definition>
                "Description: Substitution occurred or is permitted between therapeutically equivalent Brands but not Generics\r\n>\n                           Examples: \n                        \r\n\n                        \n                           Zantac for Tagamet" ;
        <http://www.w3.org/2004/02/skos/core#prefLabel>
                "therapeutic brand" .

v3-substanceAdminSubstitution:TG
        a                owl:Class ;
        rdfs:label       "therapeutic generic" ;
        rdfs:subClassOf  v3-substanceAdminSubstitution:TE ;
        <http://www.w3.org/2004/02/skos/core#definition>
                "Description: Substitution occurred or is permitted between therapeutically equivalent Generics but not Brands\r\n>\n                           Examples: \n                        \r\n\n                        \n                           Ranitidine  for cimetidine" ;
        <http://www.w3.org/2004/02/skos/core#prefLabel>
                "therapeutic generic" .
