@prefix fhir:  <http://hl7.org/fhir/> .
@prefix rdf:   <http://www.w3.org/1999/02/22-rdf-syntax-ns#> .
@prefix owl:   <http://www.w3.org/2002/07/owl#> .
@prefix xsd:   <http://www.w3.org/2001/XMLSchema#> .
@prefix rdfs:  <http://www.w3.org/2000/01/rdf-schema#> .
@prefix v3-RoleStatus: <http://hl7.org/fhir/v3/RoleStatus/> .
@prefix w5:    <http://hl7.org/fhir/w5#> .

v3-RoleStatus:normal  a  owl:Class ;
        rdfs:label  "normal" ;
        <http://www.w3.org/2004/02/skos/core#definition>
                "The 'typical' state. Excludes \"nullified\" which represents the termination state of a Role instance that was created in error." ;
        <http://www.w3.org/2004/02/skos/core#prefLabel>
                "normal" .

v3-RoleStatus:suspended
        a                owl:Class ;
        rdfs:label       "suspended" ;
        rdfs:subClassOf  v3-RoleStatus:normal ;
        <http://www.w3.org/2004/02/skos/core#definition>
                "The state that represents a suspension of the Entity playing the Role. This state is arrived at from the \"active\" state." ;
        <http://www.w3.org/2004/02/skos/core#prefLabel>
                "suspended" .

v3-RoleStatus:nullified
        a           owl:Class ;
        rdfs:label  "nullified" ;
        <http://www.w3.org/2004/02/skos/core#definition>
                "The state representing the termination of a Role instance that was created in error." ;
        <http://www.w3.org/2004/02/skos/core#prefLabel>
                "nullified" .

v3-RoleStatus:active  a  owl:Class ;
        rdfs:label       "active" ;
        rdfs:subClassOf  v3-RoleStatus:normal ;
        <http://www.w3.org/2004/02/skos/core#definition>
                "The state representing the fact that the Entity is currently active in the Role." ;
        <http://www.w3.org/2004/02/skos/core#prefLabel>
                "active" .

v3-RoleStatus:cancelled
        a                owl:Class ;
        rdfs:label       "cancelled" ;
        rdfs:subClassOf  v3-RoleStatus:normal ;
        <http://www.w3.org/2004/02/skos/core#definition>
                "The terminal state resulting from cancellation of the role prior to activation." ;
        <http://www.w3.org/2004/02/skos/core#prefLabel>
                "cancelled" .

v3-RoleStatus:terminated
        a                owl:Class ;
        rdfs:label       "terminated" ;
        rdfs:subClassOf  v3-RoleStatus:normal ;
        <http://www.w3.org/2004/02/skos/core#definition>
                "The state representing the successful termination of the Role." ;
        <http://www.w3.org/2004/02/skos/core#prefLabel>
                "terminated" .

v3-RoleStatus:  a        owl:Ontology ;
        rdfs:comment     " Codes representing the defined possible states of an Role, as defined by the Role class state machine." ;
        rdfs:label       "v3 Code System RoleStatus" ;
        owl:versionIRI   "http://hl7.org/fhir/v3/RoleStatus/2016-11-11" ;
        owl:versionInfo  "v3 Code System RoleStatus(2016-11-11)" .

v3-RoleStatus:pending
        a                owl:Class ;
        rdfs:label       "pending" ;
        rdfs:subClassOf  v3-RoleStatus:normal ;
        <http://www.w3.org/2004/02/skos/core#definition>
                "The state representing that fact that the role has not yet become active." ;
        <http://www.w3.org/2004/02/skos/core#prefLabel>
                "pending" .
