@prefix v3-ActStatus: <http://hl7.org/fhir/v3/ActStatus/> .
@prefix fhir:  <http://hl7.org/fhir/> .
@prefix rdf:   <http://www.w3.org/1999/02/22-rdf-syntax-ns#> .
@prefix owl:   <http://www.w3.org/2002/07/owl#> .
@prefix xsd:   <http://www.w3.org/2001/XMLSchema#> .
@prefix rdfs:  <http://www.w3.org/2000/01/rdf-schema#> .
@prefix w5:    <http://hl7.org/fhir/w5#> .

v3-ActStatus:held  a     owl:Class ;
        rdfs:label       "held" ;
        rdfs:subClassOf  v3-ActStatus:normal ;
        <http://www.w3.org/2004/02/skos/core#definition>
                "An Act that is still in the preparatory stages has been put aside.  No action can occur until the Act is released." ;
        <http://www.w3.org/2004/02/skos/core#prefLabel>
                "held" .

v3-ActStatus:aborted  a  owl:Class ;
        rdfs:label       "aborted" ;
        rdfs:subClassOf  v3-ActStatus:normal ;
        <http://www.w3.org/2004/02/skos/core#definition>
                "The Act has been terminated prior to the originally intended completion." ;
        <http://www.w3.org/2004/02/skos/core#prefLabel>
                "aborted" .

v3-ActStatus:active  a   owl:Class ;
        rdfs:label       "active" ;
        rdfs:subClassOf  v3-ActStatus:normal ;
        <http://www.w3.org/2004/02/skos/core#definition>
                "The Act can be performed or is being performed" ;
        <http://www.w3.org/2004/02/skos/core#prefLabel>
                "active" .

v3-ActStatus:suspended
        a                owl:Class ;
        rdfs:label       "suspended" ;
        rdfs:subClassOf  v3-ActStatus:normal ;
        <http://www.w3.org/2004/02/skos/core#definition>
                "An Act that has been activated (actions could or have been performed against it), but has been temporarily disabled.  No further action should be taken against it until it is released" ;
        <http://www.w3.org/2004/02/skos/core#prefLabel>
                "suspended" .

v3-ActStatus:obsolete
        a           owl:Class ;
        rdfs:label  "obsolete" ;
        <http://www.w3.org/2004/02/skos/core#definition>
                "This Act instance has been replaced by a new instance." ;
        <http://www.w3.org/2004/02/skos/core#prefLabel>
                "obsolete" .

v3-ActStatus:nullified
        a           owl:Class ;
        rdfs:label  "nullified" ;
        <http://www.w3.org/2004/02/skos/core#definition>
                "This Act instance was created in error and has been 'removed' and is treated as though it never existed.  A record is retained for audit purposes only." ;
        <http://www.w3.org/2004/02/skos/core#prefLabel>
                "nullified" .

v3-ActStatus:normal  a  owl:Class ;
        rdfs:label  "normal" ;
        <http://www.w3.org/2004/02/skos/core#definition>
                "Encompasses the expected states of an Act, but excludes \"nullified\" and \"obsolete\" which represent unusual terminal states for the life-cycle." ;
        <http://www.w3.org/2004/02/skos/core#prefLabel>
                "normal" .

v3-ActStatus:completed
        a                owl:Class ;
        rdfs:label       "completed" ;
        rdfs:subClassOf  v3-ActStatus:normal ;
        <http://www.w3.org/2004/02/skos/core#definition>
                "An Act that has terminated normally after all of its constituents have been performed." ;
        <http://www.w3.org/2004/02/skos/core#prefLabel>
                "completed" .

v3-ActStatus:cancelled
        a                owl:Class ;
        rdfs:label       "cancelled" ;
        rdfs:subClassOf  v3-ActStatus:normal ;
        <http://www.w3.org/2004/02/skos/core#definition>
                "The Act has been abandoned before activation." ;
        <http://www.w3.org/2004/02/skos/core#prefLabel>
                "cancelled" .

v3-ActStatus:  a         owl:Ontology ;
        rdfs:comment     " Codes representing the defined possible states of an Act, as defined by the Act class state machine." ;
        rdfs:label       "v3 Code System ActStatus" ;
        owl:versionIRI   "http://hl7.org/fhir/v3/ActStatus/2016-11-11" ;
        owl:versionInfo  "v3 Code System ActStatus(2016-11-11)" .

v3-ActStatus:new  a      owl:Class ;
        rdfs:label       "new" ;
        rdfs:subClassOf  v3-ActStatus:normal ;
        <http://www.w3.org/2004/02/skos/core#definition>
                "An Act that is in the preparatory stages and may not yet be acted upon" ;
        <http://www.w3.org/2004/02/skos/core#prefLabel>
                "new" .
