@prefix v3-RoleCode: <http://hl7.org/fhir/v3/RoleCode/> .
@prefix fhir:  <http://hl7.org/fhir/> .
@prefix rdf:   <http://www.w3.org/1999/02/22-rdf-syntax-ns#> .
@prefix owl:   <http://www.w3.org/2002/07/owl#> .
@prefix xsd:   <http://www.w3.org/2001/XMLSchema#> .
@prefix rdfs:  <http://www.w3.org/2000/01/rdf-schema#> .
@prefix w5:    <http://hl7.org/fhir/w5#> .

v3-RoleCode:HSIS  a      owl:Class ;
        rdfs:label       "half-sister" ;
        rdfs:subClassOf  v3-RoleCode:HSIB ;
        <http://www.w3.org/2004/02/skos/core#definition>
                "The player of the role is a female related to the scoping entity by sharing only one biological parent." ;
        <http://www.w3.org/2004/02/skos/core#prefLabel>
                "half-sister" .

v3-RoleCode:ENDOS  a     owl:Class ;
        rdfs:label       "Endoscopy lab" ;
        rdfs:subClassOf  v3-RoleCode:GIDX ;
        <http://www.w3.org/2004/02/skos/core#definition>
                "(X12N 261QD0000N)" ;
        <http://www.w3.org/2004/02/skos/core#prefLabel>
                "Endoscopy lab" .

v3-RoleCode:INDIG  a     owl:Class ;
        rdfs:label       "member of an indigenous people" ;
        rdfs:subClassOf  v3-RoleCode:_ProgramEligiblePartyRoleType ;
        <http://www.w3.org/2004/02/skos/core#definition>
                "Description: A person playing the role of program eligible under a program based on aboriginal ancestry or as a member of an aboriginal community.\r\n\n                        \n                           Discussion: This CoveredPartyRoleType.code is typically used when the CoveredPartyRole class code is \"program eligible\" and the person's status as a member of an indigenous people meets jurisdictional or program criteria." ;
        <http://www.w3.org/2004/02/skos/core#prefLabel>
                "member of an indigenous people" .

v3-RoleCode:OUTLAB  a    owl:Class ;
        rdfs:label       "outpatient laboratory" ;
        rdfs:subClassOf  v3-RoleCode:HLAB ;
        <http://www.w3.org/2004/02/skos/core#definition>
                "Description: A location that plays the role of delivering services which may include tests are done on clinical specimens to get health information about a patient pertaining to the diagnosis, treatment, and prevention of disease for same day visits." ;
        <http://www.w3.org/2004/02/skos/core#prefLabel>
                "outpatient laboratory" .

v3-RoleCode:NS  a        owl:Class ;
        rdfs:label       "Neurosurgery unit" ;
        rdfs:subClassOf  v3-RoleCode:HU ;
        <http://www.w3.org/2004/02/skos/core#definition>
                "Neurosurgery unit" ;
        <http://www.w3.org/2004/02/skos/core#prefLabel>
                "Neurosurgery unit" .

v3-RoleCode:RNEU  a      owl:Class ;
        rdfs:label       "Neuroradiology unit" ;
        rdfs:subClassOf  v3-RoleCode:RADDX ;
        <http://www.w3.org/2004/02/skos/core#definition>
                "Neuroradiology unit" ;
        <http://www.w3.org/2004/02/skos/core#prefLabel>
                "Neuroradiology unit" .

v3-RoleCode:GIDX  a      owl:Class ;
        rdfs:label       "Gastroenterology diagnostics or therapeutics lab" ;
        rdfs:subClassOf  v3-RoleCode:DX ;
        <http://www.w3.org/2004/02/skos/core#definition>
                "A practice setting where GI procedures (such as endoscopies) are performed" ;
        <http://www.w3.org/2004/02/skos/core#prefLabel>
                "Gastroenterology diagnostics or therapeutics lab" .

v3-RoleCode:RHII  a      owl:Class ;
        rdfs:label       "intellectual impairment center" ;
        rdfs:subClassOf  v3-RoleCode:RH ;
        <http://www.w3.org/2004/02/skos/core#definition>
                "Description: A location that plays the role of delivering services which may include adaptation, rehabilitation and social integration services for people with intellectual and/or pervasive development disorders such as autism or severe behaviour disorder." ;
        <http://www.w3.org/2004/02/skos/core#prefLabel>
                "intellectual impairment center" .

v3-RoleCode:GPARNT  a    owl:Class ;
        rdfs:label       "grandparent" ;
        rdfs:subClassOf  v3-RoleCode:_CoverageRoleType ;
        <http://www.w3.org/2004/02/skos/core#definition>
                "parent of a parent of the subject." ;
        <http://www.w3.org/2004/02/skos/core#prefLabel>
                "grandparent" .

v3-RoleCode:CAPC  a      owl:Class ;
        rdfs:label       "Child and adolescent psychiatry clinic" ;
        rdfs:subClassOf  v3-RoleCode:OF ;
        <http://www.w3.org/2004/02/skos/core#definition>
                "Child and adolescent psychiatry clinic" ;
        <http://www.w3.org/2004/02/skos/core#prefLabel>
                "Child and adolescent psychiatry clinic" .

v3-RoleCode:COCBEN  a    owl:Class ;
        rdfs:label       "continuity of coverage beneficiary" ;
        rdfs:subClassOf  v3-RoleCode:_DependentCoveredPartyRoleType ;
        <http://www.w3.org/2004/02/skos/core#definition>
                "Description: A person playing the role of an individual insured with continuity of coverage under a policy which is being terminated based on loss of original status that was the basis for coverage.  Criteria for qualifying for continuity of coverage may be set by law.\r\n\n                        \n                           Discussion: This CoveredPartyRoleType.code is typically used when the CoveredPartyRole class code is either \"program eligible\" or \"subscriber\" and the person's status as a continuity of coverage beneficiary meets jurisdictional or policy criteria." ;
        <http://www.w3.org/2004/02/skos/core#prefLabel>
                "continuity of coverage beneficiary" .

v3-RoleCode:DAUADOPT  a  owl:Class ;
        rdfs:label       "adopted daughter" ;
        rdfs:subClassOf  v3-RoleCode:CHLDADOPT ;
        <http://www.w3.org/2004/02/skos/core#definition>
                "The player of the role is a female child taken into a family through legal means and raised by the scoping person (parent) as his or her own child." ;
        <http://www.w3.org/2004/02/skos/core#prefLabel>
                "adopted daughter" .

v3-RoleCode:laboratory
        a           owl:Class ;
        rdfs:label  "Laboratory" ;
        <http://www.w3.org/2004/02/skos/core#definition>
                "Laboratory" ;
        <http://www.w3.org/2004/02/skos/core#prefLabel>
                "Laboratory" .

v3-RoleCode:_CoverageRoleType
        a                owl:Class ;
        rdfs:label       "CoverageRoleType" ;
        rdfs:subClassOf  v3-RoleCode:_PolicyOrProgramCoverageRoleType ;
        <http://www.w3.org/2004/02/skos/core#definition>
                "Role recognized through the issuance of insurance coverage to an identified covered party who has this relationship with the policy holder such as the policy holder themselves (self), spouse, child, etc" ;
        <http://www.w3.org/2004/02/skos/core#prefLabel>
                "CoverageRoleType" .

v3-RoleCode:VL  a        owl:Class ;
        rdfs:label       "Veal" ;
        rdfs:subClassOf  v3-RoleCode:_LivingSubjectProductionClass ;
        <http://www.w3.org/2004/02/skos/core#definition>
                "Cattle raised for veal meat production.  Implicit is the husbandry method." ;
        <http://www.w3.org/2004/02/skos/core#prefLabel>
                "Veal" .

v3-RoleCode:BMTU  a      owl:Class ;
        rdfs:label       "Bone marrow transplant unit" ;
        rdfs:subClassOf  v3-RoleCode:HU ;
        <http://www.w3.org/2004/02/skos/core#definition>
                "Bone marrow transplant unit" ;
        <http://www.w3.org/2004/02/skos/core#prefLabel>
                "Bone marrow transplant unit" .

v3-RoleCode:PL  a        owl:Class ;
        rdfs:label       "Pleasure" ;
        rdfs:subClassOf  v3-RoleCode:_LivingSubjectProductionClass ;
        <http://www.w3.org/2004/02/skos/core#definition>
                "Animals rasied for recreation" ;
        <http://www.w3.org/2004/02/skos/core#prefLabel>
                "Pleasure" .

v3-RoleCode:SUBSCR  a  owl:Class ;
        rdfs:label  "subscriber" ;
        <http://www.w3.org/2004/02/skos/core#definition>
                "A party covered under a policy based on association with a sponsor who is the policy holder, and whose association may provide for the eligibility of dependents for coverage" ;
        <http://www.w3.org/2004/02/skos/core#prefLabel>
                "subscriber" .

v3-RoleCode:ETU  a       owl:Class ;
        rdfs:label       "Emergency trauma unit" ;
        rdfs:subClassOf  v3-RoleCode:ER ;
        <http://www.w3.org/2004/02/skos/core#definition>
                "Emergency trauma unit" ;
        <http://www.w3.org/2004/02/skos/core#prefLabel>
                "Emergency trauma unit" .

v3-RoleCode:PSYCHCF  a  owl:Class ;
        rdfs:label  "PSYCHCF" ;
        <http://www.w3.org/2004/02/skos/core#prefLabel>
                "PSYCHCF" .

v3-RoleCode:AMPUT  a     owl:Class ;
        rdfs:label       "Amputee clinic" ;
        rdfs:subClassOf  v3-RoleCode:OF ;
        <http://www.w3.org/2004/02/skos/core#definition>
                "Amputee clinic" ;
        <http://www.w3.org/2004/02/skos/core#prefLabel>
                "Amputee clinic" .

v3-RoleCode:STPSIS  a    owl:Class ;
        rdfs:label       "stepsister" ;
        rdfs:subClassOf  v3-RoleCode:SIS ;
        <http://www.w3.org/2004/02/skos/core#definition>
                "The player of the role is a daughter of the scoping person's stepparent." ;
        <http://www.w3.org/2004/02/skos/core#prefLabel>
                "stepsister" .

v3-RoleCode:MBL  a       owl:Class ;
        rdfs:label       "medical laboratory" ;
        rdfs:subClassOf  v3-RoleCode:HU ;
        <http://www.w3.org/2004/02/skos/core#definition>
                "Description: A location that plays the role of delivering services which include biochemistry, hematology, microbiology, immunochemistry, and toxicology." ;
        <http://www.w3.org/2004/02/skos/core#prefLabel>
                "medical laboratory" .

v3-RoleCode:_ResearchSubjectRoleBasis
        a           owl:Class ;
        rdfs:label  "ResearchSubjectRoleBasis" ;
        <http://www.w3.org/2004/02/skos/core#definition>
                "Specifies the administrative functionality within a formal experimental design for which the ResearchSubject role was established.  Examples: screening - role is used for pre-enrollment evaluation portion of the design; enrolled - role is used for subjects admitted to the active treatment portion of the design." ;
        <http://www.w3.org/2004/02/skos/core#prefLabel>
                "ResearchSubjectRoleBasis" .

v3-RoleCode:_AgentRoleType
        a                owl:Class ;
        rdfs:label       "AgentRoleType" ;
        rdfs:subClassOf  v3-RoleCode:_AffiliationRoleType ;
        <http://www.w3.org/2004/02/skos/core#definition>
                "Parties that may or should contribute or have contributed to an Act." ;
        <http://www.w3.org/2004/02/skos/core#prefLabel>
                "AgentRoleType" .

v3-RoleCode:ICU  a       owl:Class ;
        rdfs:label       "Intensive care unit" ;
        rdfs:subClassOf  v3-RoleCode:HU ;
        <http://www.w3.org/2004/02/skos/core#definition>
                "Intensive care unit" ;
        <http://www.w3.org/2004/02/skos/core#prefLabel>
                "Intensive care unit" .

v3-RoleCode:PAUNT  a     owl:Class ;
        rdfs:label       "paternal aunt" ;
        rdfs:subClassOf  v3-RoleCode:AUNT ;
        <http://www.w3.org/2004/02/skos/core#definition>
                "Description:The player of the role is a biological sister of the scoping person's biological father." ;
        <http://www.w3.org/2004/02/skos/core#prefLabel>
                "paternal aunt" .

v3-RoleCode:JURID  a     owl:Class ;
        rdfs:label       "jurisdiction location identifier" ;
        rdfs:subClassOf  v3-RoleCode:_LocationIdentifiedEntityRoleCode ;
        <http://www.w3.org/2004/02/skos/core#definition>
                "Description:Identifier assigned to a location by a jurisdiction." ;
        <http://www.w3.org/2004/02/skos/core#prefLabel>
                "jurisdiction location identifier" .

v3-RoleCode:DA  a        owl:Class ;
        rdfs:label       "Dairy" ;
        rdfs:subClassOf  v3-RoleCode:_LivingSubjectProductionClass ;
        <http://www.w3.org/2004/02/skos/core#definition>
                "Milk production" ;
        <http://www.w3.org/2004/02/skos/core#prefLabel>
                "Dairy" .

v3-RoleCode:SONC  a      owl:Class ;
        rdfs:label       "son" ;
        rdfs:subClassOf  v3-RoleCode:CHILD ;
        <http://www.w3.org/2004/02/skos/core#definition>
                "Description: The player of the role is a male child (of any type) of scoping entity (parent)" ;
        <http://www.w3.org/2004/02/skos/core#prefLabel>
                "son" .

v3-RoleCode:SPS  a       owl:Class ;
        rdfs:label       "spouse" ;
        rdfs:subClassOf  v3-RoleCode:SIGOTHR ;
        <http://www.w3.org/2004/02/skos/core#definition>
                "The player of the role is a marriage partner of the scoping person." ;
        <http://www.w3.org/2004/02/skos/core#prefLabel>
                "spouse" .

v3-RoleCode:NOK  a       owl:Class ;
        rdfs:label       "next of kin" ;
        rdfs:subClassOf  v3-RoleCode:_ContactRoleType ;
        <http://www.w3.org/2004/02/skos/core#definition>
                "Played by an individual who is designated as the next of kin for another individual which scopes the role." ;
        <http://www.w3.org/2004/02/skos/core#prefLabel>
                "next of kin" .

v3-RoleCode:ERL  a       owl:Class ;
        rdfs:label       "enrollment" ;
        rdfs:subClassOf  v3-RoleCode:_ResearchSubjectRoleBasis ;
        <http://www.w3.org/2004/02/skos/core#definition>
                "Definition:The specific role being played by a research subject participating in the active treatment or primary data collection portion of a research study." ;
        <http://www.w3.org/2004/02/skos/core#prefLabel>
                "enrollment" .

v3-RoleCode:DPOWATT  a   owl:Class ;
        rdfs:label       "durable power of attorney" ;
        rdfs:subClassOf  v3-RoleCode:POWATT ;
        <http://www.w3.org/2004/02/skos/core#definition>
                "A relationship between two people in which one person authorizes another, usually a family member or relative, to act for him or her in a manner which is a legally binding upon the person giving such authority as if he or she personally were to do the acts that is often limited in the kinds of powers that can be assigned.  Unlike ordinary powers of attorney, durable powers can survive for long periods of time, and again, unlike standard powers of attorney, durable powers can continue after incompetency." ;
        <http://www.w3.org/2004/02/skos/core#prefLabel>
                "durable power of attorney" .

v3-RoleCode:ITWIN  a     owl:Class ;
        rdfs:label       "identical twin" ;
        rdfs:subClassOf  v3-RoleCode:TWIN ;
        <http://www.w3.org/2004/02/skos/core#definition>
                "The scoper and player are offspring of the same egg-sperm pair." ;
        <http://www.w3.org/2004/02/skos/core#prefLabel>
                "identical twin" .

v3-RoleCode:FTWINBRO  a  owl:Class ;
        rdfs:label       "fraternal twin brother" ;
        rdfs:subClassOf  v3-RoleCode:TWINBRO ;
        <http://www.w3.org/2004/02/skos/core#definition>
                "The scoper was carried in the same womb as the male player and shares common biological parents but is the product of a distinct egg/sperm pair." ;
        <http://www.w3.org/2004/02/skos/core#prefLabel>
                "fraternal twin brother" .

v3-RoleCode:GGRFTH  a    owl:Class ;
        rdfs:label       "great grandfather" ;
        rdfs:subClassOf  v3-RoleCode:GGRPRN ;
        <http://www.w3.org/2004/02/skos/core#definition>
                "The player of the role is the father of the scoping person's grandparent." ;
        <http://www.w3.org/2004/02/skos/core#prefLabel>
                "great grandfather" .

v3-RoleCode:PCOUSN  a    owl:Class ;
        rdfs:label       "paternal cousin" ;
        rdfs:subClassOf  v3-RoleCode:COUSN ;
        <http://www.w3.org/2004/02/skos/core#definition>
                "Description:The player of the role is a biological relative of the scoping person descended from a common ancestor on the player's father's side, such as a grandparent, by two or more steps in a diverging line." ;
        <http://www.w3.org/2004/02/skos/core#prefLabel>
                "paternal cousin" .

v3-RoleCode:IEC  a       owl:Class ;
        rdfs:label       "Impairment evaluation center" ;
        rdfs:subClassOf  v3-RoleCode:OF ;
        <http://www.w3.org/2004/02/skos/core#definition>
                "Focuses on assessing disability" ;
        <http://www.w3.org/2004/02/skos/core#prefLabel>
                "Impairment evaluation center" .

v3-RoleCode:CHLDADOPT
        a                owl:Class ;
        rdfs:label       "adopted child" ;
        rdfs:subClassOf  v3-RoleCode:CHILD ;
        <http://www.w3.org/2004/02/skos/core#definition>
                "The player of the role is a child taken into a family through legal means and raised by the scoping person (parent) as his or her own child." ;
        <http://www.w3.org/2004/02/skos/core#prefLabel>
                "adopted child" .

v3-RoleCode:DEPEN  a  owl:Class ;
        rdfs:label  "dependent" ;
        <http://www.w3.org/2004/02/skos/core#definition>
                "A party covered under a policy based on association with a subscriber." ;
        <http://www.w3.org/2004/02/skos/core#prefLabel>
                "dependent" .

v3-RoleCode:_SubscriberCoveredPartyRoleType
        a                owl:Class ;
        rdfs:label       "SubscriberCoveredPartyRoleType" ;
        rdfs:subClassOf  v3-RoleCode:_CoveredPartyRoleType ;
        <http://www.w3.org/2004/02/skos/core#definition>
                "Description: A role recognized through the eligibility of a party to play a subscriber for benefits covered or provided under a health insurance policy." ;
        <http://www.w3.org/2004/02/skos/core#prefLabel>
                "SubscriberCoveredPartyRoleType" .

v3-RoleCode:_CitizenRoleType
        a           owl:Class ;
        rdfs:label  "CitizenRoleType" ;
        <http://www.w3.org/2004/02/skos/core#definition>
                "A role type used to qualify a person's legal status within a country or nation." ;
        <http://www.w3.org/2004/02/skos/core#prefLabel>
                "CitizenRoleType" .

v3-RoleCode:RHPIH  a     owl:Class ;
        rdfs:label       "physical impairment - hearing center" ;
        rdfs:subClassOf  v3-RoleCode:RHPI ;
        <http://www.w3.org/2004/02/skos/core#definition>
                "Description: A location that plays the role of delivering services for people with hearing impairments." ;
        <http://www.w3.org/2004/02/skos/core#prefLabel>
                "physical impairment - hearing center" .

v3-RoleCode:STPSON  a    owl:Class ;
        rdfs:label       "stepson" ;
        rdfs:subClassOf  v3-RoleCode:SONC ;
        <http://www.w3.org/2004/02/skos/core#definition>
                "The player of the role is a son of the scoping person's spouse by a previous union." ;
        <http://www.w3.org/2004/02/skos/core#prefLabel>
                "stepson" .

v3-RoleCode:GGRMTH  a    owl:Class ;
        rdfs:label       "great grandmother" ;
        rdfs:subClassOf  v3-RoleCode:GGRPRN ;
        <http://www.w3.org/2004/02/skos/core#definition>
                "The player of the role is the mother of the scoping person's grandparent." ;
        <http://www.w3.org/2004/02/skos/core#prefLabel>
                "great grandmother" .

v3-RoleCode:CHLDFOST  a  owl:Class ;
        rdfs:label       "foster child" ;
        rdfs:subClassOf  v3-RoleCode:CHILD ;
        <http://www.w3.org/2004/02/skos/core#definition>
                "The player of the role is a child receiving parental care and nurture from the scoping person (parent) but not related to him or her through legal or blood ties." ;
        <http://www.w3.org/2004/02/skos/core#prefLabel>
                "foster child" .

v3-RoleCode:SIBINLAW  a  owl:Class ;
        rdfs:label       "sibling in-law" ;
        rdfs:subClassOf  v3-RoleCode:INLAW ;
        <http://www.w3.org/2004/02/skos/core#definition>
                "The player of the role is: (1) a sibling of the scoping person's spouse, or (2) the spouse of the scoping person's sibling, or (3) the spouse of a sibling of the scoping person's spouse." ;
        <http://www.w3.org/2004/02/skos/core#prefLabel>
                "sibling in-law" .

v3-RoleCode:MUNCLE  a    owl:Class ;
        rdfs:label       "maternal uncle" ;
        rdfs:subClassOf  v3-RoleCode:UNCLE ;
        <http://www.w3.org/2004/02/skos/core#definition>
                "Description:The player of the role is a biological brother of the scoping person's biological mother." ;
        <http://www.w3.org/2004/02/skos/core#prefLabel>
                "maternal uncle" .

v3-RoleCode:CNRPM  a     owl:Class ;
        rdfs:label       "non-country member minor without residence permit" ;
        rdfs:subClassOf  v3-RoleCode:CNRP ;
        <http://www.w3.org/2004/02/skos/core#definition>
                "A person who is below legal age present in a country, without his or her parents, (which is foreign to him/her) unlawfully or without the country's authorization." ;
        <http://www.w3.org/2004/02/skos/core#prefLabel>
                "non-country member minor without residence permit" .

v3-RoleCode:NEPHEW  a    owl:Class ;
        rdfs:label       "nephew" ;
        rdfs:subClassOf  v3-RoleCode:NIENEPH ;
        <http://www.w3.org/2004/02/skos/core#definition>
                "The player of the role is a son of the scoping person's brother or sister or of the brother or sister of the \tscoping person's spouse." ;
        <http://www.w3.org/2004/02/skos/core#prefLabel>
                "nephew" .

v3-RoleCode:_DependentCoveredPartyRoleType
        a                owl:Class ;
        rdfs:label       "DependentCoveredPartyRoleType" ;
        rdfs:subClassOf  v3-RoleCode:_CoveredPartyRoleType ;
        <http://www.w3.org/2004/02/skos/core#definition>
                "Description: A role recognized through the eligibility of a party to play a dependent for benefits covered or provided under a health insurance policy because of an association with the subscriber that is recognized by the policy underwriter." ;
        <http://www.w3.org/2004/02/skos/core#prefLabel>
                "DependentCoveredPartyRoleType" .

v3-RoleCode:RETIREE  a   owl:Class ;
        rdfs:label       "retiree" ;
        rdfs:subClassOf  v3-RoleCode:_IndividualInsuredPartyRoleType ;
        <http://www.w3.org/2004/02/skos/core#definition>
                "Description: A person playing the role of an individual insured under a policy based on meeting criteria for the employment status of retired set by law or the policy.\r\n\n                        \n                           Discussion: This CoveredPartyRoleType.code is typically used when the CoveredPartyRole class code is either \"program eligible\" or \"subscriber\" and the person's status as a retiree meets jurisdictional or policy criteria." ;
        <http://www.w3.org/2004/02/skos/core#prefLabel>
                "retiree" .

v3-RoleCode:  a          owl:Ontology ;
        rdfs:comment     " A set of codes further specifying the kind of Role; specific classification codes for further qualifying RoleClass codes." ;
        rdfs:label       "v3 Code System RoleCode" ;
        owl:versionIRI   "http://hl7.org/fhir/v3/RoleCode/2016-11-11" ;
        owl:versionInfo  "v3 Code System RoleCode(2016-11-11)" .

v3-RoleCode:_MedicationGeneralizationRoleType
        a           owl:Class ;
        rdfs:label  "MedicationGeneralizationRoleType" ;
        <http://www.w3.org/2004/02/skos/core#definition>
                "Identifies the specific hierarchical relationship between the playing and scoping medications. \r\n\n                        \n                           Examples: Generic, Generic Formulation, Therapeutic Class, etc." ;
        <http://www.w3.org/2004/02/skos/core#prefLabel>
                "MedicationGeneralizationRoleType" .

v3-RoleCode:O  a         owl:Class ;
        rdfs:label       "Operator Proficiency" ;
        rdfs:subClassOf  v3-RoleCode:Q ;
        <http://www.w3.org/2004/02/skos/core#definition>
                "A specimen used for evaluation of operator proficiency (operator in what context?)" ;
        <http://www.w3.org/2004/02/skos/core#prefLabel>
                "Operator Proficiency" .

v3-RoleCode:_DedicatedClinicalLocationRoleType
        a                owl:Class ;
        rdfs:label       "DedicatedClinicalLocationRoleType" ;
        rdfs:subClassOf  v3-RoleCode:_DedicatedServiceDeliveryLocationRoleType ;
        <http://www.w3.org/2004/02/skos/core#definition>
                "A role of a place that further classifies the clinical setting (e.g., cardiology clinic, primary care clinic, rehabilitation hospital, skilled nursing facility) in which care is delivered during an encounter." ;
        <http://www.w3.org/2004/02/skos/core#prefLabel>
                "DedicatedClinicalLocationRoleType" .

v3-RoleCode:MGGRPRN  a   owl:Class ;
        rdfs:label       "maternal great-grandparent" ;
        rdfs:subClassOf  v3-RoleCode:GGRPRN ;
        <http://www.w3.org/2004/02/skos/core#definition>
                "Description:The player of the role is a biological parent of the scoping person's biological mother's parent." ;
        <http://www.w3.org/2004/02/skos/core#prefLabel>
                "maternal great-grandparent" .

v3-RoleCode:DR  a        owl:Class ;
        rdfs:label       "Draft" ;
        rdfs:subClassOf  v3-RoleCode:_LivingSubjectProductionClass ;
        <http://www.w3.org/2004/02/skos/core#definition>
                "Draft animals" ;
        <http://www.w3.org/2004/02/skos/core#prefLabel>
                "Draft" .

v3-RoleCode:ACC  a       owl:Class ;
        rdfs:label       "accident site" ;
        rdfs:subClassOf  v3-RoleCode:_IncidentalServiceDeliveryLocationRoleType ;
        <http://www.w3.org/2004/02/skos/core#definition>
                "Location of an accident where healthcare service was delivered, such as a roadside." ;
        <http://www.w3.org/2004/02/skos/core#prefLabel>
                "accident site" .

v3-RoleCode:GRFTH  a     owl:Class ;
        rdfs:label       "grandfather" ;
        rdfs:subClassOf  v3-RoleCode:GRPRN ;
        <http://www.w3.org/2004/02/skos/core#definition>
                "The player of the role is the father of the scoping person's mother or father." ;
        <http://www.w3.org/2004/02/skos/core#prefLabel>
                "grandfather" .

v3-RoleCode:TWIN  a      owl:Class ;
        rdfs:label       "twin" ;
        rdfs:subClassOf  v3-RoleCode:NSIB ;
        <http://www.w3.org/2004/02/skos/core#definition>
                "The scoper and player were carried in the same womb and shared common biological parents." ;
        <http://www.w3.org/2004/02/skos/core#prefLabel>
                "twin" .

v3-RoleCode:PSTUD  a     owl:Class ;
        rdfs:label       "part-time student" ;
        rdfs:subClassOf  v3-RoleCode:STUD ;
        <http://www.w3.org/2004/02/skos/core#definition>
                "Covered party to an insurance policy has coverage through part-time attendance at a recognized educational institution as defined by a particular insurance policy." ;
        <http://www.w3.org/2004/02/skos/core#prefLabel>
                "part-time student" .

v3-RoleCode:INFD  a      owl:Class ;
        rdfs:label       "Infectious disease clinic" ;
        rdfs:subClassOf  v3-RoleCode:OF ;
        <http://www.w3.org/2004/02/skos/core#definition>
                "Infectious disease clinic" ;
        <http://www.w3.org/2004/02/skos/core#prefLabel>
                "Infectious disease clinic" .

v3-RoleCode:CNRP  a      owl:Class ;
        rdfs:label       "non-country member without residence permit" ;
        rdfs:subClassOf  v3-RoleCode:_CitizenRoleType ;
        <http://www.w3.org/2004/02/skos/core#definition>
                "A foreigner who is present in a country (which is foreign to him/her) unlawfully or without the country's authorization (may be called an illegal alien)." ;
        <http://www.w3.org/2004/02/skos/core#prefLabel>
                "non-country member without residence permit" .

v3-RoleCode:_DedicatedServiceDeliveryLocationRoleType
        a                owl:Class ;
        rdfs:label       "DedicatedServiceDeliveryLocationRoleType" ;
        rdfs:subClassOf  v3-RoleCode:_ServiceDeliveryLocationRoleType ;
        <http://www.w3.org/2004/02/skos/core#definition>
                "A role of a place that further classifies a setting that is intended to house the provision of services." ;
        <http://www.w3.org/2004/02/skos/core#prefLabel>
                "DedicatedServiceDeliveryLocationRoleType" .

v3-RoleCode:PGRPRN  a    owl:Class ;
        rdfs:label       "paternal grandparent" ;
        rdfs:subClassOf  v3-RoleCode:GRPRN ;
        <http://www.w3.org/2004/02/skos/core#definition>
                "Description:The player of the role is the biological parent of the scoping person's biological father." ;
        <http://www.w3.org/2004/02/skos/core#prefLabel>
                "paternal grandparent" .

v3-RoleCode:INLAW  a     owl:Class ;
        rdfs:label       "inlaw" ;
        rdfs:subClassOf  v3-RoleCode:EXT ;
        <http://www.w3.org/2004/02/skos/core#definition>
                "A relationship between an individual and a member of their spousal partner's immediate family." ;
        <http://www.w3.org/2004/02/skos/core#prefLabel>
                "inlaw" .

v3-RoleCode:WIFE  a      owl:Class ;
        rdfs:label       "wife" ;
        rdfs:subClassOf  v3-RoleCode:SPS ;
        <http://www.w3.org/2004/02/skos/core#definition>
                "The player of the role is a woman joined to a man (scoping person) in marriage." ;
        <http://www.w3.org/2004/02/skos/core#prefLabel>
                "wife" .

v3-RoleCode:GRMTH  a     owl:Class ;
        rdfs:label       "grandmother" ;
        rdfs:subClassOf  v3-RoleCode:GRPRN ;
        <http://www.w3.org/2004/02/skos/core#definition>
                "The player of the role is the mother of the scoping person's mother or father." ;
        <http://www.w3.org/2004/02/skos/core#prefLabel>
                "grandmother" .

v3-RoleCode:BIOTH  a     owl:Class ;
        rdfs:label       "Biotherapeutic non-person living subject" ;
        rdfs:subClassOf  v3-RoleCode:_AssignedNonPersonLivingSubjectRoleType ;
        <http://www.w3.org/2004/02/skos/core#definition>
                "Description:Animals, including fish and insects, and microorganisms which may participate as assigned entities in biotherapies." ;
        <http://www.w3.org/2004/02/skos/core#prefLabel>
                "Biotherapeutic non-person living subject" .

v3-RoleCode:CRS  a       owl:Class ;
        rdfs:label       "Colon and rectal surgery clinic" ;
        rdfs:subClassOf  v3-RoleCode:OF ;
        <http://www.w3.org/2004/02/skos/core#definition>
                "Colon and rectal surgery clinic" ;
        <http://www.w3.org/2004/02/skos/core#prefLabel>
                "Colon and rectal surgery clinic" .

v3-RoleCode:NIENE  a     owl:Class ;
        rdfs:label       "niece/nephew" ;
        rdfs:subClassOf  v3-RoleCode:_CoverageRoleType ;
        <http://www.w3.org/2004/02/skos/core#definition>
                "A child of one's brother or sister or of the brother or sister of one's spouse." ;
        <http://www.w3.org/2004/02/skos/core#prefLabel>
                "niece/nephew" .

v3-RoleCode:GRNDSON  a   owl:Class ;
        rdfs:label       "grandson" ;
        rdfs:subClassOf  v3-RoleCode:GRNDCHILD ;
        <http://www.w3.org/2004/02/skos/core#definition>
                "The player of the role is a son of the scoping person's son or daughter." ;
        <http://www.w3.org/2004/02/skos/core#prefLabel>
                "grandson" .

v3-RoleCode:HAND  a      owl:Class ;
        rdfs:label       "Hand clinic" ;
        rdfs:subClassOf  v3-RoleCode:ORTHO ;
        <http://www.w3.org/2004/02/skos/core#definition>
                "Hand clinic" ;
        <http://www.w3.org/2004/02/skos/core#prefLabel>
                "Hand clinic" .

v3-RoleCode:GDS  a       owl:Class ;
        rdfs:label       "generic drug strength" ;
        rdfs:subClassOf  v3-RoleCode:GD ;
        <http://www.w3.org/2004/02/skos/core#definition>
                "Relates a manufactured drug product to the non-proprietary (generic) representation of is ingredients with their strength.  The scoping entity identifies a unique combination of medicine ingredients with their strength." ;
        <http://www.w3.org/2004/02/skos/core#prefLabel>
                "generic drug strength" .

v3-RoleCode:SEE  a       owl:Class ;
        rdfs:label       "Seeing" ;
        rdfs:subClassOf  v3-RoleCode:_AssignedNonPersonLivingSubjectRoleType ;
        <http://www.w3.org/2004/02/skos/core#definition>
                "Description:Dogs trained to assist persons who are seeing impaired or blind." ;
        <http://www.w3.org/2004/02/skos/core#prefLabel>
                "Seeing" .

v3-RoleCode:SISINLAW  a  owl:Class ;
        rdfs:label       "sister-in-law" ;
        rdfs:subClassOf  v3-RoleCode:SIBINLAW ;
        <http://www.w3.org/2004/02/skos/core#definition>
                "The player of the role is: (1) a sister of the scoping person's spouse, or (2) the wife of the scoping person's brother, or (3) the wife of a brother of the scoping person's spouse." ;
        <http://www.w3.org/2004/02/skos/core#prefLabel>
                "sister-in-law" .

v3-RoleCode:ITWINSIS  a  owl:Class ;
        rdfs:label       "identical twin sister" ;
        rdfs:subClassOf  v3-RoleCode:TWINSIS ;
        <http://www.w3.org/2004/02/skos/core#definition>
                "The female scoper is an offspring of the same egg-sperm pair as the female player." ;
        <http://www.w3.org/2004/02/skos/core#prefLabel>
                "identical twin sister" .

v3-RoleCode:communityLaboratory
        a           owl:Class ;
        rdfs:label  "Community Laboratory" ;
        <http://www.w3.org/2004/02/skos/core#definition>
                "Community Laboratory" ;
        <http://www.w3.org/2004/02/skos/core#prefLabel>
                "Community Laboratory" .

v3-RoleCode:NPRN  a      owl:Class ;
        rdfs:label       "natural parent" ;
        rdfs:subClassOf  v3-RoleCode:PRN ;
        <http://www.w3.org/2004/02/skos/core#definition>
                "natural parent" ;
        <http://www.w3.org/2004/02/skos/core#prefLabel>
                "natural parent" .

v3-RoleCode:BROINLAW  a  owl:Class ;
        rdfs:label       "brother-in-law" ;
        rdfs:subClassOf  v3-RoleCode:SIBINLAW ;
        <http://www.w3.org/2004/02/skos/core#definition>
                "The player of the role is: (1) a brother of the scoping person's spouse, or (2) the husband of the scoping person's sister, or (3) the husband of a sister of the scoping person's spouse." ;
        <http://www.w3.org/2004/02/skos/core#prefLabel>
                "brother-in-law" .

v3-RoleCode:STPCHLD  a   owl:Class ;
        rdfs:label       "step child" ;
        rdfs:subClassOf  v3-RoleCode:CHILD ;
        <http://www.w3.org/2004/02/skos/core#definition>
                "The player of the role is a child of the scoping person's spouse by a previous union." ;
        <http://www.w3.org/2004/02/skos/core#prefLabel>
                "step child" .

v3-RoleCode:PEDC  a      owl:Class ;
        rdfs:label       "Pediatrics clinic" ;
        rdfs:subClassOf  v3-RoleCode:OF ;
        <http://www.w3.org/2004/02/skos/core#definition>
                "Pediatrics clinic" ;
        <http://www.w3.org/2004/02/skos/core#prefLabel>
                "Pediatrics clinic" .

v3-RoleCode:TWINSIS  a   owl:Class ;
        rdfs:label       "twin sister" ;
        rdfs:subClassOf  v3-RoleCode:NSIS ;
        <http://www.w3.org/2004/02/skos/core#definition>
                "The scoper was carried in the same womb as the female player and shares common biological parents." ;
        <http://www.w3.org/2004/02/skos/core#prefLabel>
                "twin sister" .

v3-RoleCode:MGRFTH  a    owl:Class ;
        rdfs:label       "maternal grandfather" ;
        rdfs:subClassOf  v3-RoleCode:GRFTH ;
        <http://www.w3.org/2004/02/skos/core#definition>
                "Description:The player of the role is the biological father of the scoping person's biological mother." ;
        <http://www.w3.org/2004/02/skos/core#prefLabel>
                "maternal grandfather" .

v3-RoleCode:_PersonalRelationshipRoleType
        a           owl:Class ;
        rdfs:label  "PersonalRelationshipRoleType" ;
        <http://www.w3.org/2004/02/skos/core#definition>
                "PersonalRelationshipRoleType" ;
        <http://www.w3.org/2004/02/skos/core#prefLabel>
                "PersonalRelationshipRoleType" .

v3-RoleCode:DAUFOST  a   owl:Class ;
        rdfs:label       "foster daughter" ;
        rdfs:subClassOf  v3-RoleCode:CHLDFOST ;
        <http://www.w3.org/2004/02/skos/core#definition>
                "The player of the role is a female child receiving parental care and nurture from the scoping person (parent) but not related to him or her through legal or blood ties." ;
        <http://www.w3.org/2004/02/skos/core#prefLabel>
                "foster daughter" .

v3-RoleCode:GYN  a       owl:Class ;
        rdfs:label       "Gynecology clinic" ;
        rdfs:subClassOf  v3-RoleCode:OF ;
        <http://www.w3.org/2004/02/skos/core#definition>
                "Gynecology clinic" ;
        <http://www.w3.org/2004/02/skos/core#prefLabel>
                "Gynecology clinic" .

v3-RoleCode:WO  a        owl:Class ;
        rdfs:label       "Working" ;
        rdfs:subClassOf  v3-RoleCode:_LivingSubjectProductionClass ;
        <http://www.w3.org/2004/02/skos/core#definition>
                "Animals used to perform work" ;
        <http://www.w3.org/2004/02/skos/core#prefLabel>
                "Working" .

v3-RoleCode:_LocationIdentifiedEntityRoleCode
        a                owl:Class ;
        rdfs:label       "LocationIdentifiedEntityRoleCode" ;
        rdfs:subClassOf  v3-RoleCode:_IdentifiedEntityType ;
        <http://www.w3.org/2004/02/skos/core#definition>
                "Description:Describes types of identifiers other than the primary location registry identifier for a service delivery location.  Identifiers may be assigned by a local service delivery organization, a formal body capable of accrediting the location for the capability to provide specific services or the identifier may be assigned at a jurisdictional level." ;
        <http://www.w3.org/2004/02/skos/core#prefLabel>
                "LocationIdentifiedEntityRoleCode" .

v3-RoleCode:DOMPART  a   owl:Class ;
        rdfs:label       "domestic partner" ;
        rdfs:subClassOf  v3-RoleCode:SIGOTHR ;
        <http://www.w3.org/2004/02/skos/core#definition>
                "The player of the role cohabits with the scoping person but is not the scoping person's spouse." ;
        <http://www.w3.org/2004/02/skos/core#prefLabel>
                "domestic partner" .

v3-RoleCode:FTH  a       owl:Class ;
        rdfs:label       "father" ;
        rdfs:subClassOf  v3-RoleCode:PRN ;
        <http://www.w3.org/2004/02/skos/core#definition>
                "The player of the role is a male who begets or raises or nurtures the scoping entity (child)." ;
        <http://www.w3.org/2004/02/skos/core#prefLabel>
                "father" .

v3-RoleCode:RHYAD  a     owl:Class ;
        rdfs:label       "youths with adjustment difficulties center" ;
        rdfs:subClassOf  v3-RoleCode:RH ;
        <http://www.w3.org/2004/02/skos/core#definition>
                "Description: A location that plays the role of delivering services which may include life training and/or social support services for the adaption, rehabilitation and social integration of youths with adjustment difficulties." ;
        <http://www.w3.org/2004/02/skos/core#prefLabel>
                "youths with adjustment difficulties center" .

v3-RoleCode:MGRMTH  a    owl:Class ;
        rdfs:label       "maternal grandmother" ;
        rdfs:subClassOf  v3-RoleCode:GRMTH ;
        <http://www.w3.org/2004/02/skos/core#definition>
                "Description:The player of the role is the biological mother of the scoping person's biological mother." ;
        <http://www.w3.org/2004/02/skos/core#prefLabel>
                "maternal grandmother" .

v3-RoleCode:CONSENTER
        a                owl:Class ;
        rdfs:label       "consenter" ;
        rdfs:subClassOf  v3-RoleCode:_AgentRoleType ;
        <http://www.w3.org/2004/02/skos/core#definition>
                "An entity or an entity's delegatee who is the grantee in an agreement such as a consent for services, advanced directive, or a privacy consent directive in accordance with jurisdictional, organizational, or patient policy." ;
        <http://www.w3.org/2004/02/skos/core#prefLabel>
                "consenter" .

v3-RoleCode:homeHealth
        a           owl:Class ;
        rdfs:label  "Home Health" ;
        <http://www.w3.org/2004/02/skos/core#definition>
                "Home Health" ;
        <http://www.w3.org/2004/02/skos/core#prefLabel>
                "Home Health" .

v3-RoleCode:MTH  a       owl:Class ;
        rdfs:label       "mother" ;
        rdfs:subClassOf  v3-RoleCode:PRN ;
        <http://www.w3.org/2004/02/skos/core#definition>
                "The player of the role is a female who conceives, gives birth to, or raises and nurtures the scoping entity (child)." ;
        <http://www.w3.org/2004/02/skos/core#prefLabel>
                "mother" .

v3-RoleCode:DX  a        owl:Class ;
        rdfs:label       "Diagnostics or therapeutics unit" ;
        rdfs:subClassOf  v3-RoleCode:_DedicatedClinicalLocationRoleType ;
        <http://www.w3.org/2004/02/skos/core#definition>
                "A practice setting where diagnostic procedures or therapeutic interventions are performed" ;
        <http://www.w3.org/2004/02/skos/core#prefLabel>
                "Diagnostics or therapeutics unit" .

v3-RoleCode:HD  a        owl:Class ;
        rdfs:label       "Hemodialysis unit" ;
        rdfs:subClassOf  v3-RoleCode:HU ;
        <http://www.w3.org/2004/02/skos/core#definition>
                "Hemodialysis unit" ;
        <http://www.w3.org/2004/02/skos/core#prefLabel>
                "Hemodialysis unit" .

v3-RoleCode:OF  a        owl:Class ;
        rdfs:label       "Outpatient facility" ;
        rdfs:subClassOf  v3-RoleCode:_DedicatedClinicalLocationRoleType ;
        <http://www.w3.org/2004/02/skos/core#definition>
                "Outpatient facility" ;
        <http://www.w3.org/2004/02/skos/core#prefLabel>
                "Outpatient facility" .

v3-RoleCode:_CoverageSponsorRoleType
        a                owl:Class ;
        rdfs:label       "CoverageSponsorRoleType" ;
        rdfs:subClassOf  v3-RoleCode:_AffiliationRoleType ;
        <http://www.w3.org/2004/02/skos/core#definition>
                "Description:Codes that indicate a specific type of sponsor.  Used when the sponsor's role is only either as a fully insured sponsor or only as a self-insured sponsor.  NOTE: Where a sponsor may be either, use the SponsorParticipationFunction.code (fully insured or self insured) to indicate the type of responsibility. (CO6-0057)" ;
        <http://www.w3.org/2004/02/skos/core#prefLabel>
                "CoverageSponsorRoleType" .

v3-RoleCode:ENROLBKR  a  owl:Class ;
        rdfs:label       "Enrollment Broker" ;
        rdfs:subClassOf  v3-RoleCode:_PayorRoleType ;
        <http://www.w3.org/2004/02/skos/core#definition>
                "Description:A payor that is responsible for functions related to the enrollment of covered parties." ;
        <http://www.w3.org/2004/02/skos/core#prefLabel>
                "Enrollment Broker" .

v3-RoleCode:HPOWATT  a   owl:Class ;
        rdfs:label       "healthcare power of attorney" ;
        rdfs:subClassOf  v3-RoleCode:POWATT ;
        <http://www.w3.org/2004/02/skos/core#definition>
                "A relationship between two people in which one person authorizes another to act for him or her in a manner which is a legally binding upon the person giving such authority as if he or she personally were to do the acts that continues (by its terms) to be effective even though the grantor has become mentally incompetent after signing the document." ;
        <http://www.w3.org/2004/02/skos/core#prefLabel>
                "healthcare power of attorney" .

v3-RoleCode:_LivingSubjectProductionClass
        a           owl:Class ;
        rdfs:label  "LivingSubjectProductionClass" ;
        <http://www.w3.org/2004/02/skos/core#definition>
                "Code indicating the primary use for which a living subject is bred or grown" ;
        <http://www.w3.org/2004/02/skos/core#prefLabel>
                "LivingSubjectProductionClass" .

v3-RoleCode:FTHFOST  a   owl:Class ;
        rdfs:label       "foster father" ;
        rdfs:subClassOf  v3-RoleCode:FTH ;
        <http://www.w3.org/2004/02/skos/core#definition>
                "The player of the role (parent) who is a male state-certified caregiver responsible for the scoper (child) who has been placed in the parent's care. The placement of the child is usually arranged through the government or a social-service agency, and temporary.\r\n\n                        The state, via a jurisdiction recognized child protection agency, stands as in loco parentis to the child, making all legal decisions while the foster parent is responsible for the day-to-day care of the specified child." ;
        <http://www.w3.org/2004/02/skos/core#prefLabel>
                "foster father" .

v3-RoleCode:UPC  a       owl:Class ;
        rdfs:label       "underage protection center" ;
        rdfs:subClassOf  v3-RoleCode:_IncidentalServiceDeliveryLocationRoleType ;
        <http://www.w3.org/2004/02/skos/core#definition>
                "Description: A location that plays the role of delivering services which may include: social emergency services required for a young person as required under any jurisdictional youth laws, child placement, and family mediation in the defined geographical area the SDL is responsible for. It may provide expertise in a judiciary setting on child custody, adoption and biological history research." ;
        <http://www.w3.org/2004/02/skos/core#prefLabel>
                "underage protection center" .

v3-RoleCode:NMTHF  a     owl:Class ;
        rdfs:label       "natural mother of fetus" ;
        rdfs:subClassOf  v3-RoleCode:NMTH ;
        <http://www.w3.org/2004/02/skos/core#definition>
                "The player is the biologic female parent of the scoping fetus." ;
        <http://www.w3.org/2004/02/skos/core#prefLabel>
                "natural mother of fetus" .

v3-RoleCode:SH  a        owl:Class ;
        rdfs:label       "Show" ;
        rdfs:subClassOf  v3-RoleCode:_LivingSubjectProductionClass ;
        <http://www.w3.org/2004/02/skos/core#definition>
                "Animals raised for shows" ;
        <http://www.w3.org/2004/02/skos/core#prefLabel>
                "Show" .

v3-RoleCode:WND  a       owl:Class ;
        rdfs:label       "Wound clinic" ;
        rdfs:subClassOf  v3-RoleCode:OF ;
        <http://www.w3.org/2004/02/skos/core#definition>
                "Wound clinic" ;
        <http://www.w3.org/2004/02/skos/core#prefLabel>
                "Wound clinic" .

v3-RoleCode:LYMPH  a     owl:Class ;
        rdfs:label       "Lympedema clinic" ;
        rdfs:subClassOf  v3-RoleCode:OF ;
        <http://www.w3.org/2004/02/skos/core#definition>
                "Lympedema clinic" ;
        <http://www.w3.org/2004/02/skos/core#prefLabel>
                "Lympedema clinic" .

v3-RoleCode:FTHINLAW  a  owl:Class ;
        rdfs:label       "father-in-law" ;
        rdfs:subClassOf  v3-RoleCode:PRNINLAW ;
        <http://www.w3.org/2004/02/skos/core#definition>
                "The player of the role is the father of the scoping person's husband or wife." ;
        <http://www.w3.org/2004/02/skos/core#prefLabel>
                "father-in-law" .

v3-RoleCode:PH  a   owl:Class ;
        rdfs:label  "Policy Holder" ;
        <http://www.w3.org/2004/02/skos/core#definition>
                "Policy holder for the insurance policy." ;
        <http://www.w3.org/2004/02/skos/core#prefLabel>
                "Policy Holder" .

v3-RoleCode:FAMMEMB  a   owl:Class ;
        rdfs:label       "family member" ;
        rdfs:subClassOf  v3-RoleCode:_PersonalRelationshipRoleType ;
        <http://www.w3.org/2004/02/skos/core#definition>
                "A relationship between two people characterizing their \"familial\" relationship" ;
        <http://www.w3.org/2004/02/skos/core#prefLabel>
                "family member" .

v3-RoleCode:ASSIST  a    owl:Class ;
        rdfs:label       "Assistive non-person living subject" ;
        rdfs:subClassOf  v3-RoleCode:_AssignedNonPersonLivingSubjectRoleType ;
        <http://www.w3.org/2004/02/skos/core#definition>
                "Description:Dogs trained to assist the ill or physically challenged." ;
        <http://www.w3.org/2004/02/skos/core#prefLabel>
                "Assistive non-person living subject" .

v3-RoleCode:UNCLE  a     owl:Class ;
        rdfs:label       "uncle" ;
        rdfs:subClassOf  v3-RoleCode:EXT ;
        <http://www.w3.org/2004/02/skos/core#definition>
                "The player of the role is a brother of the scoping person's mother or father." ;
        <http://www.w3.org/2004/02/skos/core#prefLabel>
                "uncle" .

v3-RoleCode:SPON  a      owl:Class ;
        rdfs:label       "sponsored dependent" ;
        rdfs:subClassOf  v3-RoleCode:_CoverageRoleType ;
        <http://www.w3.org/2004/02/skos/core#definition>
                "Covered party is an individual that the policy holder has assumed responsibility for, such as foster child or legal ward." ;
        <http://www.w3.org/2004/02/skos/core#prefLabel>
                "sponsored dependent" .

v3-RoleCode:SIB  a       owl:Class ;
        rdfs:label       "sibling" ;
        rdfs:subClassOf  v3-RoleCode:FAMMEMB ;
        <http://www.w3.org/2004/02/skos/core#definition>
                "The player of the role shares one or both parents in common with the scoping entity." ;
        <http://www.w3.org/2004/02/skos/core#prefLabel>
                "sibling" .

v3-RoleCode:PEDID  a     owl:Class ;
        rdfs:label       "Pediatric infectious disease clinic" ;
        rdfs:subClassOf  v3-RoleCode:INFD ;
        <http://www.w3.org/2004/02/skos/core#definition>
                "Pediatric infectious disease clinic" ;
        <http://www.w3.org/2004/02/skos/core#prefLabel>
                "Pediatric infectious disease clinic" .

v3-RoleCode:PEDICU  a    owl:Class ;
        rdfs:label       "Pediatric intensive care unit" ;
        rdfs:subClassOf  v3-RoleCode:ICU ;
        <http://www.w3.org/2004/02/skos/core#definition>
                "Pediatric intensive care unit" ;
        <http://www.w3.org/2004/02/skos/core#prefLabel>
                "Pediatric intensive care unit" .

v3-RoleCode:SPSE  a      owl:Class ;
        rdfs:label       "spouse" ;
        rdfs:subClassOf  v3-RoleCode:_CoverageRoleType ;
        <http://www.w3.org/2004/02/skos/core#definition>
                "A marriage partner; a husband or wife." ;
        <http://www.w3.org/2004/02/skos/core#prefLabel>
                "spouse" .

v3-RoleCode:NCCF  a      owl:Class ;
        rdfs:label       "Nursing or custodial care facility" ;
        rdfs:subClassOf  v3-RoleCode:_DedicatedClinicalLocationRoleType ;
        <http://www.w3.org/2004/02/skos/core#definition>
                "Nursing or custodial care facility" ;
        <http://www.w3.org/2004/02/skos/core#prefLabel>
                "Nursing or custodial care facility" .

v3-RoleCode:E  a         owl:Class ;
        rdfs:label       "Electronic QC" ;
        rdfs:subClassOf  v3-RoleCode:Q ;
        <http://www.w3.org/2004/02/skos/core#definition>
                "An electronically simulated QC specimen" ;
        <http://www.w3.org/2004/02/skos/core#prefLabel>
                "Electronic QC" .

v3-RoleCode:RHPIVS  a    owl:Class ;
        rdfs:label       "physical impairment - visual skills center" ;
        rdfs:subClassOf  v3-RoleCode:RHPI ;
        <http://www.w3.org/2004/02/skos/core#definition>
                "Description: A location that plays the role of delivering services for people with visual skill impairments." ;
        <http://www.w3.org/2004/02/skos/core#prefLabel>
                "physical impairment - visual skills center" .

v3-RoleCode:_AdministrativeContactRoleType
        a                owl:Class ;
        rdfs:label       "AdministrativeContactRoleType" ;
        rdfs:subClassOf  v3-RoleCode:_ContactRoleType ;
        <http://www.w3.org/2004/02/skos/core#definition>
                "A contact role used for business and/or administrative purposes." ;
        <http://www.w3.org/2004/02/skos/core#prefLabel>
                "AdministrativeContactRoleType" .

v3-RoleCode:OUTPHARM  a  owl:Class ;
        rdfs:label       "outpatient pharmacy" ;
        rdfs:subClassOf  v3-RoleCode:HU ;
        <http://www.w3.org/2004/02/skos/core#definition>
                "Description: A location that plays the role of delivering services which may include providing judicious, safe, efficacious, appropriate and cost effective use of medicines for treatment of patients for outpatient visits and may also be used for discharge prescriptions." ;
        <http://www.w3.org/2004/02/skos/core#prefLabel>
                "outpatient pharmacy" .

v3-RoleCode:PARNT  a     owl:Class ;
        rdfs:label       "parent" ;
        rdfs:subClassOf  v3-RoleCode:_CoverageRoleType ;
        <http://www.w3.org/2004/02/skos/core#definition>
                "One that begets or brings forth offspring or a person who brings up and cares for for another (Webster's Collegiate Dictionary)" ;
        <http://www.w3.org/2004/02/skos/core#prefLabel>
                "parent" .

v3-RoleCode:GRNDCHILD
        a                owl:Class ;
        rdfs:label       "grandchild" ;
        rdfs:subClassOf  v3-RoleCode:EXT ;
        <http://www.w3.org/2004/02/skos/core#definition>
                "The player of the role is a child of the scoping person's son or daughter." ;
        <http://www.w3.org/2004/02/skos/core#prefLabel>
                "grandchild" .

v3-RoleCode:FRND  a      owl:Class ;
        rdfs:label       "unrelated friend" ;
        rdfs:subClassOf  v3-RoleCode:_PersonalRelationshipRoleType ;
        <http://www.w3.org/2004/02/skos/core#definition>
                "The player of the role is a person who is known, liked, and trusted by the scoping person." ;
        <http://www.w3.org/2004/02/skos/core#prefLabel>
                "unrelated friend" .

v3-RoleCode:P  a         owl:Class ;
        rdfs:label       "Patient" ;
        rdfs:subClassOf  v3-RoleCode:_SpecimenRoleType ;
        <http://www.w3.org/2004/02/skos/core#definition>
                "A specimen that has been collected from a patient." ;
        <http://www.w3.org/2004/02/skos/core#prefLabel>
                "Patient" .

v3-RoleCode:STEP  a      owl:Class ;
        rdfs:label       "step child" ;
        rdfs:subClassOf  v3-RoleCode:_CoverageRoleType ;
        <http://www.w3.org/2004/02/skos/core#definition>
                "A child receiving parental care and nurture from a person who is related to them through marriage to their parent." ;
        <http://www.w3.org/2004/02/skos/core#prefLabel>
                "step child" .

v3-RoleCode:HEM  a       owl:Class ;
        rdfs:label       "Hematology clinic" ;
        rdfs:subClassOf  v3-RoleCode:OF ;
        <http://www.w3.org/2004/02/skos/core#definition>
                "Hematology clinic" ;
        <http://www.w3.org/2004/02/skos/core#prefLabel>
                "Hematology clinic" .

v3-RoleCode:DIFFABL  a   owl:Class ;
        rdfs:label       "differently abled" ;
        rdfs:subClassOf  v3-RoleCode:_DependentCoveredPartyRoleType ;
        <http://www.w3.org/2004/02/skos/core#definition>
                "Description: A person playing the role of program eligible under a program based on meeting criteria for health or functional limitation set by law or by the program.\r\n\n                        \n                           Discussion: This CoveredPartyRoleType.code is typically used when the CoveredPartyRole class code is either \"program eligible\", \"named insured\", \"individual insured\", or \"dependent\", and the person's status as differently abled meets jurisdictional, policy, or program criteria." ;
        <http://www.w3.org/2004/02/skos/core#prefLabel>
                "differently abled" .

v3-RoleCode:RHMAD  a     owl:Class ;
        rdfs:label       "parents with adjustment difficulties center" ;
        rdfs:subClassOf  v3-RoleCode:RH ;
        <http://www.w3.org/2004/02/skos/core#definition>
                "Description: A location that plays the role of delivering services which may social support services for adolescents who are pregnant or have child and are experiencing adaptation issues/difficulties in their current or eventual parenting role." ;
        <http://www.w3.org/2004/02/skos/core#prefLabel>
                "parents with adjustment difficulties center" .

v3-RoleCode:HRAD  a      owl:Class ;
        rdfs:label       "radiology unit" ;
        rdfs:subClassOf  v3-RoleCode:HU ;
        <http://www.w3.org/2004/02/skos/core#definition>
                "Description: A location that plays the role of delivering services which may include the branch of medicine that uses ionizing and non-ionizing radiation to diagnose and treat diseases.  The radiology unit may be further divided into subspecialties such as Imaging, Cardiovascular, Thoracic, and Ultrasound." ;
        <http://www.w3.org/2004/02/skos/core#prefLabel>
                "radiology unit" .

v3-RoleCode:INJ  a       owl:Class ;
        rdfs:label       "injured plaintiff" ;
        rdfs:subClassOf  v3-RoleCode:_CoverageRoleType ;
        <http://www.w3.org/2004/02/skos/core#definition>
                "Covered party is an injured party with a legal claim for compensation against a policy holder under an insurance policy." ;
        <http://www.w3.org/2004/02/skos/core#prefLabel>
                "injured plaintiff" .

v3-RoleCode:OPTC  a      owl:Class ;
        rdfs:label       "optometry clinic" ;
        rdfs:subClassOf  v3-RoleCode:OF ;
        <http://www.w3.org/2004/02/skos/core#definition>
                "Description: A location that plays the role of delivering services which may include examination, diagnosis, treatment, management, and prevention of diseases and disorders of the eye as well as prescribing and fitting appropriate corrective lenses (glasses or contact lenses) as needed.  Optometry clinics may also provide tests for visual field screening, measuring intra-ocular pressure and ophthalmoscopy, as and when required." ;
        <http://www.w3.org/2004/02/skos/core#prefLabel>
                "optometry clinic" .

v3-RoleCode:NBRO  a      owl:Class ;
        rdfs:label       "natural brother" ;
        rdfs:subClassOf  v3-RoleCode:BRO ;
        <http://www.w3.org/2004/02/skos/core#definition>
                "The player of the role is a male having the same biological parents as the scoping entity." ;
        <http://www.w3.org/2004/02/skos/core#prefLabel>
                "natural brother" .

v3-RoleCode:TPA  a       owl:Class ;
        rdfs:label       "Third party administrator" ;
        rdfs:subClassOf  v3-RoleCode:_PayorRoleType ;
        <http://www.w3.org/2004/02/skos/core#definition>
                "Description:Third party administrator (TPA) is a payor organization that processes health care claims without carrying insurance risk. Third party administrators are prominent players in the managed care industry and have the expertise and capability to administer all or a portion of the claims process. They are normally contracted by a health insurer or self-insuring companies to administer services, including claims administration, premium collection, enrollment and other administrative activities.\r\n\n                        Self-insured employers often contract with third party administrator to handle their insurance functions. Insurance companies oftentimes outsource the claims, utilization review or membership functions to a TPA. Sometimes TPAs only manage provider networks, only claims or only utilization review.\r\n\n                        While some third-party administrators may operate as units of insurance companies, they are often independent. However, hospitals or provider organizations desiring to set up their own health plans will often outsource certain responsibilities to TPAs.  TPAs may perform one or several payor functions, specified by the PayorParticipationFunction value set, such as provider management, enrollment, utilization management, and fee for service claims adjudication management." ;
        <http://www.w3.org/2004/02/skos/core#prefLabel>
                "Third party administrator" .

v3-RoleCode:INLAB  a     owl:Class ;
        rdfs:label       "inpatient laboratory" ;
        rdfs:subClassOf  v3-RoleCode:HLAB ;
        <http://www.w3.org/2004/02/skos/core#definition>
                "Description: A location that plays the role of delivering services which may include tests are done on clinical specimens to get health information about a patient pertaining to the diagnosis, treatment, and prevention of disease for a hospital visit longer than one day." ;
        <http://www.w3.org/2004/02/skos/core#prefLabel>
                "inpatient laboratory" .

v3-RoleCode:RHPIMS  a    owl:Class ;
        rdfs:label       "physical impairment - motor skills center" ;
        rdfs:subClassOf  v3-RoleCode:RHPI ;
        <http://www.w3.org/2004/02/skos/core#definition>
                "Description: A location that plays the role of delivering services for people with motor skill impairments." ;
        <http://www.w3.org/2004/02/skos/core#prefLabel>
                "physical impairment - motor skills center" .

v3-RoleCode:FSTUD  a     owl:Class ;
        rdfs:label       "full-time student" ;
        rdfs:subClassOf  v3-RoleCode:STUD ;
        <http://www.w3.org/2004/02/skos/core#definition>
                "Covered party to an insurance policy has coverage through full-time attendance at a recognized educational institution as defined by a particular insurance policy." ;
        <http://www.w3.org/2004/02/skos/core#prefLabel>
                "full-time student" .

v3-RoleCode:SNF  a       owl:Class ;
        rdfs:label       "Skilled nursing facility" ;
        rdfs:subClassOf  v3-RoleCode:NCCF ;
        <http://www.w3.org/2004/02/skos/core#definition>
                "(X12N 314000000N)" ;
        <http://www.w3.org/2004/02/skos/core#prefLabel>
                "Skilled nursing facility" .

v3-RoleCode:HU  a        owl:Class ;
        rdfs:label       "Hospital unit" ;
        rdfs:subClassOf  v3-RoleCode:_DedicatedClinicalLocationRoleType ;
        <http://www.w3.org/2004/02/skos/core#definition>
                "Hospital unit" ;
        <http://www.w3.org/2004/02/skos/core#prefLabel>
                "Hospital unit" .

v3-RoleCode:INPHARM  a   owl:Class ;
        rdfs:label       "inpatient pharmacy" ;
        rdfs:subClassOf  v3-RoleCode:HU ;
        <http://www.w3.org/2004/02/skos/core#definition>
                "Description: A location that plays the role of delivering services which may include providing judicious, safe, efficacious, appropriate and cost effective use of medicines for treatment of patients for visits longer than one day. The distinction between inpatient pharmacies and retail (or outpatient) pharmacies is that they are part of a patient's continuity of care while staying in the hospital." ;
        <http://www.w3.org/2004/02/skos/core#prefLabel>
                "inpatient pharmacy" .

v3-RoleCode:WARD  a      owl:Class ;
        rdfs:label       "ward" ;
        rdfs:subClassOf  v3-RoleCode:_DependentCoveredPartyRoleType ;
        <http://www.w3.org/2004/02/skos/core#definition>
                "Description: A person, who is a minor or is deemed incompetent, who plays the role of a program eligible where eligibility for coverage is based on meeting program eligibility criteria for status as a ward of a court or jurisdiction.\r\n\n                        \n                           Discussion: This CoveredPartyRoleType.code is typically used when the CoveredPartyRole class code is a \"claimant\", \"program eligible\", a \"named insured\", an \"individual Insured\" or a \"dependent\", and the person's status as a ward meets program or policy criteria. In the case of a ward covered under a program providing financial or health benefits, a governmental agency may take temporary custody of a minor or incompetent for his/her protection and care, e.g., if the ward is suffering from neglect or abuse, or has been in trouble with the law." ;
        <http://www.w3.org/2004/02/skos/core#prefLabel>
                "ward" .

v3-RoleCode:CHR  a       owl:Class ;
        rdfs:label       "Chronic Care Facility" ;
        rdfs:subClassOf  v3-RoleCode:HOSP ;
        <http://www.w3.org/2004/02/skos/core#definition>
                "(1) A hospital including a physical plant and personnel that provides multidisciplinary diagnosis and treatment for diseases that have one or more of the following characteristics: is permanent; leaves residual disability; is caused by nonreversible pathological alteration; requires special training of the patient for rehabilitation; and/or may be expected to require a long period of supervision or care. In addition, patients require the safety, security, and shelter of these specialized inpatient or partial hospitalization settings. (2) A hospital that provides medical and skilled nursing services to patients with long-term illnesses who are not in an acute phase but who require an intensity of services not available in nursing homes" ;
        <http://www.w3.org/2004/02/skos/core#prefLabel>
                "Chronic Care Facility" .

v3-RoleCode:PGGRPRN  a   owl:Class ;
        rdfs:label       "paternal great-grandparent" ;
        rdfs:subClassOf  v3-RoleCode:GGRPRN ;
        <http://www.w3.org/2004/02/skos/core#definition>
                "Description:The player of the role is a biological parent of the scoping person's biological father's parent." ;
        <http://www.w3.org/2004/02/skos/core#prefLabel>
                "paternal great-grandparent" .

v3-RoleCode:AMENDER  a   owl:Class ;
        rdfs:label       "amender" ;
        rdfs:subClassOf  v3-RoleCode:_AgentRoleType ;
        <http://www.w3.org/2004/02/skos/core#definition>
                "An entity which corrected, edited, or amended pre-existing information." ;
        <http://www.w3.org/2004/02/skos/core#prefLabel>
                "amender" .

v3-RoleCode:STPPRN  a    owl:Class ;
        rdfs:label       "step parent" ;
        rdfs:subClassOf  v3-RoleCode:PRN ;
        <http://www.w3.org/2004/02/skos/core#definition>
                "The player of the role is the spouse of the scoping person's parent and not the scoping person's natural parent." ;
        <http://www.w3.org/2004/02/skos/core#prefLabel>
                "step parent" .

v3-RoleCode:_ServiceDeliveryLocationRoleType
        a           owl:Class ;
        rdfs:label  "ServiceDeliveryLocationRoleType" ;
        <http://www.w3.org/2004/02/skos/core#definition>
                "A role of a place that further classifies the setting (e.g., accident site, road side, work site, community location) in which services are delivered." ;
        <http://www.w3.org/2004/02/skos/core#prefLabel>
                "ServiceDeliveryLocationRoleType" .

v3-RoleCode:ECON  a      owl:Class ;
        rdfs:label       "emergency contact" ;
        rdfs:subClassOf  v3-RoleCode:_ContactRoleType ;
        <http://www.w3.org/2004/02/skos/core#definition>
                "A contact designated for contact in emergent situations." ;
        <http://www.w3.org/2004/02/skos/core#prefLabel>
                "emergency contact" .

v3-RoleCode:ADOPTP  a    owl:Class ;
        rdfs:label       "adoptive parent" ;
        rdfs:subClassOf  v3-RoleCode:PRN ;
        <http://www.w3.org/2004/02/skos/core#definition>
                "The player of the role (parent) has taken the scoper (child) into their family through legal means and raises them as his or her own child." ;
        <http://www.w3.org/2004/02/skos/core#prefLabel>
                "adoptive parent" .

v3-RoleCode:PC  a        owl:Class ;
        rdfs:label       "Primary care clinic" ;
        rdfs:subClassOf  v3-RoleCode:OF ;
        <http://www.w3.org/2004/02/skos/core#definition>
                "(X12N 261QP2300N)" ;
        <http://www.w3.org/2004/02/skos/core#prefLabel>
                "Primary care clinic" .

v3-RoleCode:DAUC  a      owl:Class ;
        rdfs:label       "daughter" ;
        rdfs:subClassOf  v3-RoleCode:CHILD ;
        <http://www.w3.org/2004/02/skos/core#definition>
                "Description: The player of the role is a female child (of any type) of scoping entity (parent)" ;
        <http://www.w3.org/2004/02/skos/core#prefLabel>
                "daughter" .

v3-RoleCode:PHU  a       owl:Class ;
        rdfs:label       "Psychiatric hospital unit" ;
        rdfs:subClassOf  v3-RoleCode:HU ;
        <http://www.w3.org/2004/02/skos/core#definition>
                "(X12N 273R00000N)" ;
        <http://www.w3.org/2004/02/skos/core#prefLabel>
                "Psychiatric hospital unit" .

v3-RoleCode:SPMED  a     owl:Class ;
        rdfs:label       "Sports medicine clinic" ;
        rdfs:subClassOf  v3-RoleCode:OF ;
        <http://www.w3.org/2004/02/skos/core#definition>
                "Sports medicine clinic" ;
        <http://www.w3.org/2004/02/skos/core#prefLabel>
                "Sports medicine clinic" .

v3-RoleCode:FAMDEP  a    owl:Class ;
        rdfs:label       "family dependent" ;
        rdfs:subClassOf  v3-RoleCode:_CoverageRoleType ;
        <http://www.w3.org/2004/02/skos/core#definition>
                "The player of the role is dependent of the scoping entity." ;
        <http://www.w3.org/2004/02/skos/core#prefLabel>
                "family dependent" .

v3-RoleCode:_ProgramEligiblePartyRoleType
        a                owl:Class ;
        rdfs:label       "ProgramEligiblePartyRoleType" ;
        rdfs:subClassOf  v3-RoleCode:_CoveredPartyRoleType ;
        <http://www.w3.org/2004/02/skos/core#definition>
                "Description:A role recognized through the eligibility of a party to play a program eligible for benefits covered or provided under a program." ;
        <http://www.w3.org/2004/02/skos/core#prefLabel>
                "ProgramEligiblePartyRoleType" .

v3-RoleCode:_CertifiedEntityType
        a           owl:Class ;
        rdfs:label  "CertifiedEntityType" ;
        <http://www.w3.org/2004/02/skos/core#definition>
                "Defines types of certifications for all entities" ;
        <http://www.w3.org/2004/02/skos/core#prefLabel>
                "CertifiedEntityType" .

v3-RoleCode:PEDRHEUM  a  owl:Class ;
        rdfs:label       "Pediatric rheumatology clinic" ;
        rdfs:subClassOf  v3-RoleCode:PEDC ;
        <http://www.w3.org/2004/02/skos/core#definition>
                "Pediatric rheumatology clinic" ;
        <http://www.w3.org/2004/02/skos/core#prefLabel>
                "Pediatric rheumatology clinic" .

v3-RoleCode:_ClaimantCoveredPartyRoleType
        a                owl:Class ;
        rdfs:label       "ClaimantCoveredPartyRoleType" ;
        rdfs:subClassOf  v3-RoleCode:_CoveredPartyRoleType ;
        <http://www.w3.org/2004/02/skos/core#definition>
                "DescriptionA role recognized through the eligibility of a party play a claimant for benefits covered or provided under an insurance policy." ;
        <http://www.w3.org/2004/02/skos/core#prefLabel>
                "ClaimantCoveredPartyRoleType" .

v3-RoleCode:DAUINLAW  a  owl:Class ;
        rdfs:label       "daughter in-law" ;
        rdfs:subClassOf  v3-RoleCode:CHLDINLAW ;
        <http://www.w3.org/2004/02/skos/core#definition>
                "The player of the role is the wife of scoping person's son." ;
        <http://www.w3.org/2004/02/skos/core#prefLabel>
                "daughter in-law" .

v3-RoleCode:GCHILD  a    owl:Class ;
        rdfs:label       "grandchild" ;
        rdfs:subClassOf  v3-RoleCode:_CoverageRoleType ;
        <http://www.w3.org/2004/02/skos/core#definition>
                "A child of one's son or daughter." ;
        <http://www.w3.org/2004/02/skos/core#prefLabel>
                "grandchild" .

v3-RoleCode:NAT  a       owl:Class ;
        rdfs:label       "natural child" ;
        rdfs:subClassOf  v3-RoleCode:_CoverageRoleType ;
        <http://www.w3.org/2004/02/skos/core#definition>
                "A child as determined by birth." ;
        <http://www.w3.org/2004/02/skos/core#prefLabel>
                "natural child" .

v3-RoleCode:SIS  a       owl:Class ;
        rdfs:label       "sister" ;
        rdfs:subClassOf  v3-RoleCode:SIB ;
        <http://www.w3.org/2004/02/skos/core#definition>
                "The player of the role is a female sharing one or both parents in common with the scoping entity." ;
        <http://www.w3.org/2004/02/skos/core#prefLabel>
                "sister" .

v3-RoleCode:ONESELF  a   owl:Class ;
        rdfs:label       "self" ;
        rdfs:subClassOf  v3-RoleCode:_PersonalRelationshipRoleType ;
        <http://www.w3.org/2004/02/skos/core#definition>
                "The relationship that a person has with his or her self." ;
        <http://www.w3.org/2004/02/skos/core#prefLabel>
                "self" .

v3-RoleCode:SPOWATT  a   owl:Class ;
        rdfs:label       "special power of attorney" ;
        rdfs:subClassOf  v3-RoleCode:POWATT ;
        <http://www.w3.org/2004/02/skos/core#definition>
                "A relationship between two people in which one person authorizes another to act for him or her in a manner which is a legally binding upon the person giving such authority as if he or she personally were to do the acts that is often limited in the kinds of powers that can be assigned." ;
        <http://www.w3.org/2004/02/skos/core#prefLabel>
                "special power of attorney" .

v3-RoleCode:SELFINS  a   owl:Class ;
        rdfs:label       "Self insured coverage sponsor" ;
        rdfs:subClassOf  v3-RoleCode:_CoverageSponsorRoleType ;
        <http://www.w3.org/2004/02/skos/core#definition>
                "Description:An employer or organization that assumes the financial risk and administrative responsibility for coverage of health services for covered parties." ;
        <http://www.w3.org/2004/02/skos/core#prefLabel>
                "Self insured coverage sponsor" .

v3-RoleCode:_CoveredPartyRoleType
        a                owl:Class ;
        rdfs:label       "covered party role type" ;
        rdfs:subClassOf  v3-RoleCode:_PolicyOrProgramCoverageRoleType ;
        <http://www.w3.org/2004/02/skos/core#definition>
                "A role recognized through the eligibility of an identified living subject for benefits covered under an insurance policy or a program.  Eligibility as a covered party may be conditioned on a relationship with (1) the policy holder such as the policy holder who is covered as an individual under a poliy or as a party sponsored for coverage by the policy holder.\r\n\n                        \n                           Example:An employee as a subscriber; or (2) on being scoped another covered party such as the subscriber, as in the case of a dependent. \r\n\n                        \n                           Discussion:  The Abstract Value Set \"CoverageRoleType\", which was developed for use in the Canadian realm \"pre-coordinate\" coverage roles with other roles that a covered party must play in order to be eligible for coverage, e.g., \"handicapped dependent\".  Other codes in the Abstract Value Set CoveredPartyRoleType domain can be \"post-coordinated\" with the EligiblePartyRoleType codes to denote comparable concepts.  Decoupling the concepts is intended to support a wider range of concepts and semantic comparability of coded concepts." ;
        <http://www.w3.org/2004/02/skos/core#prefLabel>
                "covered party role type" .

v3-RoleCode:GIM  a       owl:Class ;
        rdfs:label       "General internal medicine clinic" ;
        rdfs:subClassOf  v3-RoleCode:OF ;
        <http://www.w3.org/2004/02/skos/core#definition>
                "General internal medicine clinic" ;
        <http://www.w3.org/2004/02/skos/core#prefLabel>
                "General internal medicine clinic" .

v3-RoleCode:DC  a        owl:Class ;
        rdfs:label       "therapeutic class" ;
        rdfs:subClassOf  v3-RoleCode:_MedicationGeneralizationRoleType ;
        <http://www.w3.org/2004/02/skos/core#definition>
                "Description:A categorization of medicinal products by their therapeutic properties and/or main therapeutic use." ;
        <http://www.w3.org/2004/02/skos/core#prefLabel>
                "therapeutic class" .

v3-RoleCode:PSY  a       owl:Class ;
        rdfs:label       "Psychiatry clinic" ;
        rdfs:subClassOf  v3-RoleCode:OF ;
        <http://www.w3.org/2004/02/skos/core#definition>
                "Psychiatry clinic" ;
        <http://www.w3.org/2004/02/skos/core#prefLabel>
                "Psychiatry clinic" .

v3-RoleCode:SONADOPT  a  owl:Class ;
        rdfs:label       "adopted son" ;
        rdfs:subClassOf  v3-RoleCode:CHLDADOPT ;
        <http://www.w3.org/2004/02/skos/core#definition>
                "The player of the role is a male child taken into a family through legal means and raised by the scoping person (parent) as his or her own child." ;
        <http://www.w3.org/2004/02/skos/core#prefLabel>
                "adopted son" .

v3-RoleCode:POWATT  a    owl:Class ;
        rdfs:label       "power of attorney" ;
        rdfs:subClassOf  v3-RoleCode:RESPRSN ;
        <http://www.w3.org/2004/02/skos/core#definition>
                "A relationship between two people in which one person authorizes another to act for him in a manner which is a legally binding upon the person giving such authority as if he or she personally were to do the acts." ;
        <http://www.w3.org/2004/02/skos/core#prefLabel>
                "power of attorney" .

v3-RoleCode:V  a         owl:Class ;
        rdfs:label       "Verifying" ;
        rdfs:subClassOf  v3-RoleCode:Q ;
        <http://www.w3.org/2004/02/skos/core#definition>
                "A specimen used for periodic calibration checks of instruments" ;
        <http://www.w3.org/2004/02/skos/core#prefLabel>
                "Verifying" .

v3-RoleCode:HBRO  a      owl:Class ;
        rdfs:label       "half-brother" ;
        rdfs:subClassOf  v3-RoleCode:BRO ;
        <http://www.w3.org/2004/02/skos/core#definition>
                "The player of the role is a male related to the scoping entity by sharing only one biological parent." ;
        <http://www.w3.org/2004/02/skos/core#prefLabel>
                "half-brother" .

v3-RoleCode:PROCTO  a    owl:Class ;
        rdfs:label       "Proctology clinic" ;
        rdfs:subClassOf  v3-RoleCode:OF ;
        <http://www.w3.org/2004/02/skos/core#definition>
                "Proctology clinic" ;
        <http://www.w3.org/2004/02/skos/core#prefLabel>
                "Proctology clinic" .

v3-RoleCode:_IncidentalServiceDeliveryLocationRoleType
        a                owl:Class ;
        rdfs:label       "IncidentalServiceDeliveryLocationRoleType" ;
        rdfs:subClassOf  v3-RoleCode:_ServiceDeliveryLocationRoleType ;
        <http://www.w3.org/2004/02/skos/core#definition>
                "IncidentalServiceDeliveryLocationRoleType" ;
        <http://www.w3.org/2004/02/skos/core#prefLabel>
                "IncidentalServiceDeliveryLocationRoleType" .

v3-RoleCode:EXCEST  a    owl:Class ;
        rdfs:label       "executor of estate" ;
        rdfs:subClassOf  v3-RoleCode:RESPRSN ;
        <http://www.w3.org/2004/02/skos/core#definition>
                "The role played by a person acting as the estate executor for a deceased subscriber or policyholder who was the responsible party" ;
        <http://www.w3.org/2004/02/skos/core#prefLabel>
                "executor of estate" .

v3-RoleCode:NEPH  a      owl:Class ;
        rdfs:label       "Nephrology clinic" ;
        rdfs:subClassOf  v3-RoleCode:OF ;
        <http://www.w3.org/2004/02/skos/core#definition>
                "Nephrology clinic" ;
        <http://www.w3.org/2004/02/skos/core#prefLabel>
                "Nephrology clinic" .

v3-RoleCode:BREAST  a    owl:Class ;
        rdfs:label       "Breast clinic" ;
        rdfs:subClassOf  v3-RoleCode:OF ;
        <http://www.w3.org/2004/02/skos/core#definition>
                "Breast clinic" ;
        <http://www.w3.org/2004/02/skos/core#prefLabel>
                "Breast clinic" .

v3-RoleCode:MTHFOST  a   owl:Class ;
        rdfs:label       "foster mother" ;
        rdfs:subClassOf  v3-RoleCode:MTH ;
        <http://www.w3.org/2004/02/skos/core#definition>
                "The player of the role (parent) who is a female state-certified caregiver responsible for the scoper (child) who has been placed in the parent's care. The placement of the child is usually arranged through the government or a social-service agency, and temporary.\r\n\n                        The state, via a jurisdiction recognized child protection agency, stands as in loco parentis to the child, making all legal decisions while the foster parent is responsible for the day-to-day care of the specified child." ;
        <http://www.w3.org/2004/02/skos/core#prefLabel>
                "foster mother" .

v3-RoleCode:SLEEP  a     owl:Class ;
        rdfs:label       "Sleep disorders unit" ;
        rdfs:subClassOf  v3-RoleCode:HU ;
        <http://www.w3.org/2004/02/skos/core#definition>
                "(X12N 261QA1200N)" ;
        <http://www.w3.org/2004/02/skos/core#prefLabel>
                "Sleep disorders unit" .

v3-RoleCode:STPDAU  a    owl:Class ;
        rdfs:label       "stepdaughter" ;
        rdfs:subClassOf  v3-RoleCode:DAUC ;
        <http://www.w3.org/2004/02/skos/core#definition>
                "The player of the role is a daughter of the scoping person's spouse by a previous union." ;
        <http://www.w3.org/2004/02/skos/core#prefLabel>
                "stepdaughter" .

v3-RoleCode:CONSWIT  a   owl:Class ;
        rdfs:label       "consent witness" ;
        rdfs:subClassOf  v3-RoleCode:_AgentRoleType ;
        <http://www.w3.org/2004/02/skos/core#definition>
                "An entity which has witnessed and attests to observing another entity being counseled about an agreement such as a consent for services, advanced directive, or a privacy consent directive." ;
        <http://www.w3.org/2004/02/skos/core#prefLabel>
                "consent witness" .

v3-RoleCode:HTN  a       owl:Class ;
        rdfs:label       "Hypertension clinic" ;
        rdfs:subClassOf  v3-RoleCode:OF ;
        <http://www.w3.org/2004/02/skos/core#definition>
                "Hypertension clinic" ;
        <http://www.w3.org/2004/02/skos/core#prefLabel>
                "Hypertension clinic" .

v3-RoleCode:FULLINS  a   owl:Class ;
        rdfs:label       "Fully insured coverage sponsor" ;
        rdfs:subClassOf  v3-RoleCode:_CoverageSponsorRoleType ;
        <http://www.w3.org/2004/02/skos/core#definition>
                "Description:An employer or organization that contracts with an underwriter to assumes the financial risk and administrative responsibility for coverage of health services for covered parties." ;
        <http://www.w3.org/2004/02/skos/core#prefLabel>
                "Fully insured coverage sponsor" .

v3-RoleCode:_SpecimenRoleType
        a           owl:Class ;
        rdfs:label  "SpecimenRoleType" ;
        <http://www.w3.org/2004/02/skos/core#definition>
                "SpecimenRoleType" ;
        <http://www.w3.org/2004/02/skos/core#prefLabel>
                "SpecimenRoleType" .

v3-RoleCode:SON  a       owl:Class ;
        rdfs:label       "natural son" ;
        rdfs:subClassOf  v3-RoleCode:NCHILD ;
        <http://www.w3.org/2004/02/skos/core#definition>
                "The player of the role is a male offspring of the scoping entity (parent)." ;
        <http://www.w3.org/2004/02/skos/core#prefLabel>
                "natural son" .

v3-RoleCode:UMO  a       owl:Class ;
        rdfs:label       "Utilization management organization" ;
        rdfs:subClassOf  v3-RoleCode:_PayorRoleType ;
        <http://www.w3.org/2004/02/skos/core#definition>
                "Description:A payor that is responsible for review and case management of health services covered under a policy or program." ;
        <http://www.w3.org/2004/02/skos/core#prefLabel>
                "Utilization management organization" .

v3-RoleCode:SNIFF  a     owl:Class ;
        rdfs:label       "Sniffing" ;
        rdfs:subClassOf  v3-RoleCode:_AssignedNonPersonLivingSubjectRoleType ;
        <http://www.w3.org/2004/02/skos/core#definition>
                "Description:Dogs trained or having the ability to detect imminent seizures or cancers in humans, probably as a result of volatile chemical (odors) given off by the malignancy of the host." ;
        <http://www.w3.org/2004/02/skos/core#prefLabel>
                "Sniffing" .

v3-RoleCode:FMRSPS  a    owl:Class ;
        rdfs:label       "former spouse" ;
        rdfs:subClassOf  v3-RoleCode:SIGOTHR ;
        <http://www.w3.org/2004/02/skos/core#definition>
                "Player of the role was previously joined to the scoping person in marriage and this marriage is now dissolved and inactive.\r\n\n                        \n                           Usage Note: This is significant to indicate as some jurisdictions have different legal requirements for former spouse to access the patient's record, from a general friend." ;
        <http://www.w3.org/2004/02/skos/core#prefLabel>
                "former spouse" .

v3-RoleCode:CHILD  a     owl:Class ;
        rdfs:label       "child" ;
        rdfs:subClassOf  v3-RoleCode:FAMMEMB ;
        <http://www.w3.org/2004/02/skos/core#definition>
                "The player of the role is a child of the scoping entity." ;
        <http://www.w3.org/2004/02/skos/core#prefLabel>
                "child" .

v3-RoleCode:PT  a   owl:Class ;
        rdfs:label  "Patient" ;
        <http://www.w3.org/2004/02/skos/core#definition>
                "The recipient for the service(s) and/or product(s) when they are not the covered party." ;
        <http://www.w3.org/2004/02/skos/core#prefLabel>
                "Patient" .

v3-RoleCode:CHLDINLAW
        a                owl:Class ;
        rdfs:label       "child-in-law" ;
        rdfs:subClassOf  v3-RoleCode:INLAW ;
        <http://www.w3.org/2004/02/skos/core#definition>
                "The player of the role is the spouse of scoping person's child." ;
        <http://www.w3.org/2004/02/skos/core#prefLabel>
                "child-in-law" .

v3-RoleCode:CRIMEVIC  a  owl:Class ;
        rdfs:label       "crime victim" ;
        rdfs:subClassOf  v3-RoleCode:_ClaimantCoveredPartyRoleType ;
        <http://www.w3.org/2004/02/skos/core#definition>
                "Description: A person playing the role of program eligible under a program based on allegations of being the victim of a crime.\r\n\n                        \n                           Discussion: This CoveredPartyRoleType.code is typically used when the CoveredPartyRole class code is \"program eligible\" and the person's status as a crime victim meets jurisdictional or program criteria." ;
        <http://www.w3.org/2004/02/skos/core#prefLabel>
                "crime victim" .

v3-RoleCode:PSI  a       owl:Class ;
        rdfs:label       "Psychology clinic" ;
        rdfs:subClassOf  v3-RoleCode:OF ;
        <http://www.w3.org/2004/02/skos/core#definition>
                "Psychology clinic" ;
        <http://www.w3.org/2004/02/skos/core#prefLabel>
                "Psychology clinic" .

v3-RoleCode:MT  a        owl:Class ;
        rdfs:label       "Meat" ;
        rdfs:subClassOf  v3-RoleCode:_LivingSubjectProductionClass ;
        <http://www.w3.org/2004/02/skos/core#definition>
                "Animals raised for meat production" ;
        <http://www.w3.org/2004/02/skos/core#prefLabel>
                "Meat" .

v3-RoleCode:CCO  a       owl:Class ;
        rdfs:label       "Clinical Companion" ;
        rdfs:subClassOf  v3-RoleCode:_AssignedNonPersonLivingSubjectRoleType ;
        <http://www.w3.org/2004/02/skos/core#definition>
                "Description:Companion animals, such as dogs, cats, and rabbits, which may be provided to patients to improve general mood, decrease depression and loneliness, and distract from stress-inducing concerns to improve quality of life." ;
        <http://www.w3.org/2004/02/skos/core#prefLabel>
                "Clinical Companion" .

v3-RoleCode:EXT  a       owl:Class ;
        rdfs:label       "extended family member" ;
        rdfs:subClassOf  v3-RoleCode:FAMMEMB ;
        <http://www.w3.org/2004/02/skos/core#definition>
                "Description: A family member not having an immediate genetic or legal relationship e.g. Aunt, cousin, great grandparent, grandchild, grandparent, niece, nephew or uncle." ;
        <http://www.w3.org/2004/02/skos/core#prefLabel>
                "extended family member" .

v3-RoleCode:F  a         owl:Class ;
        rdfs:label       "Filler Proficiency" ;
        rdfs:subClassOf  v3-RoleCode:Q ;
        <http://www.w3.org/2004/02/skos/core#definition>
                "Specimen used for testing proficiency of an organization performing testing (how does this differ from O?)" ;
        <http://www.w3.org/2004/02/skos/core#prefLabel>
                "Filler Proficiency" .

v3-RoleCode:EPIL  a      owl:Class ;
        rdfs:label       "Epilepsy unit" ;
        rdfs:subClassOf  v3-RoleCode:HU ;
        <http://www.w3.org/2004/02/skos/core#definition>
                "Epilepsy unit" ;
        <http://www.w3.org/2004/02/skos/core#prefLabel>
                "Epilepsy unit" .

v3-RoleCode:GI  a        owl:Class ;
        rdfs:label       "Gastroenterology clinic" ;
        rdfs:subClassOf  v3-RoleCode:OF ;
        <http://www.w3.org/2004/02/skos/core#definition>
                "Gastroenterology clinic" ;
        <http://www.w3.org/2004/02/skos/core#prefLabel>
                "Gastroenterology clinic" .

v3-RoleCode:PEDU  a      owl:Class ;
        rdfs:label       "Pediatric unit" ;
        rdfs:subClassOf  v3-RoleCode:HU ;
        <http://www.w3.org/2004/02/skos/core#definition>
                "Pediatric unit" ;
        <http://www.w3.org/2004/02/skos/core#prefLabel>
                "Pediatric unit" .

v3-RoleCode:STPBRO  a    owl:Class ;
        rdfs:label       "stepbrother" ;
        rdfs:subClassOf  v3-RoleCode:BRO ;
        <http://www.w3.org/2004/02/skos/core#definition>
                "The player of the role is a son of the scoping person's stepparent." ;
        <http://www.w3.org/2004/02/skos/core#prefLabel>
                "stepbrother" .

v3-RoleCode:CARD  a      owl:Class ;
        rdfs:label       "Ambulatory Health Care Facilities; Clinic/Center; Rehabilitation: Cardiac Facilities" ;
        rdfs:subClassOf  v3-RoleCode:OF ;
        <http://www.w3.org/2004/02/skos/core#definition>
                "Ambulatory Health Care Facilities; Clinic/Center; Rehabilitation: Cardiac Facilities" ;
        <http://www.w3.org/2004/02/skos/core#prefLabel>
                "Ambulatory Health Care Facilities; Clinic/Center; Rehabilitation: Cardiac Facilities" .

v3-RoleCode:Q  a         owl:Class ;
        rdfs:label       "Quality Control" ;
        rdfs:subClassOf  v3-RoleCode:_SpecimenRoleType ;
        <http://www.w3.org/2004/02/skos/core#definition>
                "A specimen specifically used to verify the sensitivity, specificity, accuracy or other perfomance parameter of a diagnostic test." ;
        <http://www.w3.org/2004/02/skos/core#prefLabel>
                "Quality Control" .

v3-RoleCode:GT  a   owl:Class ;
        rdfs:label  "Guarantor" ;
        <http://www.w3.org/2004/02/skos/core#definition>
                "An individual or organization that makes or gives a promise, assurance, pledge to pay or has paid the healthcare service provider." ;
        <http://www.w3.org/2004/02/skos/core#prefLabel>
                "Guarantor" .

v3-RoleCode:SCN  a       owl:Class ;
        rdfs:label       "screening" ;
        rdfs:subClassOf  v3-RoleCode:_ResearchSubjectRoleBasis ;
        <http://www.w3.org/2004/02/skos/core#definition>
                "Definition:The specific role being played by a research subject participating in the pre-enrollment evaluation portion of  a research study." ;
        <http://www.w3.org/2004/02/skos/core#prefLabel>
                "screening" .

v3-RoleCode:VALIDATOR
        a                owl:Class ;
        rdfs:label       "validator" ;
        rdfs:subClassOf  v3-RoleCode:_AgentRoleType ;
        <http://www.w3.org/2004/02/skos/core#definition>
                "An entity authorized to validate information for inclusion in a record." ;
        <http://www.w3.org/2004/02/skos/core#prefLabel>
                "validator" .

v3-RoleCode:DERM  a      owl:Class ;
        rdfs:label       "Dermatology clinic" ;
        rdfs:subClassOf  v3-RoleCode:OF ;
        <http://www.w3.org/2004/02/skos/core#definition>
                "Dermatology clinic" ;
        <http://www.w3.org/2004/02/skos/core#prefLabel>
                "Dermatology clinic" .

v3-RoleCode:HLAB  a      owl:Class ;
        rdfs:label       "hospital laboratory" ;
        rdfs:subClassOf  v3-RoleCode:HU ;
        <http://www.w3.org/2004/02/skos/core#definition>
                "Description: A location that plays the role of delivering services which may include tests done based on clinical specimens to get health information about a patient as pertaining to the diagnosis, treatment and prevention of disease.  Hospital laboratories may be further divided into specialized units such as Anatomic Pathology, Microbiology, and Biochemistry." ;
        <http://www.w3.org/2004/02/skos/core#prefLabel>
                "hospital laboratory" .

v3-RoleCode:_ContactRoleType
        a           owl:Class ;
        rdfs:label  "ContactRoleType" ;
        <http://www.w3.org/2004/02/skos/core#definition>
                "Types of contact for Role code \"CON\"" ;
        <http://www.w3.org/2004/02/skos/core#prefLabel>
                "ContactRoleType" .

v3-RoleCode:DELEGATEE
        a                owl:Class ;
        rdfs:label       "delegatee" ;
        rdfs:subClassOf  v3-RoleCode:_AgentRoleType ;
        <http://www.w3.org/2004/02/skos/core#definition>
                "A party to whom some right or authority is granted by a delegator." ;
        <http://www.w3.org/2004/02/skos/core#prefLabel>
                "delegatee" .

v3-RoleCode:GRANTEE  a   owl:Class ;
        rdfs:label       "grantee" ;
        rdfs:subClassOf  v3-RoleCode:_AgentRoleType ;
        <http://www.w3.org/2004/02/skos/core#definition>
                "An entity which accepts certain rights or authority from a grantor." ;
        <http://www.w3.org/2004/02/skos/core#prefLabel>
                "grantee" .

v3-RoleCode:_PolicyOrProgramCoverageRoleType
        a           owl:Class ;
        rdfs:label  "PolicyOrProgramCoverageRoleType" ;
        <http://www.w3.org/2004/02/skos/core#definition>
                "Description: A role recognized through the eligibility of an identified party for benefits covered under an insurance policy or a program based on meeting eligibility criteria.\r\n\n                        Eligibility as a covered party may be conditioned on the party meeting criteria to qualify for coverage under a policy or program, which may be mandated by law.  These criteria may be: \r\n\n                        \n                           \n                              The sole basis for coverage, e.g., being differently abled may qualify a person for disability coverage\r\n\n                           \n                           \n                              May more fully qualify a covered party role e.g, being differently abled may qualify an adult child as a dependent\r\n\n                           \n                           \n                              May impact the level of coverage for a covered party under a policy or program, e.g., being differently abled may qualify a program eligible for additional benefits.\r\n\n                           \n                        \n                        \n                           Discussion:  The Abstract Value Set \"CoverageRoleType\", which was developed for use in the Canadian realm \"pre-coordinate\" coverage roles with other roles that a covered party must play in order to be eligible for coverage, e.g., \"handicapped dependent\".   These role.codes may only be used with COVPTY to avoid overlapping concepts that would result from using them to specify the specializations of COVPTY, e.g., the role.class DEPEN should not be used with the role.code family dependent because that relationship has overlapping concepts due to the role.code precoodination and is conveyed in FICO with the personal relationship role that has a PART role link to the covered party role.  For the same reasons, the role.class DEPEN should not be used with the role.code HANDIC (handicapped dependent); the role.code DIFFABLE (differently abled) should be used instead.\r\n\n                        In summary, the coded concepts in the Abstract Value Set \"CoveredPartyRoleType\" can be \"post-coordinated\" with the \"RoleClassCoveredParty\" Abstract Value Set.  Decoupling these concepts is intended to support an expansive range of covered party concepts and their semantic comparability." ;
        <http://www.w3.org/2004/02/skos/core#prefLabel>
                "PolicyOrProgramCoverageRoleType" .

v3-RoleCode:INV  a       owl:Class ;
        rdfs:label       "Infertility clinic" ;
        rdfs:subClassOf  v3-RoleCode:OF ;
        <http://www.w3.org/2004/02/skos/core#definition>
                "Infertility clinic" ;
        <http://www.w3.org/2004/02/skos/core#prefLabel>
                "Infertility clinic" .

v3-RoleCode:SELF  a      owl:Class ;
        rdfs:label       "self" ;
        rdfs:subClassOf  v3-RoleCode:_CoverageRoleType ;
        <http://www.w3.org/2004/02/skos/core#definition>
                "Covered party is the policy holder.  Also known as the subscriber." ;
        <http://www.w3.org/2004/02/skos/core#prefLabel>
                "self" .

v3-RoleCode:DELEGATOR
        a                owl:Class ;
        rdfs:label       "delegator" ;
        rdfs:subClassOf  v3-RoleCode:_AgentRoleType ;
        <http://www.w3.org/2004/02/skos/core#definition>
                "A party that grants all or some portion its right or authority to another party." ;
        <http://www.w3.org/2004/02/skos/core#prefLabel>
                "delegator" .

v3-RoleCode:OB  a        owl:Class ;
        rdfs:label       "Obstetrics clinic" ;
        rdfs:subClassOf  v3-RoleCode:OF ;
        <http://www.w3.org/2004/02/skos/core#definition>
                "Obstetrics clinic" ;
        <http://www.w3.org/2004/02/skos/core#prefLabel>
                "Obstetrics clinic" .

v3-RoleCode:NIENEPH  a   owl:Class ;
        rdfs:label       "niece/nephew" ;
        rdfs:subClassOf  v3-RoleCode:EXT ;
        <http://www.w3.org/2004/02/skos/core#definition>
                "The player of the role is a child of scoping person's brother or sister or of the brother or sister of the \tscoping person's spouse." ;
        <http://www.w3.org/2004/02/skos/core#prefLabel>
                "niece/nephew" .

v3-RoleCode:RHU  a       owl:Class ;
        rdfs:label       "Rehabilitation hospital unit" ;
        rdfs:subClassOf  v3-RoleCode:HU ;
        <http://www.w3.org/2004/02/skos/core#definition>
                "Rehabilitation hospital unit" ;
        <http://www.w3.org/2004/02/skos/core#prefLabel>
                "Rehabilitation hospital unit" .

v3-RoleCode:GRANTOR  a   owl:Class ;
        rdfs:label       "grantor" ;
        rdfs:subClassOf  v3-RoleCode:_AgentRoleType ;
        <http://www.w3.org/2004/02/skos/core#definition>
                "An entity which agrees to confer certain rights or authority to a grantee." ;
        <http://www.w3.org/2004/02/skos/core#prefLabel>
                "grantor" .

v3-RoleCode:ONCL  a      owl:Class ;
        rdfs:label       "Medical oncology clinic" ;
        rdfs:subClassOf  v3-RoleCode:OF ;
        <http://www.w3.org/2004/02/skos/core#definition>
                "Medical oncology clinic" ;
        <http://www.w3.org/2004/02/skos/core#prefLabel>
                "Medical oncology clinic" .

v3-RoleCode:ADOPTF  a    owl:Class ;
        rdfs:label       "adoptive father" ;
        rdfs:subClassOf  v3-RoleCode:ADOPTP ;
        <http://www.w3.org/2004/02/skos/core#definition>
                "The player of the role (father) is a male who has taken the scoper (child) into their family through legal means and raises them as his own child." ;
        <http://www.w3.org/2004/02/skos/core#prefLabel>
                "adoptive father" .

v3-RoleCode:ACHFID  a    owl:Class ;
        rdfs:label       "accreditation location identifier" ;
        rdfs:subClassOf  v3-RoleCode:_LocationIdentifiedEntityRoleCode ;
        <http://www.w3.org/2004/02/skos/core#definition>
                "Description:Identifier assigned to a  location by the organization responsible for accrediting the location." ;
        <http://www.w3.org/2004/02/skos/core#prefLabel>
                "accreditation location identifier" .

v3-RoleCode:GRNDDAU  a   owl:Class ;
        rdfs:label       "granddaughter" ;
        rdfs:subClassOf  v3-RoleCode:GRNDCHILD ;
        <http://www.w3.org/2004/02/skos/core#definition>
                "The player of the role is a daughter of the scoping person's son or daughter." ;
        <http://www.w3.org/2004/02/skos/core#prefLabel>
                "granddaughter" .

v3-RoleCode:NFTHF  a     owl:Class ;
        rdfs:label       "natural father of fetus" ;
        rdfs:subClassOf  v3-RoleCode:NFTH ;
        <http://www.w3.org/2004/02/skos/core#definition>
                "Indicates the biologic male parent of a fetus." ;
        <http://www.w3.org/2004/02/skos/core#prefLabel>
                "natural father of fetus" .

v3-RoleCode:CATH  a      owl:Class ;
        rdfs:label       "Cardiac catheterization lab" ;
        rdfs:subClassOf  v3-RoleCode:CVDX ;
        <http://www.w3.org/2004/02/skos/core#definition>
                "Cardiac catheterization lab" ;
        <http://www.w3.org/2004/02/skos/core#prefLabel>
                "Cardiac catheterization lab" .

v3-RoleCode:FM  a   owl:Class ;
        rdfs:label  "Family Member" ;
        <http://www.w3.org/2004/02/skos/core#definition>
                "A member of the covered party's family. This could be the spouse, a parent, a grand parent, a sibling, etc." ;
        <http://www.w3.org/2004/02/skos/core#prefLabel>
                "Family Member" .

v3-RoleCode:ANTIBIOT  a  owl:Class ;
        rdfs:label       "Antibiotic" ;
        rdfs:subClassOf  v3-RoleCode:BIOTH ;
        <http://www.w3.org/2004/02/skos/core#definition>
                "Description:Non-person living subject used as antibiotic.\r\n\n                        \n                           Examples:Bacteriophage, is a virus that infects bacteria." ;
        <http://www.w3.org/2004/02/skos/core#prefLabel>
                "Antibiotic" .

v3-RoleCode:INTPRTER  a  owl:Class ;
        rdfs:label       "interpreter" ;
        rdfs:subClassOf  v3-RoleCode:_AgentRoleType ;
        <http://www.w3.org/2004/02/skos/core#definition>
                "An entity which converts spoken or written language into the language of key participants in an event such as when a provider is obtaining a patient's consent to treatment or permission to disclose information." ;
        <http://www.w3.org/2004/02/skos/core#prefLabel>
                "interpreter" .

v3-RoleCode:DECLASSIFIER
        a                owl:Class ;
        rdfs:label       "declassifier" ;
        rdfs:subClassOf  v3-RoleCode:_AgentRoleType ;
        <http://www.w3.org/2004/02/skos/core#definition>
                "An individual which is authorized to declassify information based on a determination that the information no longer requires protection against unauthorized disclosure.  The individual marks the information being declassified using computable and human readable security labels indicating that this is copy of previously classified information is unclassified in accordance with applicable security labeling policies.  The labeling policies provide instructions on whether and if so how the security labels may be later reclassified [i.e., upgraded or used in derivative classification] in a manner that preserves the overridden original classification binding and provenance." ;
        <http://www.w3.org/2004/02/skos/core#prefLabel>
                "declassifier" .

v3-RoleCode:SCHOOL  a    owl:Class ;
        rdfs:label       "school" ;
        rdfs:subClassOf  v3-RoleCode:_IncidentalServiceDeliveryLocationRoleType ;
        <http://www.w3.org/2004/02/skos/core#definition>
                "Location where healthcare service was delivered, identified as a school or educational facility." ;
        <http://www.w3.org/2004/02/skos/core#prefLabel>
                "school" .

v3-RoleCode:PEDE  a      owl:Class ;
        rdfs:label       "Pediatric endocrinology clinic" ;
        rdfs:subClassOf  v3-RoleCode:ENDO ;
        <http://www.w3.org/2004/02/skos/core#definition>
                "Pediatric endocrinology clinic" ;
        <http://www.w3.org/2004/02/skos/core#prefLabel>
                "Pediatric endocrinology clinic" .

v3-RoleCode:ENDO  a      owl:Class ;
        rdfs:label       "Endocrinology clinic" ;
        rdfs:subClassOf  v3-RoleCode:OF ;
        <http://www.w3.org/2004/02/skos/core#definition>
                "Endocrinology clinic" ;
        <http://www.w3.org/2004/02/skos/core#prefLabel>
                "Endocrinology clinic" .

v3-RoleCode:DEP  a  owl:Class ;
        rdfs:label  "DEP" ;
        <http://www.w3.org/2004/02/skos/core#prefLabel>
                "DEP" .

v3-RoleCode:MGEN  a      owl:Class ;
        rdfs:label       "Medical genetics clinic" ;
        rdfs:subClassOf  v3-RoleCode:OF ;
        <http://www.w3.org/2004/02/skos/core#definition>
                "Medical genetics clinic" ;
        <http://www.w3.org/2004/02/skos/core#prefLabel>
                "Medical genetics clinic" .

v3-RoleCode:GD  a        owl:Class ;
        rdfs:label       "generic drug" ;
        rdfs:subClassOf  v3-RoleCode:_MedicationGeneralizationRoleType ;
        <http://www.w3.org/2004/02/skos/core#definition>
                "Relates a manufactured drug product to the non-proprietary (generic) representation of its ingredients independent of strength, and form.\r\n\n                        The scoping entity identifies a unique combination of medicine ingredients; sometimes referred to as \"ingredient set\"." ;
        <http://www.w3.org/2004/02/skos/core#prefLabel>
                "generic drug" .

v3-RoleCode:_MemberRoleType
        a           owl:Class ;
        rdfs:label  "MemberRoleType" ;
        <http://www.w3.org/2004/02/skos/core#definition>
                "Types of membership for Role code \"MBR\"" ;
        <http://www.w3.org/2004/02/skos/core#prefLabel>
                "MemberRoleType" .

v3-RoleCode:CCU  a       owl:Class ;
        rdfs:label       "Coronary care unit" ;
        rdfs:subClassOf  v3-RoleCode:HU ;
        <http://www.w3.org/2004/02/skos/core#definition>
                "Coronary care unit" ;
        <http://www.w3.org/2004/02/skos/core#prefLabel>
                "Coronary care unit" .

v3-RoleCode:CRPM  a      owl:Class ;
        rdfs:label       "non-country member minor with residence permit" ;
        rdfs:subClassOf  v3-RoleCode:CRP ;
        <http://www.w3.org/2004/02/skos/core#definition>
                "A person who is a resident below legal age of the country without his or her parents and does not have citizenship." ;
        <http://www.w3.org/2004/02/skos/core#prefLabel>
                "non-country member minor with residence permit" .

v3-RoleCode:GGRPRN  a    owl:Class ;
        rdfs:label       "great grandparent" ;
        rdfs:subClassOf  v3-RoleCode:EXT ;
        <http://www.w3.org/2004/02/skos/core#definition>
                "The player of the role is a parent of the scoping person's grandparent." ;
        <http://www.w3.org/2004/02/skos/core#prefLabel>
                "great grandparent" .

v3-RoleCode:L  a         owl:Class ;
        rdfs:label       "Pool" ;
        rdfs:subClassOf  v3-RoleCode:_SpecimenRoleType ;
        <http://www.w3.org/2004/02/skos/core#definition>
                "Aliquots of individual specimens combined to form a single specimen representing all of the included individuals." ;
        <http://www.w3.org/2004/02/skos/core#prefLabel>
                "Pool" .

v3-RoleCode:_IdentifiedEntityType
        a           owl:Class ;
        rdfs:label  "IdentifiedEntityType" ;
        <http://www.w3.org/2004/02/skos/core#definition>
                "Definition: A code representing the type of identifier that has been assigned to the identified entity (IDENT).\r\n\n                        \n                           Examples: Example values include Social Insurance Number, Product Catalog ID, Product Model Number." ;
        <http://www.w3.org/2004/02/skos/core#prefLabel>
                "IdentifiedEntityType" .

v3-RoleCode:PEDHEM  a    owl:Class ;
        rdfs:label       "Pediatric hematology clinic" ;
        rdfs:subClassOf  v3-RoleCode:HEM ;
        <http://www.w3.org/2004/02/skos/core#definition>
                "Pediatric hematology clinic" ;
        <http://www.w3.org/2004/02/skos/core#prefLabel>
                "Pediatric hematology clinic" .

v3-RoleCode:_PayorRoleType
        a                owl:Class ;
        rdfs:label       "PayorRoleType" ;
        rdfs:subClassOf  v3-RoleCode:_AffiliationRoleType ;
        <http://www.w3.org/2004/02/skos/core#definition>
                "Description:PayorRoleType for a particular type of policy or program benefit package or plan where more detail about the coverage administration role of the Payor is required.  The functions performed by a Payor qualified by a PayorRoleType may be specified by the PayorParticpationFunction value set.\r\n\n                        \n                           Examples:A Payor that is a TPA may administer a managed care plan without underwriting the risk." ;
        <http://www.w3.org/2004/02/skos/core#prefLabel>
                "PayorRoleType" .

v3-RoleCode:NEUR  a      owl:Class ;
        rdfs:label       "Neurology clinic" ;
        rdfs:subClassOf  v3-RoleCode:OF ;
        <http://www.w3.org/2004/02/skos/core#definition>
                "Neurology clinic" ;
        <http://www.w3.org/2004/02/skos/core#prefLabel>
                "Neurology clinic" .

v3-RoleCode:FTWINSIS  a  owl:Class ;
        rdfs:label       "fraternal twin sister" ;
        rdfs:subClassOf  v3-RoleCode:TWINSIS ;
        <http://www.w3.org/2004/02/skos/core#definition>
                "The scoper was carried in the same womb as the female player and shares common biological parents but is the product of a distinct egg/sperm pair." ;
        <http://www.w3.org/2004/02/skos/core#prefLabel>
                "fraternal twin sister" .

v3-RoleCode:_IndividualInsuredPartyRoleType
        a                owl:Class ;
        rdfs:label       "IndividualInsuredPartyRoleType" ;
        rdfs:subClassOf  v3-RoleCode:_CoveredPartyRoleType ;
        <http://www.w3.org/2004/02/skos/core#definition>
                "A role recognized through the eligibility of a party to play an individual insured for benefits covered or provided under an insurance policy where the party is also the policy holder." ;
        <http://www.w3.org/2004/02/skos/core#prefLabel>
                "IndividualInsuredPartyRoleType" .

v3-RoleCode:GUADLTM  a   owl:Class ;
        rdfs:label       "guardian ad lidem" ;
        rdfs:subClassOf  v3-RoleCode:RESPRSN ;
        <http://www.w3.org/2004/02/skos/core#definition>
                "The role played by a person appointed by the court to look out for the best interests of a minor child during the course of legal proceedings." ;
        <http://www.w3.org/2004/02/skos/core#prefLabel>
                "guardian ad lidem" .

v3-RoleCode:NCHILD  a    owl:Class ;
        rdfs:label       "natural child" ;
        rdfs:subClassOf  v3-RoleCode:CHILD ;
        <http://www.w3.org/2004/02/skos/core#definition>
                "The player of the role is an offspring of the scoping entity as determined by birth." ;
        <http://www.w3.org/2004/02/skos/core#prefLabel>
                "natural child" .

v3-RoleCode:AMB  a       owl:Class ;
        rdfs:label       "Ambulance" ;
        rdfs:subClassOf  v3-RoleCode:MOBL ;
        <http://www.w3.org/2004/02/skos/core#definition>
                "Location (mobile) where healthcare service was delivered, identified specifically as an ambulance." ;
        <http://www.w3.org/2004/02/skos/core#prefLabel>
                "Ambulance" .

v3-RoleCode:RH  a        owl:Class ;
        rdfs:label       "Rehabilitation hospital" ;
        rdfs:subClassOf  v3-RoleCode:HOSP ;
        <http://www.w3.org/2004/02/skos/core#definition>
                "(X12N 283X00000N)" ;
        <http://www.w3.org/2004/02/skos/core#prefLabel>
                "Rehabilitation hospital" .

v3-RoleCode:MGDSF  a     owl:Class ;
        rdfs:label       "manufactured drug strength form" ;
        rdfs:subClassOf  v3-RoleCode:_MedicationGeneralizationRoleType ;
        <http://www.w3.org/2004/02/skos/core#definition>
                "Relates a manufactured drug product to the non-proprietary (generic) representation of its ingredients with their strength in a specific dose form. The scoping entity identifies a unique combination of medicine ingredients with their strength in a single dose form." ;
        <http://www.w3.org/2004/02/skos/core#prefLabel>
                "manufactured drug strength form" .

v3-RoleCode:CPCA  a      owl:Class ;
        rdfs:label       "permit card applicant" ;
        rdfs:subClassOf  v3-RoleCode:_CitizenRoleType ;
        <http://www.w3.org/2004/02/skos/core#definition>
                "A non-country member admitted to the territory of a nation or country as a non-resident for an explicit purpose." ;
        <http://www.w3.org/2004/02/skos/core#prefLabel>
                "permit card applicant" .

v3-RoleCode:MGGRFTH  a   owl:Class ;
        rdfs:label       "maternal great-grandfather" ;
        rdfs:subClassOf  v3-RoleCode:GGRFTH ;
        <http://www.w3.org/2004/02/skos/core#definition>
                "Description:The player of the role is the biological father of the scoping person's biological mother's parent." ;
        <http://www.w3.org/2004/02/skos/core#prefLabel>
                "maternal great-grandfather" .

v3-RoleCode:RHPI  a      owl:Class ;
        rdfs:label       "physical impairment center" ;
        rdfs:subClassOf  v3-RoleCode:RH ;
        <http://www.w3.org/2004/02/skos/core#definition>
                "Description: A location that plays the role of delivering services which may include adaptation, rehabilitation and social integration services for people with physical impairments." ;
        <http://www.w3.org/2004/02/skos/core#prefLabel>
                "physical impairment center" .

v3-RoleCode:AUNT  a      owl:Class ;
        rdfs:label       "aunt" ;
        rdfs:subClassOf  v3-RoleCode:EXT ;
        <http://www.w3.org/2004/02/skos/core#definition>
                "The player of the role is a sister of the scoping person's mother or father." ;
        <http://www.w3.org/2004/02/skos/core#prefLabel>
                "aunt" .

v3-RoleCode:BF  a        owl:Class ;
        rdfs:label       "Beef" ;
        rdfs:subClassOf  v3-RoleCode:_LivingSubjectProductionClass ;
        <http://www.w3.org/2004/02/skos/core#definition>
                "Cattle used for meat production" ;
        <http://www.w3.org/2004/02/skos/core#prefLabel>
                "Beef" .

v3-RoleCode:CRP  a       owl:Class ;
        rdfs:label       "non-country member with residence permit" ;
        rdfs:subClassOf  v3-RoleCode:_CitizenRoleType ;
        <http://www.w3.org/2004/02/skos/core#definition>
                "A foreigner who is a resident of the country but does not have citizenship." ;
        <http://www.w3.org/2004/02/skos/core#prefLabel>
                "non-country member with residence permit" .

v3-RoleCode:MCOUSN  a    owl:Class ;
        rdfs:label       "maternal cousin" ;
        rdfs:subClassOf  v3-RoleCode:COUSN ;
        <http://www.w3.org/2004/02/skos/core#definition>
                "Description:The player of the role is a biological relative of the scoping person descended from a common ancestor on the player's mother's side, such as a grandparent, by two or more steps in a diverging line." ;
        <http://www.w3.org/2004/02/skos/core#prefLabel>
                "maternal cousin" .

v3-RoleCode:HUSB  a      owl:Class ;
        rdfs:label       "husband" ;
        rdfs:subClassOf  v3-RoleCode:SPS ;
        <http://www.w3.org/2004/02/skos/core#definition>
                "The player of the role is a man joined to a woman (scoping person) in marriage." ;
        <http://www.w3.org/2004/02/skos/core#prefLabel>
                "husband" .

v3-RoleCode:thirdParty
        a           owl:Class ;
        rdfs:label  "Third Party" ;
        <http://www.w3.org/2004/02/skos/core#definition>
                "Third Party" ;
        <http://www.w3.org/2004/02/skos/core#prefLabel>
                "Third Party" .

v3-RoleCode:PAYOR  a     owl:Class ;
        rdfs:label       "Payor Contact" ;
        rdfs:subClassOf  v3-RoleCode:_AdministrativeContactRoleType ;
        <http://www.w3.org/2004/02/skos/core#definition>
                "A contact role used to identify a person within a Payor organization to whom this communication is addressed." ;
        <http://www.w3.org/2004/02/skos/core#prefLabel>
                "Payor Contact" .

v3-RoleCode:PEDNEPH  a   owl:Class ;
        rdfs:label       "Pediatric nephrology clinic" ;
        rdfs:subClassOf  v3-RoleCode:NEPH ;
        <http://www.w3.org/2004/02/skos/core#definition>
                "Pediatric nephrology clinic" ;
        <http://www.w3.org/2004/02/skos/core#prefLabel>
                "Pediatric nephrology clinic" .

v3-RoleCode:PEDHO  a     owl:Class ;
        rdfs:label       "Pediatric oncology clinic" ;
        rdfs:subClassOf  v3-RoleCode:ONCL ;
        <http://www.w3.org/2004/02/skos/core#definition>
                "Pediatric oncology clinic" ;
        <http://www.w3.org/2004/02/skos/core#prefLabel>
                "Pediatric oncology clinic" .

v3-RoleCode:PHARM  a     owl:Class ;
        rdfs:label       "Pharmacy" ;
        rdfs:subClassOf  v3-RoleCode:_DedicatedNonClinicalLocationRoleType ;
        <http://www.w3.org/2004/02/skos/core#definition>
                "Location where healthcare service was delivered, identified as a pharmacy." ;
        <http://www.w3.org/2004/02/skos/core#prefLabel>
                "Pharmacy" .

v3-RoleCode:MGGRMTH  a   owl:Class ;
        rdfs:label       "maternal great-grandmother" ;
        rdfs:subClassOf  v3-RoleCode:GGRMTH ;
        <http://www.w3.org/2004/02/skos/core#definition>
                "Description:The player of the role is the biological mother of the scoping person's biological mother's parent." ;
        <http://www.w3.org/2004/02/skos/core#prefLabel>
                "maternal great-grandmother" .

v3-RoleCode:RHEUM  a     owl:Class ;
        rdfs:label       "Rheumatology clinic" ;
        rdfs:subClassOf  v3-RoleCode:OF ;
        <http://www.w3.org/2004/02/skos/core#definition>
                "Rheumatology clinic" ;
        <http://www.w3.org/2004/02/skos/core#prefLabel>
                "Rheumatology clinic" .

v3-RoleCode:PGRFTH  a    owl:Class ;
        rdfs:label       "paternal grandfather" ;
        rdfs:subClassOf  v3-RoleCode:GRFTH ;
        <http://www.w3.org/2004/02/skos/core#definition>
                "Description:The player of the role is the biological father of the scoping person's biological father." ;
        <http://www.w3.org/2004/02/skos/core#prefLabel>
                "paternal grandfather" .

v3-RoleCode:SU  a        owl:Class ;
        rdfs:label       "Surgery clinic" ;
        rdfs:subClassOf  v3-RoleCode:OF ;
        <http://www.w3.org/2004/02/skos/core#definition>
                "Surgery clinic" ;
        <http://www.w3.org/2004/02/skos/core#prefLabel>
                "Surgery clinic" .

v3-RoleCode:VET  a       owl:Class ;
        rdfs:label       "veteran" ;
        rdfs:subClassOf  v3-RoleCode:MIL ;
        <http://www.w3.org/2004/02/skos/core#definition>
                "Description: A person playing the role of program eligible under a program based on status as a military veteran.\r\n\n                        \n                           Discussion: This CoveredPartyRoleType.code is typically used when the CoveredPartyRole class code is either \"program eligible\" or \"subscriber\" and the persons status as a veteran meets jurisdictional or program criteria." ;
        <http://www.w3.org/2004/02/skos/core#prefLabel>
                "veteran" .

v3-RoleCode:RETMIL  a    owl:Class ;
        rdfs:label       "retired military" ;
        rdfs:subClassOf  v3-RoleCode:MIL ;
        <http://www.w3.org/2004/02/skos/core#definition>
                "Description: A person playing the role of program eligible under a program based on retired military status.\r\n\n                        \n                           Discussion: This CoveredPartyRoleType.code is typically used when the CoveredPartyRole class code is either \"program eligible\" or \"subscriber\" and the persons status as retired military meets jurisdictional or program criteria." ;
        <http://www.w3.org/2004/02/skos/core#prefLabel>
                "retired military" .

v3-RoleCode:_AssignedRoleType
        a           owl:Class ;
        rdfs:label  "AssignedRoleType" ;
        <http://www.w3.org/2004/02/skos/core#definition>
                "AssignedRoleType" ;
        <http://www.w3.org/2004/02/skos/core#prefLabel>
                "AssignedRoleType" .

v3-RoleCode:HUSCS  a     owl:Class ;
        rdfs:label       "specimen collection site" ;
        rdfs:subClassOf  v3-RoleCode:HU ;
        <http://www.w3.org/2004/02/skos/core#definition>
                "Description: A location that plays the role of delivering services which may include collecting specimens and/or samples from patients for laboratory testing purposes, but does not perform any tests or analysis functions." ;
        <http://www.w3.org/2004/02/skos/core#prefLabel>
                "specimen collection site" .

v3-RoleCode:FMC  a       owl:Class ;
        rdfs:label       "Family medicine clinic" ;
        rdfs:subClassOf  v3-RoleCode:OF ;
        <http://www.w3.org/2004/02/skos/core#definition>
                "Family medicine clinic" ;
        <http://www.w3.org/2004/02/skos/core#prefLabel>
                "Family medicine clinic" .

v3-RoleCode:WL  a        owl:Class ;
        rdfs:label       "Wool" ;
        rdfs:subClassOf  v3-RoleCode:_LivingSubjectProductionClass ;
        <http://www.w3.org/2004/02/skos/core#definition>
                "Sheep, goats and other mammals raised for their fiber" ;
        <http://www.w3.org/2004/02/skos/core#prefLabel>
                "Wool" .

v3-RoleCode:CANC  a      owl:Class ;
        rdfs:label       "Child and adolescent neurology clinic" ;
        rdfs:subClassOf  v3-RoleCode:OF ;
        <http://www.w3.org/2004/02/skos/core#definition>
                "Child and adolescent neurology clinic" ;
        <http://www.w3.org/2004/02/skos/core#prefLabel>
                "Child and adolescent neurology clinic" .

v3-RoleCode:ITWINBRO  a  owl:Class ;
        rdfs:label       "identical twin brother" ;
        rdfs:subClassOf  v3-RoleCode:TWINBRO ;
        <http://www.w3.org/2004/02/skos/core#definition>
                "The male scoper is an offspring of the same egg-sperm pair as the male player." ;
        <http://www.w3.org/2004/02/skos/core#prefLabel>
                "identical twin brother" .

v3-RoleCode:PLS  a       owl:Class ;
        rdfs:label       "Plastic surgery clinic" ;
        rdfs:subClassOf  v3-RoleCode:SU ;
        <http://www.w3.org/2004/02/skos/core#definition>
                "Plastic surgery clinic" ;
        <http://www.w3.org/2004/02/skos/core#prefLabel>
                "Plastic surgery clinic" .

v3-RoleCode:MU  a        owl:Class ;
        rdfs:label       "Multiplier" ;
        rdfs:subClassOf  v3-RoleCode:_LivingSubjectProductionClass ;
        <http://www.w3.org/2004/02/skos/core#definition>
                "Poultry flocks used for chick/poult production" ;
        <http://www.w3.org/2004/02/skos/core#prefLabel>
                "Multiplier" .

v3-RoleCode:MIL  a       owl:Class ;
        rdfs:label       "military" ;
        rdfs:subClassOf  v3-RoleCode:_ProgramEligiblePartyRoleType ;
        <http://www.w3.org/2004/02/skos/core#definition>
                "Definition: A person playing the role of program eligible under a program based on military status.\r\n\n                        \n                           Discussion:  This CoveredPartyRoleType.code is typically used when the CoveredPartyRole class code is either \"program eligible\" or \"subscriber\" and the person's status as a member of the military meets jurisdictional or program criteria" ;
        <http://www.w3.org/2004/02/skos/core#prefLabel>
                "military" .

v3-RoleCode:PGRMTH  a    owl:Class ;
        rdfs:label       "paternal grandmother" ;
        rdfs:subClassOf  v3-RoleCode:GRMTH ;
        <http://www.w3.org/2004/02/skos/core#definition>
                "Description:The player of the role is the biological mother of the scoping person's biological father." ;
        <http://www.w3.org/2004/02/skos/core#prefLabel>
                "paternal grandmother" .

v3-RoleCode:G  a         owl:Class ;
        rdfs:label       "Group" ;
        rdfs:subClassOf  v3-RoleCode:_SpecimenRoleType ;
        <http://www.w3.org/2004/02/skos/core#definition>
                "A set of patient samples in which the individuals of the group may or may not be identified." ;
        <http://www.w3.org/2004/02/skos/core#prefLabel>
                "Group" .

v3-RoleCode:TWINBRO  a   owl:Class ;
        rdfs:label       "twin brother" ;
        rdfs:subClassOf  v3-RoleCode:NBRO ;
        <http://www.w3.org/2004/02/skos/core#definition>
                "The scoper was carried in the same womb as the male player and shares common biological parents." ;
        <http://www.w3.org/2004/02/skos/core#prefLabel>
                "twin brother" .

v3-RoleCode:NFTH  a      owl:Class ;
        rdfs:label       "natural father" ;
        rdfs:subClassOf  v3-RoleCode:FTH ;
        <http://www.w3.org/2004/02/skos/core#definition>
                "The player of the role is a male who begets the scoping entity (child)." ;
        <http://www.w3.org/2004/02/skos/core#prefLabel>
                "natural father" .

v3-RoleCode:MTHINLAW  a  owl:Class ;
        rdfs:label       "mother-in-law" ;
        rdfs:subClassOf  v3-RoleCode:PRNINLAW ;
        <http://www.w3.org/2004/02/skos/core#definition>
                "The player of the role is the mother of the scoping person's husband or wife." ;
        <http://www.w3.org/2004/02/skos/core#prefLabel>
                "mother-in-law" .

v3-RoleCode:_AffiliationRoleType
        a           owl:Class ;
        rdfs:label  "AffiliationRoleType" ;
        <http://www.w3.org/2004/02/skos/core#definition>
                "Concepts characterizing the type of association formed by player and scoper when there is a recognized Affiliate role by which the two parties are related.\r\n\n                        \n                           Examples: Business Partner, Business Associate, Colleague" ;
        <http://www.w3.org/2004/02/skos/core#prefLabel>
                "AffiliationRoleType" .

v3-RoleCode:NCCS  a      owl:Class ;
        rdfs:label       "Neurology critical care and stroke unit" ;
        rdfs:subClassOf  v3-RoleCode:HU ;
        <http://www.w3.org/2004/02/skos/core#definition>
                "Neurology critical care and stroke unit" ;
        <http://www.w3.org/2004/02/skos/core#prefLabel>
                "Neurology critical care and stroke unit" .

v3-RoleCode:WORK  a      owl:Class ;
        rdfs:label       "work site" ;
        rdfs:subClassOf  v3-RoleCode:_IncidentalServiceDeliveryLocationRoleType ;
        <http://www.w3.org/2004/02/skos/core#definition>
                "Location where healthcare service was delivered, identified as a work place." ;
        <http://www.w3.org/2004/02/skos/core#prefLabel>
                "work site" .

v3-RoleCode:RHAT  a      owl:Class ;
        rdfs:label       "addiction treatment center" ;
        rdfs:subClassOf  v3-RoleCode:RH ;
        <http://www.w3.org/2004/02/skos/core#definition>
                "Description: A location that plays the role of delivering services which may include life training and/or social support to people with addictions." ;
        <http://www.w3.org/2004/02/skos/core#prefLabel>
                "addiction treatment center" .

v3-RoleCode:PRNINLAW  a  owl:Class ;
        rdfs:label       "parent in-law" ;
        rdfs:subClassOf  v3-RoleCode:INLAW ;
        <http://www.w3.org/2004/02/skos/core#definition>
                "The player of the role is the parent of scoping person's husband or wife." ;
        <http://www.w3.org/2004/02/skos/core#prefLabel>
                "parent in-law" .

v3-RoleCode:R  a         owl:Class ;
        rdfs:label       "Replicate" ;
        rdfs:subClassOf  v3-RoleCode:_SpecimenRoleType ;
        <http://www.w3.org/2004/02/skos/core#definition>
                "A portion of an original patent sample that is tested at the same time as the original sample" ;
        <http://www.w3.org/2004/02/skos/core#prefLabel>
                "Replicate" .

v3-RoleCode:phlebotomist
        a           owl:Class ;
        rdfs:label  "Phlebotomist" ;
        <http://www.w3.org/2004/02/skos/core#definition>
                "Phlebotomist" ;
        <http://www.w3.org/2004/02/skos/core#prefLabel>
                "Phlebotomist" .

v3-RoleCode:PEDNICU  a   owl:Class ;
        rdfs:label       "Pediatric neonatal intensive care unit" ;
        rdfs:subClassOf  v3-RoleCode:PEDICU ;
        <http://www.w3.org/2004/02/skos/core#definition>
                "Pediatric neonatal intensive care unit" ;
        <http://www.w3.org/2004/02/skos/core#prefLabel>
                "Pediatric neonatal intensive care unit" .

v3-RoleCode:PAINCL  a    owl:Class ;
        rdfs:label       "Pain clinic" ;
        rdfs:subClassOf  v3-RoleCode:OF ;
        <http://www.w3.org/2004/02/skos/core#definition>
                "(X12N 261QP3300N)" ;
        <http://www.w3.org/2004/02/skos/core#prefLabel>
                "Pain clinic" .

v3-RoleCode:PEDCARD  a   owl:Class ;
        rdfs:label       "Pediatric cardiology clinic" ;
        rdfs:subClassOf  v3-RoleCode:CARD ;
        <http://www.w3.org/2004/02/skos/core#definition>
                "Pediatric cardiology clinic" ;
        <http://www.w3.org/2004/02/skos/core#prefLabel>
                "Pediatric cardiology clinic" .

v3-RoleCode:INDIV  a  owl:Class ;
        rdfs:label  "individual" ;
        <http://www.w3.org/2004/02/skos/core#definition>
                "A party covered under a policy as the policyholder." ;
        <http://www.w3.org/2004/02/skos/core#prefLabel>
                "individual" .

v3-RoleCode:DU  a        owl:Class ;
        rdfs:label       "Dual" ;
        rdfs:subClassOf  v3-RoleCode:_LivingSubjectProductionClass ;
        <http://www.w3.org/2004/02/skos/core#definition>
                "Dual purpose.  Defined purposes based on species and breed" ;
        <http://www.w3.org/2004/02/skos/core#prefLabel>
                "Dual" .

v3-RoleCode:_DedicatedNonClinicalLocationRoleType
        a                owl:Class ;
        rdfs:label       "DedicatedNonClinicalLocationRoleType" ;
        rdfs:subClassOf  v3-RoleCode:_DedicatedServiceDeliveryLocationRoleType ;
        <http://www.w3.org/2004/02/skos/core#definition>
                "A role of a place that further classifies a setting that is intended to house the provision of non-clinical services." ;
        <http://www.w3.org/2004/02/skos/core#prefLabel>
                "DedicatedNonClinicalLocationRoleType" .

v3-RoleCode:SURF  a      owl:Class ;
        rdfs:label       "Substance use rehabilitation facility" ;
        rdfs:subClassOf  v3-RoleCode:RTF ;
        <http://www.w3.org/2004/02/skos/core#definition>
                "(X12N 324500000N)" ;
        <http://www.w3.org/2004/02/skos/core#prefLabel>
                "Substance use rehabilitation facility" .

v3-RoleCode:RC  a        owl:Class ;
        rdfs:label       "Racing" ;
        rdfs:subClassOf  v3-RoleCode:_LivingSubjectProductionClass ;
        <http://www.w3.org/2004/02/skos/core#definition>
                "Animals raised for racing perfomance" ;
        <http://www.w3.org/2004/02/skos/core#prefLabel>
                "Racing" .

v3-RoleCode:NMTH  a      owl:Class ;
        rdfs:label       "natural mother" ;
        rdfs:subClassOf  v3-RoleCode:MTH ;
        <http://www.w3.org/2004/02/skos/core#definition>
                "The player of the role is a female who conceives or gives birth to the scoping entity (child)." ;
        <http://www.w3.org/2004/02/skos/core#prefLabel>
                "natural mother" .

v3-RoleCode:PROG  a  owl:Class ;
        rdfs:label  "program eligible" ;
        <http://www.w3.org/2004/02/skos/core#definition>
                "A party that meets the eligibility criteria for coverage under a program." ;
        <http://www.w3.org/2004/02/skos/core#prefLabel>
                "program eligible" .

v3-RoleCode:SONFOST  a   owl:Class ;
        rdfs:label       "foster son" ;
        rdfs:subClassOf  v3-RoleCode:CHLDFOST ;
        <http://www.w3.org/2004/02/skos/core#definition>
                "The player of the role is a male child receiving parental care and nurture from the scoping person (parent) but not related to him or her through legal or blood ties." ;
        <http://www.w3.org/2004/02/skos/core#prefLabel>
                "foster son" .

v3-RoleCode:MAUNT  a     owl:Class ;
        rdfs:label       "maternal aunt" ;
        rdfs:subClassOf  v3-RoleCode:AUNT ;
        <http://www.w3.org/2004/02/skos/core#definition>
                "Description:The player of the role is a biological sister of the scoping person's biological mother." ;
        <http://www.w3.org/2004/02/skos/core#prefLabel>
                "maternal aunt" .

v3-RoleCode:ROOM  a      owl:Class ;
        rdfs:label       "Roommate" ;
        rdfs:subClassOf  v3-RoleCode:_PersonalRelationshipRoleType ;
        <http://www.w3.org/2004/02/skos/core#definition>
                "One who shares living quarters with the subject." ;
        <http://www.w3.org/2004/02/skos/core#prefLabel>
                "Roommate" .

v3-RoleCode:BMTC  a      owl:Class ;
        rdfs:label       "Bone marrow transplant clinic" ;
        rdfs:subClassOf  v3-RoleCode:OF ;
        <http://www.w3.org/2004/02/skos/core#definition>
                "Bone marrow transplant clinic" ;
        <http://www.w3.org/2004/02/skos/core#prefLabel>
                "Bone marrow transplant clinic" .

v3-RoleCode:MGRPRN  a    owl:Class ;
        rdfs:label       "maternal grandparent" ;
        rdfs:subClassOf  v3-RoleCode:GRPRN ;
        <http://www.w3.org/2004/02/skos/core#definition>
                "Description:The player of the role is the biological parent of the scoping person's biological mother." ;
        <http://www.w3.org/2004/02/skos/core#prefLabel>
                "maternal grandparent" .

v3-RoleCode:BL  a        owl:Class ;
        rdfs:label       "Broiler" ;
        rdfs:subClassOf  v3-RoleCode:_LivingSubjectProductionClass ;
        <http://www.w3.org/2004/02/skos/core#definition>
                "Chickens raised for meat" ;
        <http://www.w3.org/2004/02/skos/core#prefLabel>
                "Broiler" .

v3-RoleCode:PRC  a       owl:Class ;
        rdfs:label       "Pain rehabilitation center" ;
        rdfs:subClassOf  v3-RoleCode:RTF ;
        <http://www.w3.org/2004/02/skos/core#definition>
                "Pain rehabilitation center" ;
        <http://www.w3.org/2004/02/skos/core#prefLabel>
                "Pain rehabilitation center" .

v3-RoleCode:DADDR  a     owl:Class ;
        rdfs:label       "Delivery Address" ;
        rdfs:subClassOf  v3-RoleCode:_DedicatedNonClinicalLocationRoleType ;
        <http://www.w3.org/2004/02/skos/core#definition>
                "Location address where medical supplies were transported to for use." ;
        <http://www.w3.org/2004/02/skos/core#prefLabel>
                "Delivery Address" .

v3-RoleCode:PRN  a       owl:Class ;
        rdfs:label       "parent" ;
        rdfs:subClassOf  v3-RoleCode:FAMMEMB ;
        <http://www.w3.org/2004/02/skos/core#definition>
                "The player of the role is one who begets, gives birth to, or nurtures and raises the scoping entity (child)." ;
        <http://www.w3.org/2004/02/skos/core#prefLabel>
                "parent" .

v3-RoleCode:RADO  a      owl:Class ;
        rdfs:label       "Radiation oncology unit" ;
        rdfs:subClassOf  v3-RoleCode:RADDX ;
        <http://www.w3.org/2004/02/skos/core#definition>
                "(X12N 261QX0203N)" ;
        <http://www.w3.org/2004/02/skos/core#prefLabel>
                "Radiation oncology unit" .

v3-RoleCode:LY  a        owl:Class ;
        rdfs:label       "Layer" ;
        rdfs:subClassOf  v3-RoleCode:_LivingSubjectProductionClass ;
        <http://www.w3.org/2004/02/skos/core#definition>
                "Chickens raised for egg production" ;
        <http://www.w3.org/2004/02/skos/core#prefLabel>
                "Layer" .

v3-RoleCode:OPH  a       owl:Class ;
        rdfs:label       "Opthalmology clinic" ;
        rdfs:subClassOf  v3-RoleCode:OF ;
        <http://www.w3.org/2004/02/skos/core#definition>
                "Opthalmology clinic" ;
        <http://www.w3.org/2004/02/skos/core#prefLabel>
                "Opthalmology clinic" .

v3-RoleCode:HOSP  a      owl:Class ;
        rdfs:label       "Hospital" ;
        rdfs:subClassOf  v3-RoleCode:_DedicatedClinicalLocationRoleType ;
        <http://www.w3.org/2004/02/skos/core#definition>
                "An acute care institution that provides medical, surgical, or psychiatric care and treatment for the sick or the injured." ;
        <http://www.w3.org/2004/02/skos/core#prefLabel>
                "Hospital" .

v3-RoleCode:FTWIN  a     owl:Class ;
        rdfs:label       "fraternal twin" ;
        rdfs:subClassOf  v3-RoleCode:TWIN ;
        <http://www.w3.org/2004/02/skos/core#definition>
                "The scoper and player were carried in the same womb and share common biological parents but are the product of distinct egg/sperm pairs." ;
        <http://www.w3.org/2004/02/skos/core#prefLabel>
                "fraternal twin" .

v3-RoleCode:CHEST  a     owl:Class ;
        rdfs:label       "Chest unit" ;
        rdfs:subClassOf  v3-RoleCode:HU ;
        <http://www.w3.org/2004/02/skos/core#definition>
                "A specialty unit in hospital that focuses on chronic respirator patients and pulmonary failure" ;
        <http://www.w3.org/2004/02/skos/core#prefLabel>
                "Chest unit" .

v3-RoleCode:STUD  a      owl:Class ;
        rdfs:label       "student" ;
        rdfs:subClassOf  v3-RoleCode:_CoverageRoleType ;
        <http://www.w3.org/2004/02/skos/core#definition>
                "Covered party to an insurance policy has coverage through full-time or part-time attendance at a recognized educational institution as defined by a particular insurance policy." ;
        <http://www.w3.org/2004/02/skos/core#prefLabel>
                "student" .

v3-RoleCode:RTF  a       owl:Class ;
        rdfs:label       "Residential treatment facility" ;
        rdfs:subClassOf  v3-RoleCode:_DedicatedClinicalLocationRoleType ;
        <http://www.w3.org/2004/02/skos/core#definition>
                "Residential treatment facility" ;
        <http://www.w3.org/2004/02/skos/core#prefLabel>
                "Residential treatment facility" .

v3-RoleCode:CN  a        owl:Class ;
        rdfs:label       "national" ;
        rdfs:subClassOf  v3-RoleCode:_CitizenRoleType ;
        <http://www.w3.org/2004/02/skos/core#definition>
                "A person who is legally recognized as a member of a nation or country, with associated rights and obligations." ;
        <http://www.w3.org/2004/02/skos/core#prefLabel>
                "national" .

v3-RoleCode:NSIB  a      owl:Class ;
        rdfs:label       "natural sibling" ;
        rdfs:subClassOf  v3-RoleCode:SIB ;
        <http://www.w3.org/2004/02/skos/core#definition>
                "The player of the role has both biological parents in common with the scoping entity." ;
        <http://www.w3.org/2004/02/skos/core#prefLabel>
                "natural sibling" .

v3-RoleCode:OMS  a       owl:Class ;
        rdfs:label       "Oral and maxillofacial surgery clinic" ;
        rdfs:subClassOf  v3-RoleCode:OF ;
        <http://www.w3.org/2004/02/skos/core#definition>
                "Oral and maxillofacial surgery clinic" ;
        <http://www.w3.org/2004/02/skos/core#prefLabel>
                "Oral and maxillofacial surgery clinic" .

v3-RoleCode:LOCHFID  a   owl:Class ;
        rdfs:label       "local location identifier" ;
        rdfs:subClassOf  v3-RoleCode:_LocationIdentifiedEntityRoleCode ;
        <http://www.w3.org/2004/02/skos/core#definition>
                "Description:Identifier assigned to a  location by a local party (which could be the facility itself or organization overseeing a group of facilities)." ;
        <http://www.w3.org/2004/02/skos/core#prefLabel>
                "local location identifier" .

v3-RoleCode:BILL  a      owl:Class ;
        rdfs:label       "Billing Contact" ;
        rdfs:subClassOf  v3-RoleCode:_AdministrativeContactRoleType ;
        <http://www.w3.org/2004/02/skos/core#definition>
                "A contact role used to identify a person within a Provider organization that can be contacted for billing purposes (e.g. about the content of the Invoice)." ;
        <http://www.w3.org/2004/02/skos/core#prefLabel>
                "Billing Contact" .

v3-RoleCode:B  a         owl:Class ;
        rdfs:label       "Blind" ;
        rdfs:subClassOf  v3-RoleCode:Q ;
        <http://www.w3.org/2004/02/skos/core#definition>
                "Quality Control specimen submitted to the lab whose identity and composition is not known to the lab." ;
        <http://www.w3.org/2004/02/skos/core#prefLabel>
                "Blind" .

v3-RoleCode:ADOPT  a     owl:Class ;
        rdfs:label       "adopted child" ;
        rdfs:subClassOf  v3-RoleCode:_CoverageRoleType ;
        <http://www.w3.org/2004/02/skos/core#definition>
                "A child taken into one's family through legal means and raised as one's own child." ;
        <http://www.w3.org/2004/02/skos/core#prefLabel>
                "adopted child" .

v3-RoleCode:ALL  a       owl:Class ;
        rdfs:label       "Allergy clinic" ;
        rdfs:subClassOf  v3-RoleCode:OF ;
        <http://www.w3.org/2004/02/skos/core#definition>
                "Allergy clinic" ;
        <http://www.w3.org/2004/02/skos/core#prefLabel>
                "Allergy clinic" .

v3-RoleCode:TR  a        owl:Class ;
        rdfs:label       "Transplant clinic" ;
        rdfs:subClassOf  v3-RoleCode:OF ;
        <http://www.w3.org/2004/02/skos/core#definition>
                "Transplant clinic" ;
        <http://www.w3.org/2004/02/skos/core#prefLabel>
                "Transplant clinic" .

v3-RoleCode:GDSF  a      owl:Class ;
        rdfs:label       "generic drug strength form" ;
        rdfs:subClassOf  v3-RoleCode:GD ;
        <http://www.w3.org/2004/02/skos/core#definition>
                "Relates a manufactured drug product to the non-proprietary (generic) representation of its ingredients with their strength in a specific dose form. The scoping entity identifies a unique combination of medicine ingredients with their strength in a single dose form." ;
        <http://www.w3.org/2004/02/skos/core#prefLabel>
                "generic drug strength form" .

v3-RoleCode:COPART  a    owl:Class ;
        rdfs:label       "co-participant" ;
        rdfs:subClassOf  v3-RoleCode:_AgentRoleType ;
        <http://www.w3.org/2004/02/skos/core#definition>
                "An entity which participates in the generation of and attest to veracity of content, but is not an author or coauthor. For example a surgeon who is required by institutional, regulatory, or legal rules to sign an operative report, but who was not involved in the authorship of that report." ;
        <http://www.w3.org/2004/02/skos/core#prefLabel>
                "co-participant" .

v3-RoleCode:INJWKR  a    owl:Class ;
        rdfs:label       "injured worker" ;
        rdfs:subClassOf  v3-RoleCode:_ClaimantCoveredPartyRoleType ;
        <http://www.w3.org/2004/02/skos/core#definition>
                "Description: A person playing the role of program eligible under a workers compensation program based on the filing of work-related injury claim.\r\n\n                        \n                           Discussion:  This CoveredPartyRoleType.code is used when the CoveredPartyRole class code is either \"program eligible\", a \"named insured\", and \"individual insured\",  or \"dependent\", and the person's status as differently abled or \"handicapped\" meets jurisdictional, policy, or program criteria." ;
        <http://www.w3.org/2004/02/skos/core#prefLabel>
                "injured worker" .

v3-RoleCode:subject  a  owl:Class ;
        rdfs:label  "Self" ;
        <http://www.w3.org/2004/02/skos/core#definition>
                "Self" ;
        <http://www.w3.org/2004/02/skos/core#prefLabel>
                "Self" .

v3-RoleCode:URO  a       owl:Class ;
        rdfs:label       "Urology clinic" ;
        rdfs:subClassOf  v3-RoleCode:SU ;
        <http://www.w3.org/2004/02/skos/core#definition>
                "Urology clinic" ;
        <http://www.w3.org/2004/02/skos/core#prefLabel>
                "Urology clinic" .

v3-RoleCode:PUNCLE  a    owl:Class ;
        rdfs:label       "paternal uncle" ;
        rdfs:subClassOf  v3-RoleCode:UNCLE ;
        <http://www.w3.org/2004/02/skos/core#definition>
                "Description:The player of the role is a biological brother of the scoping person's biological father." ;
        <http://www.w3.org/2004/02/skos/core#prefLabel>
                "paternal uncle" .

v3-RoleCode:GACH  a      owl:Class ;
        rdfs:label       "Hospitals; General Acute Care Hospital" ;
        rdfs:subClassOf  v3-RoleCode:HOSP ;
        <http://www.w3.org/2004/02/skos/core#definition>
                "(X12N 282N00000N)" ;
        <http://www.w3.org/2004/02/skos/core#prefLabel>
                "Hospitals; General Acute Care Hospital" .

v3-RoleCode:DEBR  a      owl:Class ;
        rdfs:label       "Debridement" ;
        rdfs:subClassOf  v3-RoleCode:BIOTH ;
        <http://www.w3.org/2004/02/skos/core#definition>
                "Description:Maggots raised for biodebridement.\r\n\n                        \n                           Discussion: Maggot Debridement Therapy is the medical use of live maggots for cleaning non-healing wounds.\r\n\n                        \n                           Examples:Removal of burnt skin." ;
        <http://www.w3.org/2004/02/skos/core#prefLabel>
                "Debridement" .

v3-RoleCode:CLAIM  a  owl:Class ;
        rdfs:label  "claimant" ;
        <http://www.w3.org/2004/02/skos/core#definition>
                "A party that makes a claim for coverage under a policy." ;
        <http://www.w3.org/2004/02/skos/core#prefLabel>
                "claimant" .

v3-RoleCode:MHSP  a      owl:Class ;
        rdfs:label       "Military Hospital" ;
        rdfs:subClassOf  v3-RoleCode:HOSP ;
        <http://www.w3.org/2004/02/skos/core#definition>
                "A health care facility operated by the Department of Defense or other military operation." ;
        <http://www.w3.org/2004/02/skos/core#prefLabel>
                "Military Hospital" .

v3-RoleCode:CASM  a      owl:Class ;
        rdfs:label       "single minor asylum seeker" ;
        rdfs:subClassOf  v3-RoleCode:CAS ;
        <http://www.w3.org/2004/02/skos/core#definition>
                "A person who is someone of below legal age who has fled his or her home country, without his or her parents, to find a safe place elsewhere at time of categorization." ;
        <http://www.w3.org/2004/02/skos/core#prefLabel>
                "single minor asylum seeker" .

v3-RoleCode:GDF  a       owl:Class ;
        rdfs:label       "generic drug form" ;
        rdfs:subClassOf  v3-RoleCode:GD ;
        <http://www.w3.org/2004/02/skos/core#definition>
                "Relates a manufactured drug product to the non-proprietary (generic) representation of its ingredients and dose form, independent of strength of the ingredients. The scoping entity identifies a unique combination of medicine ingredients in a specific dose form." ;
        <http://www.w3.org/2004/02/skos/core#prefLabel>
                "generic drug form" .

v3-RoleCode:COAG  a      owl:Class ;
        rdfs:label       "Coagulation clinic" ;
        rdfs:subClassOf  v3-RoleCode:OF ;
        <http://www.w3.org/2004/02/skos/core#definition>
                "Coagulation clinic" ;
        <http://www.w3.org/2004/02/skos/core#prefLabel>
                "Coagulation clinic" .

v3-RoleCode:ER  a        owl:Class ;
        rdfs:label       "Emergency room" ;
        rdfs:subClassOf  v3-RoleCode:HU ;
        <http://www.w3.org/2004/02/skos/core#definition>
                "The section of a health care facility for providing rapid treatment to victims of sudden illness or trauma." ;
        <http://www.w3.org/2004/02/skos/core#prefLabel>
                "Emergency room" .

v3-RoleCode:SONINLAW  a  owl:Class ;
        rdfs:label       "son in-law" ;
        rdfs:subClassOf  v3-RoleCode:CHLDINLAW ;
        <http://www.w3.org/2004/02/skos/core#definition>
                "The player of the role is the husband of scoping person's daughter." ;
        <http://www.w3.org/2004/02/skos/core#prefLabel>
                "son in-law" .

v3-RoleCode:PREV  a      owl:Class ;
        rdfs:label       "Preventive medicine clinic" ;
        rdfs:subClassOf  v3-RoleCode:OF ;
        <http://www.w3.org/2004/02/skos/core#definition>
                "Preventive medicine clinic" ;
        <http://www.w3.org/2004/02/skos/core#prefLabel>
                "Preventive medicine clinic" .

v3-RoleCode:DOWNGRDER
        a                owl:Class ;
        rdfs:label       "downgrader" ;
        rdfs:subClassOf  v3-RoleCode:_AgentRoleType ;
        <http://www.w3.org/2004/02/skos/core#definition>
                "An individual authorized to lower the classification level of labeled content and provide rationale for doing so as directed by a classification guide." ;
        <http://www.w3.org/2004/02/skos/core#prefLabel>
                "downgrader" .

v3-RoleCode:MOBL  a      owl:Class ;
        rdfs:label       "Mobile Unit" ;
        rdfs:subClassOf  v3-RoleCode:_DedicatedNonClinicalLocationRoleType ;
        <http://www.w3.org/2004/02/skos/core#definition>
                "Location (mobile) where healthcare service was delivered." ;
        <http://www.w3.org/2004/02/skos/core#prefLabel>
                "Mobile Unit" .

v3-RoleCode:BR  a        owl:Class ;
        rdfs:label       "Breeder" ;
        rdfs:subClassOf  v3-RoleCode:_LivingSubjectProductionClass ;
        <http://www.w3.org/2004/02/skos/core#definition>
                "Breeding/genetic stock" ;
        <http://www.w3.org/2004/02/skos/core#prefLabel>
                "Breeder" .

v3-RoleCode:COUSN  a     owl:Class ;
        rdfs:label       "cousin" ;
        rdfs:subClassOf  v3-RoleCode:EXT ;
        <http://www.w3.org/2004/02/skos/core#definition>
                "The player of the role is a relative of the scoping person descended from a common ancestor, such as a \tgrandparent, by two or more steps in a diverging line." ;
        <http://www.w3.org/2004/02/skos/core#prefLabel>
                "cousin" .

v3-RoleCode:ADOPTM  a    owl:Class ;
        rdfs:label       "adoptive mother" ;
        rdfs:subClassOf  v3-RoleCode:ADOPTP ;
        <http://www.w3.org/2004/02/skos/core#definition>
                "The player of the role (father) is a female who has taken the scoper (child) into their family through legal means and raises them as her own child." ;
        <http://www.w3.org/2004/02/skos/core#prefLabel>
                "adoptive mother" .

v3-RoleCode:RADDX  a     owl:Class ;
        rdfs:label       "Radiology diagnostics or therapeutics unit" ;
        rdfs:subClassOf  v3-RoleCode:DX ;
        <http://www.w3.org/2004/02/skos/core#definition>
                "A practice setting where radiology services (diagnostic or therapeutic) are provided            (X12N 261QR0200N)" ;
        <http://www.w3.org/2004/02/skos/core#prefLabel>
                "Radiology diagnostics or therapeutics unit" .

v3-RoleCode:NAMED  a  owl:Class ;
        rdfs:label  "named insured" ;
        <http://www.w3.org/2004/02/skos/core#definition>
                "A party to an insurance policy to whom the insurer agrees to indemnify for losses, provides benefits for, or renders services." ;
        <http://www.w3.org/2004/02/skos/core#prefLabel>
                "named insured" .

v3-RoleCode:FI  a        owl:Class ;
        rdfs:label       "Fiber" ;
        rdfs:subClassOf  v3-RoleCode:_LivingSubjectProductionClass ;
        <http://www.w3.org/2004/02/skos/core#definition>
                "Animals raised for their fur, hair or skins" ;
        <http://www.w3.org/2004/02/skos/core#prefLabel>
                "Fiber" .

v3-RoleCode:DAU  a       owl:Class ;
        rdfs:label       "natural daughter" ;
        rdfs:subClassOf  v3-RoleCode:DAUC ;
        <http://www.w3.org/2004/02/skos/core#definition>
                "The player of the role is a female offspring of the scoping entity (parent)." ;
        <http://www.w3.org/2004/02/skos/core#prefLabel>
                "natural daughter" .

v3-RoleCode:TRB  a       owl:Class ;
        rdfs:label       "Tribal Member" ;
        rdfs:subClassOf  v3-RoleCode:_MemberRoleType ;
        <http://www.w3.org/2004/02/skos/core#definition>
                "A person who is a member of a tribe." ;
        <http://www.w3.org/2004/02/skos/core#prefLabel>
                "Tribal Member" .

v3-RoleCode:PGGRFTH  a   owl:Class ;
        rdfs:label       "paternal great-grandfather" ;
        rdfs:subClassOf  v3-RoleCode:GGRFTH ;
        <http://www.w3.org/2004/02/skos/core#definition>
                "Description:The player of the role is the biological father of the scoping person's biological father's parent." ;
        <http://www.w3.org/2004/02/skos/core#prefLabel>
                "paternal great-grandfather" .

v3-RoleCode:HSIB  a      owl:Class ;
        rdfs:label       "half-sibling" ;
        rdfs:subClassOf  v3-RoleCode:SIB ;
        <http://www.w3.org/2004/02/skos/core#definition>
                "The player of the role is related to the scoping entity by sharing only one biological parent." ;
        <http://www.w3.org/2004/02/skos/core#prefLabel>
                "half-sibling" .

v3-RoleCode:STPFTH  a    owl:Class ;
        rdfs:label       "stepfather" ;
        rdfs:subClassOf  v3-RoleCode:FTH ;
        <http://www.w3.org/2004/02/skos/core#definition>
                "The player of the role is the husband of scoping person's mother and not the scoping person's natural father." ;
        <http://www.w3.org/2004/02/skos/core#prefLabel>
                "stepfather" .

v3-RoleCode:ACTMIL  a    owl:Class ;
        rdfs:label       "active duty military" ;
        rdfs:subClassOf  v3-RoleCode:MIL ;
        <http://www.w3.org/2004/02/skos/core#definition>
                "Description: A person playing the role of program eligible under a program based on active military status.\r\n\n                        \n                           Discussion: This CoveredPartyRoleType.code is typically used when the CoveredPartyRole class code is either \"program eligible\" or \"subscriber\" and the persons status as active duty military meets jurisdictional or program criteria." ;
        <http://www.w3.org/2004/02/skos/core#prefLabel>
                "active duty military" .

v3-RoleCode:ENT  a       owl:Class ;
        rdfs:label       "Otorhinolaryngology clinic" ;
        rdfs:subClassOf  v3-RoleCode:OF ;
        <http://www.w3.org/2004/02/skos/core#definition>
                "Otorhinolaryngology clinic" ;
        <http://www.w3.org/2004/02/skos/core#prefLabel>
                "Otorhinolaryngology clinic" .

v3-RoleCode:PSYCHF  a    owl:Class ;
        rdfs:label       "Psychatric Care Facility" ;
        rdfs:subClassOf  v3-RoleCode:HOSP ;
        <http://www.w3.org/2004/02/skos/core#definition>
                "Healthcare facility that cares for patients with psychiatric illness(s)." ;
        <http://www.w3.org/2004/02/skos/core#prefLabel>
                "Psychatric Care Facility" .

v3-RoleCode:HANDIC  a    owl:Class ;
        rdfs:label       "handicapped dependent" ;
        rdfs:subClassOf  v3-RoleCode:_CoverageRoleType ;
        <http://www.w3.org/2004/02/skos/core#definition>
                "Covered party is a dependent of the policy holder with a physical or mental disability causing a disadvantage that makes independent achievement unusually difficult." ;
        <http://www.w3.org/2004/02/skos/core#prefLabel>
                "handicapped dependent" .

v3-RoleCode:NSIS  a      owl:Class ;
        rdfs:label       "natural sister" ;
        rdfs:subClassOf  v3-RoleCode:NSIB ;
        <http://www.w3.org/2004/02/skos/core#definition>
                "The player of the role is a female having the same biological parents as the scoping entity." ;
        <http://www.w3.org/2004/02/skos/core#prefLabel>
                "natural sister" .

v3-RoleCode:ORTHO  a     owl:Class ;
        rdfs:label       "Orthopedics clinic" ;
        rdfs:subClassOf  v3-RoleCode:OF ;
        <http://www.w3.org/2004/02/skos/core#definition>
                "Orthopedics clinic" ;
        <http://www.w3.org/2004/02/skos/core#prefLabel>
                "Orthopedics clinic" .

v3-RoleCode:PGGRMTH  a   owl:Class ;
        rdfs:label       "paternal great-grandmother" ;
        rdfs:subClassOf  v3-RoleCode:GGRMTH ;
        <http://www.w3.org/2004/02/skos/core#definition>
                "Description:The player of the role is the biological mother of the scoping person's biological father's parent." ;
        <http://www.w3.org/2004/02/skos/core#prefLabel>
                "paternal great-grandmother" .

v3-RoleCode:STPMTH  a    owl:Class ;
        rdfs:label       "stepmother" ;
        rdfs:subClassOf  v3-RoleCode:MTH ;
        <http://www.w3.org/2004/02/skos/core#definition>
                "The player of the role is the wife of scoping person's father and not the scoping person's natural mother." ;
        <http://www.w3.org/2004/02/skos/core#prefLabel>
                "stepmother" .

v3-RoleCode:BRO  a       owl:Class ;
        rdfs:label       "brother" ;
        rdfs:subClassOf  v3-RoleCode:SIB ;
        <http://www.w3.org/2004/02/skos/core#definition>
                "The player of the role is a male sharing one or both parents in common with the scoping entity." ;
        <http://www.w3.org/2004/02/skos/core#prefLabel>
                "brother" .

v3-RoleCode:COMM  a      owl:Class ;
        rdfs:label       "Community Location" ;
        rdfs:subClassOf  v3-RoleCode:_IncidentalServiceDeliveryLocationRoleType ;
        <http://www.w3.org/2004/02/skos/core#definition>
                "Community location where healthcare is delivered." ;
        <http://www.w3.org/2004/02/skos/core#prefLabel>
                "Community Location" .

v3-RoleCode:PROFF  a     owl:Class ;
        rdfs:label       "Provider's Office" ;
        rdfs:subClassOf  v3-RoleCode:OF ;
        <http://www.w3.org/2004/02/skos/core#definition>
                "Location where healthcare service was delivered, identified as the healthcare provider's practice office." ;
        <http://www.w3.org/2004/02/skos/core#prefLabel>
                "Provider's Office" .

v3-RoleCode:NIECE  a     owl:Class ;
        rdfs:label       "niece" ;
        rdfs:subClassOf  v3-RoleCode:NIENEPH ;
        <http://www.w3.org/2004/02/skos/core#definition>
                "The player of the role is a daughter of the scoping person's brother or sister or of the brother or sister of the \tscoping person's spouse." ;
        <http://www.w3.org/2004/02/skos/core#prefLabel>
                "niece" .

v3-RoleCode:ORG  a       owl:Class ;
        rdfs:label       "organizational contact" ;
        rdfs:subClassOf  v3-RoleCode:_AdministrativeContactRoleType ;
        <http://www.w3.org/2004/02/skos/core#definition>
                "A contact for an organization for administrative purposes. Contact role specifies a person acting as a liason for the organization.\r\n\n                        Example: HR Department representative." ;
        <http://www.w3.org/2004/02/skos/core#prefLabel>
                "organizational contact" .

v3-RoleCode:PEDGI  a     owl:Class ;
        rdfs:label       "Pediatric gastroenterology clinic" ;
        rdfs:subClassOf  v3-RoleCode:GI ;
        <http://www.w3.org/2004/02/skos/core#definition>
                "Pediatric gastroenterology clinic" ;
        <http://www.w3.org/2004/02/skos/core#prefLabel>
                "Pediatric gastroenterology clinic" .

v3-RoleCode:NBOR  a      owl:Class ;
        rdfs:label       "neighbor" ;
        rdfs:subClassOf  v3-RoleCode:_PersonalRelationshipRoleType ;
        <http://www.w3.org/2004/02/skos/core#definition>
                "The player of the role lives near or next to the \tscoping person." ;
        <http://www.w3.org/2004/02/skos/core#prefLabel>
                "neighbor" .

v3-RoleCode:CLASSIFIER
        a                owl:Class ;
        rdfs:label       "classifier" ;
        rdfs:subClassOf  v3-RoleCode:_AgentRoleType ;
        <http://www.w3.org/2004/02/skos/core#definition>
                "An individual authorized to assign an original classification to information, including compilations of unclassified information, based on a determination that the information requires protection against unauthorized disclosure. The individual marks the information with immutable, computable, and human readable security labels in accordance with applicable security labeling policies.  The labeling policies provide instructions on whether and if so how the security labels may be later reclassified [i.e., upgraded, downgraded, used in derivative classification, or declassified] in a manner that preserves the overridden original classification binding and provenance." ;
        <http://www.w3.org/2004/02/skos/core#prefLabel>
                "classifier" .

v3-RoleCode:CAS  a       owl:Class ;
        rdfs:label       "asylum seeker" ;
        rdfs:subClassOf  v3-RoleCode:_CitizenRoleType ;
        <http://www.w3.org/2004/02/skos/core#definition>
                "A person who has fled his or her home country to find a safe place elsewhere." ;
        <http://www.w3.org/2004/02/skos/core#prefLabel>
                "asylum seeker" .

v3-RoleCode:pathologist
        a           owl:Class ;
        rdfs:label  "Pathologist" ;
        <http://www.w3.org/2004/02/skos/core#definition>
                "Pathologist" ;
        <http://www.w3.org/2004/02/skos/core#prefLabel>
                "Pathologist" .

v3-RoleCode:SIGOTHR  a   owl:Class ;
        rdfs:label       "significant other" ;
        rdfs:subClassOf  v3-RoleCode:FAMMEMB ;
        <http://www.w3.org/2004/02/skos/core#definition>
                "A person who is important to one's well being; especially a spouse or one in a similar relationship.  (The player is the one who is important)" ;
        <http://www.w3.org/2004/02/skos/core#prefLabel>
                "significant other" .

v3-RoleCode:TRAVEL  a    owl:Class ;
        rdfs:label       "Travel and geographic medicine clinic" ;
        rdfs:subClassOf  v3-RoleCode:OF ;
        <http://www.w3.org/2004/02/skos/core#definition>
                "Travel and geographic medicine clinic" ;
        <http://www.w3.org/2004/02/skos/core#prefLabel>
                "Travel and geographic medicine clinic" .

v3-RoleCode:GESTM  a     owl:Class ;
        rdfs:label       "gestational mother" ;
        rdfs:subClassOf  v3-RoleCode:MTH ;
        <http://www.w3.org/2004/02/skos/core#definition>
                "The player is a female whose womb carries the fetus of the scoper.  Generally used when the gestational mother and natural mother are not the same." ;
        <http://www.w3.org/2004/02/skos/core#prefLabel>
                "gestational mother" .

v3-RoleCode:PROS  a      owl:Class ;
        rdfs:label       "Prosthodontics clinic" ;
        rdfs:subClassOf  v3-RoleCode:OF ;
        <http://www.w3.org/2004/02/skos/core#definition>
                "Prosthodontics clinic" ;
        <http://www.w3.org/2004/02/skos/core#prefLabel>
                "Prosthodontics clinic" .

v3-RoleCode:ECHO  a      owl:Class ;
        rdfs:label       "Echocardiography lab" ;
        rdfs:subClassOf  v3-RoleCode:CVDX ;
        <http://www.w3.org/2004/02/skos/core#definition>
                "Echocardiography lab" ;
        <http://www.w3.org/2004/02/skos/core#prefLabel>
                "Echocardiography lab" .

v3-RoleCode:GRPRN  a     owl:Class ;
        rdfs:label       "grandparent" ;
        rdfs:subClassOf  v3-RoleCode:EXT ;
        <http://www.w3.org/2004/02/skos/core#definition>
                "The player of the role is a parent of the scoping person's mother or father." ;
        <http://www.w3.org/2004/02/skos/core#prefLabel>
                "grandparent" .

v3-RoleCode:CSC  a       owl:Class ;
        rdfs:label       "community service center" ;
        rdfs:subClassOf  v3-RoleCode:COMM ;
        <http://www.w3.org/2004/02/skos/core#definition>
                "Description: A location that plays the role of delivering services which may include providing front-line services to the population of a defined geographic area such as: healthcare services and social services, preventive or curative, rehabilitation or reintegration." ;
        <http://www.w3.org/2004/02/skos/core#prefLabel>
                "community service center" .

v3-RoleCode:POD  a       owl:Class ;
        rdfs:label       "Podiatry clinic" ;
        rdfs:subClassOf  v3-RoleCode:OF ;
        <http://www.w3.org/2004/02/skos/core#definition>
                "(X12N 261QP1100N)" ;
        <http://www.w3.org/2004/02/skos/core#prefLabel>
                "Podiatry clinic" .

v3-RoleCode:GUARD  a     owl:Class ;
        rdfs:label       "guardian" ;
        rdfs:subClassOf  v3-RoleCode:RESPRSN ;
        <http://www.w3.org/2004/02/skos/core#definition>
                "The role played by a person or institution legally empowered with responsibility for the care of a ward." ;
        <http://www.w3.org/2004/02/skos/core#prefLabel>
                "guardian" .

v3-RoleCode:STPSIB  a    owl:Class ;
        rdfs:label       "step sibling" ;
        rdfs:subClassOf  v3-RoleCode:SIB ;
        <http://www.w3.org/2004/02/skos/core#definition>
                "The player of the role is a child of the scoping person's stepparent." ;
        <http://www.w3.org/2004/02/skos/core#prefLabel>
                "step sibling" .

v3-RoleCode:_AssignedNonPersonLivingSubjectRoleType
        a                owl:Class ;
        rdfs:label       "AssignedNonPersonLivingSubjectRoleType" ;
        rdfs:subClassOf  v3-RoleCode:_AssignedRoleType ;
        <http://www.w3.org/2004/02/skos/core#definition>
                "Description:A role type that is used to further qualify a non-person subject playing a role where the role class attribute is set to RoleClass AssignedEntity" ;
        <http://www.w3.org/2004/02/skos/core#prefLabel>
                "AssignedNonPersonLivingSubjectRoleType" .

v3-RoleCode:RESPRSN  a   owl:Class ;
        rdfs:label       "responsible party" ;
        rdfs:subClassOf  v3-RoleCode:_AffiliationRoleType ;
        <http://www.w3.org/2004/02/skos/core#definition>
                "The role played by a party who has legal responsibility for another party." ;
        <http://www.w3.org/2004/02/skos/core#prefLabel>
                "responsible party" .

v3-RoleCode:REVIEWER  a  owl:Class ;
        rdfs:label       "reviewer" ;
        rdfs:subClassOf  v3-RoleCode:_AgentRoleType ;
        <http://www.w3.org/2004/02/skos/core#definition>
                "An entity authorized to filter information according to approved criteria." ;
        <http://www.w3.org/2004/02/skos/core#prefLabel>
                "reviewer" .

v3-RoleCode:DRIVCLASSIFIER
        a                owl:Class ;
        rdfs:label       "derivative classifier" ;
        rdfs:subClassOf  v3-RoleCode:_AgentRoleType ;
        <http://www.w3.org/2004/02/skos/core#definition>
                "An individual who is only authorized to classify reproduced, extracted, or summarized classified information, or compile classified and unclassified information by applying classification markings derived from source material or as directed by a classification guide." ;
        <http://www.w3.org/2004/02/skos/core#prefLabel>
                "derivative classifier" .

v3-RoleCode:CVDX  a      owl:Class ;
        rdfs:label       "Cardiovascular diagnostics or therapeutics unit" ;
        rdfs:subClassOf  v3-RoleCode:DX ;
        <http://www.w3.org/2004/02/skos/core#definition>
                "A practice setting where cardiovascular diagnostic procedures or therapeutic interventions are performed (e.g., cardiac catheterization lab, echocardiography suite)" ;
        <http://www.w3.org/2004/02/skos/core#prefLabel>
                "Cardiovascular diagnostics or therapeutics unit" .

v3-RoleCode:PRNFOST  a   owl:Class ;
        rdfs:label       "foster parent" ;
        rdfs:subClassOf  v3-RoleCode:PRN ;
        <http://www.w3.org/2004/02/skos/core#definition>
                "The player of the role (parent) who is a state-certified caregiver responsible for the scoper (child) who has been placed in the parent's care. The placement of the child is usually arranged through the government or a social-service agency, and temporary.\r\n\n                        The state, via a jurisdiction recognized child protection agency, stands as in loco parentis to the child, making all legal decisions while the foster parent is responsible for the day-to-day care of the specified child." ;
        <http://www.w3.org/2004/02/skos/core#prefLabel>
                "foster parent" .

v3-RoleCode:CO  a        owl:Class ;
        rdfs:label       "Companion" ;
        rdfs:subClassOf  v3-RoleCode:_LivingSubjectProductionClass ;
        <http://www.w3.org/2004/02/skos/core#definition>
                "Companion animals" ;
        <http://www.w3.org/2004/02/skos/core#prefLabel>
                "Companion" .

v3-RoleCode:C  a         owl:Class ;
        rdfs:label       "Calibrator" ;
        rdfs:subClassOf  v3-RoleCode:_SpecimenRoleType ;
        <http://www.w3.org/2004/02/skos/core#definition>
                "A specimen used for initial calibration settings of an instrument" ;
        <http://www.w3.org/2004/02/skos/core#prefLabel>
                "Calibrator" .

v3-RoleCode:PTRES  a     owl:Class ;
        rdfs:label       "Patient's Residence" ;
        rdfs:subClassOf  v3-RoleCode:_IncidentalServiceDeliveryLocationRoleType ;
        <http://www.w3.org/2004/02/skos/core#definition>
                "location where healthcare was delivered which is the residence of the Patient." ;
        <http://www.w3.org/2004/02/skos/core#prefLabel>
                "Patient's Residence" .
