@prefix fhir:  <http://hl7.org/fhir/> .
@prefix rdf:   <http://www.w3.org/1999/02/22-rdf-syntax-ns#> .
@prefix owl:   <http://www.w3.org/2002/07/owl#> .
@prefix v3-orderableDrugForm: <http://hl7.org/fhir/v3/orderableDrugForm/> .
@prefix xsd:   <http://www.w3.org/2001/XMLSchema#> .
@prefix rdfs:  <http://www.w3.org/2000/01/rdf-schema#> .
@prefix w5:    <http://hl7.org/fhir/w5#> .

v3-orderableDrugForm:AER
        a                owl:Class ;
        rdfs:label       "Aerosol" ;
        rdfs:subClassOf  v3-orderableDrugForm:_GasLiquidMixture ;
        <http://www.w3.org/2004/02/skos/core#definition>
                "Aerosol" ;
        <http://www.w3.org/2004/02/skos/core#prefLabel>
                "Aerosol" .

v3-orderableDrugForm:TPATHWK
        a                owl:Class ;
        rdfs:label       "Weekly Transdermal Patch" ;
        rdfs:subClassOf  v3-orderableDrugForm:TPATCH ;
        <http://www.w3.org/2004/02/skos/core#definition>
                "Weekly Transdermal Patch" ;
        <http://www.w3.org/2004/02/skos/core#prefLabel>
                "Weekly Transdermal Patch" .

v3-orderableDrugForm:_SolidDrugForm
        a                owl:Class ;
        rdfs:label       "SolidDrugForm" ;
        rdfs:subClassOf  v3-orderableDrugForm:_DispensableDrugForm ;
        <http://www.w3.org/2004/02/skos/core#definition>
                "SolidDrugForm" ;
        <http://www.w3.org/2004/02/skos/core#prefLabel>
                "SolidDrugForm" .

v3-orderableDrugForm:DOUCHE
        a                owl:Class ;
        rdfs:label       "Douche" ;
        rdfs:subClassOf  v3-orderableDrugForm:IRSOL ;
        <http://www.w3.org/2004/02/skos/core#definition>
                "A liquid preparation, intended for the irrigative cleansing of the vagina, that is prepared from powders, liquid solutions, or liquid concentrates and contains one or more chemical substances dissolved in a suitable solvent or mutually miscible solvents." ;
        <http://www.w3.org/2004/02/skos/core#prefLabel>
                "Douche" .

v3-orderableDrugForm:IVSOL
        a                owl:Class ;
        rdfs:label       "Intravenous Solution" ;
        rdfs:subClassOf  v3-orderableDrugForm:SOL ;
        <http://www.w3.org/2004/02/skos/core#definition>
                "Intravenous Solution" ;
        <http://www.w3.org/2004/02/skos/core#prefLabel>
                "Intravenous Solution" .

v3-orderableDrugForm:OTSUSP
        a                owl:Class ;
        rdfs:label       "Otic Suspension" ;
        rdfs:subClassOf  v3-orderableDrugForm:SUSP ;
        <http://www.w3.org/2004/02/skos/core#definition>
                "Otic Suspension" ;
        <http://www.w3.org/2004/02/skos/core#prefLabel>
                "Otic Suspension" .

v3-orderableDrugForm:CAP
        a                owl:Class ;
        rdfs:label       "Capsule" ;
        rdfs:subClassOf  v3-orderableDrugForm:PILL ;
        <http://www.w3.org/2004/02/skos/core#definition>
                "A solid dosage form in which the drug is enclosed within either a hard or soft soluble container or \"shell\" made from a suitable form of gelatin." ;
        <http://www.w3.org/2004/02/skos/core#prefLabel>
                "Capsule" .

v3-orderableDrugForm:DRTAB
        a                owl:Class ;
        rdfs:label       "Delayed Release Tablet" ;
        rdfs:subClassOf  v3-orderableDrugForm:ORTAB ;
        <http://www.w3.org/2004/02/skos/core#definition>
                "Delayed Release Tablet" ;
        <http://www.w3.org/2004/02/skos/core#prefLabel>
                "Delayed Release Tablet" .

v3-orderableDrugForm:RECFORM
        a                owl:Class ;
        rdfs:label       "Rectal foam" ;
        rdfs:subClassOf  v3-orderableDrugForm:FOAM ;
        <http://www.w3.org/2004/02/skos/core#definition>
                "Rectal foam" ;
        <http://www.w3.org/2004/02/skos/core#prefLabel>
                "Rectal foam" .

v3-orderableDrugForm:BARSOAP
        a                owl:Class ;
        rdfs:label       "Bar Soap" ;
        rdfs:subClassOf  v3-orderableDrugForm:BAR ;
        <http://www.w3.org/2004/02/skos/core#definition>
                "Bar Soap" ;
        <http://www.w3.org/2004/02/skos/core#prefLabel>
                "Bar Soap" .

v3-orderableDrugForm:TOPSOL
        a                owl:Class ;
        rdfs:label       "Topical Solution" ;
        rdfs:subClassOf  v3-orderableDrugForm:SOL ;
        <http://www.w3.org/2004/02/skos/core#definition>
                "Topical Solution" ;
        <http://www.w3.org/2004/02/skos/core#prefLabel>
                "Topical Solution" .

v3-orderableDrugForm:TAB
        a                owl:Class ;
        rdfs:label       "Tablet" ;
        rdfs:subClassOf  v3-orderableDrugForm:PILL ;
        <http://www.w3.org/2004/02/skos/core#definition>
                "A solid dosage form containing medicinal substances with or without suitable diluents." ;
        <http://www.w3.org/2004/02/skos/core#prefLabel>
                "Tablet" .

v3-orderableDrugForm:RECSUSP
        a                owl:Class ;
        rdfs:label       "Rectal Suspension" ;
        rdfs:subClassOf  v3-orderableDrugForm:SUSP ;
        <http://www.w3.org/2004/02/skos/core#definition>
                "Rectal Suspension" ;
        <http://www.w3.org/2004/02/skos/core#prefLabel>
                "Rectal Suspension" .

v3-orderableDrugForm:SLTAB
        a                owl:Class ;
        rdfs:label       "Sublingual Tablet" ;
        rdfs:subClassOf  v3-orderableDrugForm:ORTAB ;
        <http://www.w3.org/2004/02/skos/core#definition>
                "Sublingual Tablet" ;
        <http://www.w3.org/2004/02/skos/core#prefLabel>
                "Sublingual Tablet" .

v3-orderableDrugForm:SWAB
        a                owl:Class ;
        rdfs:label       "Swab" ;
        rdfs:subClassOf  v3-orderableDrugForm:_SolidDrugForm ;
        <http://www.w3.org/2004/02/skos/core#definition>
                "A wad of absorbent material usually wound around one end of a small stick and used for applying medication or for removing material from an area." ;
        <http://www.w3.org/2004/02/skos/core#prefLabel>
                "Swab" .

v3-orderableDrugForm:URETHGEL
        a                owl:Class ;
        rdfs:label       "Urethral Gel" ;
        rdfs:subClassOf  v3-orderableDrugForm:GEL ;
        <http://www.w3.org/2004/02/skos/core#definition>
                "Urethral Gel" ;
        <http://www.w3.org/2004/02/skos/core#prefLabel>
                "Urethral Gel" .

v3-orderableDrugForm:OPCRM
        a                owl:Class ;
        rdfs:label       "Ophthalmic Cream" ;
        rdfs:subClassOf  v3-orderableDrugForm:CRM ;
        <http://www.w3.org/2004/02/skos/core#definition>
                "Ophthalmic Cream" ;
        <http://www.w3.org/2004/02/skos/core#prefLabel>
                "Ophthalmic Cream" .

v3-orderableDrugForm:CHEWTAB
        a                owl:Class ;
        rdfs:label       "Chewable Tablet" ;
        rdfs:subClassOf  v3-orderableDrugForm:ORTAB ;
        <http://www.w3.org/2004/02/skos/core#definition>
                "A solid dosage form containing medicinal substances with or without suitable diluents that is intended to be chewed, producing a pleasant tasting residue in the oral cavity that is easily swallowed and does not leave a bitter or unpleasant after-taste." ;
        <http://www.w3.org/2004/02/skos/core#prefLabel>
                "Chewable Tablet" .

v3-orderableDrugForm:APPFUL
        a                owl:Class ;
        rdfs:label       "Applicatorful" ;
        rdfs:subClassOf  v3-orderableDrugForm:_AdministrableDrugForm ;
        <http://www.w3.org/2004/02/skos/core#definition>
                "Applicatorful" ;
        <http://www.w3.org/2004/02/skos/core#prefLabel>
                "Applicatorful" .

v3-orderableDrugForm:ENEMA
        a                owl:Class ;
        rdfs:label       "Enema" ;
        rdfs:subClassOf  v3-orderableDrugForm:IRSOL ;
        <http://www.w3.org/2004/02/skos/core#definition>
                "A rectal preparation for therapeutic, diagnostic, or nutritive purposes." ;
        <http://www.w3.org/2004/02/skos/core#prefLabel>
                "Enema" .

v3-orderableDrugForm:_LiquidLiquidEmulsion
        a                owl:Class ;
        rdfs:label       "LiquidLiquidEmulsion" ;
        rdfs:subClassOf  v3-orderableDrugForm:_DispensableDrugForm ;
        <http://www.w3.org/2004/02/skos/core#definition>
                "A two-phase system in which one liquid is dispersed throughout another liquid in the form of small droplets." ;
        <http://www.w3.org/2004/02/skos/core#prefLabel>
                "LiquidLiquidEmulsion" .

v3-orderableDrugForm:_GasSolidSpray
        a                owl:Class ;
        rdfs:label       "GasSolidSpray" ;
        rdfs:subClassOf  v3-orderableDrugForm:_DispensableDrugForm ;
        <http://www.w3.org/2004/02/skos/core#definition>
                "GasSolidSpray" ;
        <http://www.w3.org/2004/02/skos/core#prefLabel>
                "GasSolidSpray" .

v3-orderableDrugForm:GUM
        a                owl:Class ;
        rdfs:label       "ChewingGum" ;
        rdfs:subClassOf  v3-orderableDrugForm:_SolidDrugForm ;
        <http://www.w3.org/2004/02/skos/core#definition>
                "A sweetened and flavored insoluble plastic material of various shapes which when chewed, releases a drug substance into the oral cavity." ;
        <http://www.w3.org/2004/02/skos/core#prefLabel>
                "ChewingGum" .

v3-orderableDrugForm:VAGGEL
        a                owl:Class ;
        rdfs:label       "Vaginal Gel" ;
        rdfs:subClassOf  v3-orderableDrugForm:GEL ;
        <http://www.w3.org/2004/02/skos/core#definition>
                "Vaginal Gel" ;
        <http://www.w3.org/2004/02/skos/core#prefLabel>
                "Vaginal Gel" .

v3-orderableDrugForm:TOPOIL
        a                owl:Class ;
        rdfs:label       "Topical Oil" ;
        rdfs:subClassOf  v3-orderableDrugForm:OIL ;
        <http://www.w3.org/2004/02/skos/core#definition>
                "Topical Oil" ;
        <http://www.w3.org/2004/02/skos/core#prefLabel>
                "Topical Oil" .

v3-orderableDrugForm:PELLET
        a                owl:Class ;
        rdfs:label       "Pellet" ;
        rdfs:subClassOf  v3-orderableDrugForm:_SolidDrugForm ;
        <http://www.w3.org/2004/02/skos/core#definition>
                "A small sterile solid mass consisting of a highly purified drug (with or without excipients) made by the formation of granules, or by compression and molding." ;
        <http://www.w3.org/2004/02/skos/core#prefLabel>
                "Pellet" .

v3-orderableDrugForm:NASCRM
        a                owl:Class ;
        rdfs:label       "Nasal Cream" ;
        rdfs:subClassOf  v3-orderableDrugForm:CRM ;
        <http://www.w3.org/2004/02/skos/core#definition>
                "Nasal Cream" ;
        <http://www.w3.org/2004/02/skos/core#prefLabel>
                "Nasal Cream" .

v3-orderableDrugForm:SOL
        a                owl:Class ;
        rdfs:label       "Solution" ;
        rdfs:subClassOf  v3-orderableDrugForm:_Liquid ;
        <http://www.w3.org/2004/02/skos/core#definition>
                "A liquid preparation that contains one or more chemical substances dissolved, i.e., molecularly dispersed, in a suitable solvent or mixture of mutually miscible solvents." ;
        <http://www.w3.org/2004/02/skos/core#prefLabel>
                "Solution" .

v3-orderableDrugForm:NDROP
        a                owl:Class ;
        rdfs:label       "Nasal Drops" ;
        rdfs:subClassOf  v3-orderableDrugForm:DROP ;
        <http://www.w3.org/2004/02/skos/core#definition>
                "Nasal Drops" ;
        <http://www.w3.org/2004/02/skos/core#prefLabel>
                "Nasal Drops" .

v3-orderableDrugForm:OTCRM
        a                owl:Class ;
        rdfs:label       "Otic Cream" ;
        rdfs:subClassOf  v3-orderableDrugForm:CRM ;
        <http://www.w3.org/2004/02/skos/core#definition>
                "Otic Cream" ;
        <http://www.w3.org/2004/02/skos/core#prefLabel>
                "Otic Cream" .

v3-orderableDrugForm:ERCAP
        a                owl:Class ;
        rdfs:label       "Extended Release Capsule" ;
        rdfs:subClassOf  v3-orderableDrugForm:ORCAP ;
        <http://www.w3.org/2004/02/skos/core#definition>
                "A solid dosage form in which the drug is enclosed within either a hard or soft soluble container made from a suitable form of gelatin, and which releases a drug (or drugs) in such a manner to allow a reduction in dosing frequency as compared to that drug (or drugs) presented as a conventional dosage form." ;
        <http://www.w3.org/2004/02/skos/core#prefLabel>
                "Extended Release Capsule" .

v3-orderableDrugForm:ERSUSP
        a                owl:Class ;
        rdfs:label       "Extended-Release Suspension" ;
        rdfs:subClassOf  v3-orderableDrugForm:ORSUSP ;
        <http://www.w3.org/2004/02/skos/core#definition>
                "Extended-Release Suspension" ;
        <http://www.w3.org/2004/02/skos/core#prefLabel>
                "Extended-Release Suspension" .

v3-orderableDrugForm:ERTAB
        a                owl:Class ;
        rdfs:label       "Extended Release Tablet" ;
        rdfs:subClassOf  v3-orderableDrugForm:ORTAB ;
        <http://www.w3.org/2004/02/skos/core#definition>
                "A solid dosage form containing a drug which allows at least a reduction in dosing frequency as compared to that drug presented in conventional dosage form." ;
        <http://www.w3.org/2004/02/skos/core#prefLabel>
                "Extended Release Tablet" .

v3-orderableDrugForm:ORDROP
        a                owl:Class ;
        rdfs:label       "Oral Drops" ;
        rdfs:subClassOf  v3-orderableDrugForm:DROP ;
        <http://www.w3.org/2004/02/skos/core#definition>
                "Oral Drops" ;
        <http://www.w3.org/2004/02/skos/core#prefLabel>
                "Oral Drops" .

v3-orderableDrugForm:OTOINT
        a                owl:Class ;
        rdfs:label       "Otic Ointment" ;
        rdfs:subClassOf  v3-orderableDrugForm:OINT ;
        <http://www.w3.org/2004/02/skos/core#definition>
                "Otic Ointment" ;
        <http://www.w3.org/2004/02/skos/core#prefLabel>
                "Otic Ointment" .

v3-orderableDrugForm:OIL
        a                owl:Class ;
        rdfs:label       "Oil" ;
        rdfs:subClassOf  v3-orderableDrugForm:_Liquid ;
        <http://www.w3.org/2004/02/skos/core#definition>
                "An unctuous, combustible substance which is liquid, or easily liquefiable, on warming, and is soluble in ether but insoluble in water. Such substances, depending on their origin, are classified as animal, mineral, or vegetable oils." ;
        <http://www.w3.org/2004/02/skos/core#prefLabel>
                "Oil" .

v3-orderableDrugForm:ENTCAP
        a                owl:Class ;
        rdfs:label       "Enteric Coated Capsule" ;
        rdfs:subClassOf  v3-orderableDrugForm:ORCAP ;
        <http://www.w3.org/2004/02/skos/core#definition>
                "Enteric Coated Capsule" ;
        <http://www.w3.org/2004/02/skos/core#prefLabel>
                "Enteric Coated Capsule" .

v3-orderableDrugForm:MEDSWAB
        a                owl:Class ;
        rdfs:label       "Medicated swab" ;
        rdfs:subClassOf  v3-orderableDrugForm:SWAB ;
        <http://www.w3.org/2004/02/skos/core#definition>
                "Medicated swab" ;
        <http://www.w3.org/2004/02/skos/core#prefLabel>
                "Medicated swab" .

v3-orderableDrugForm:MDINHLPWD
        a                owl:Class ;
        rdfs:label       "Metered Dose Powder Inhaler" ;
        rdfs:subClassOf  v3-orderableDrugForm:INHL ;
        <http://www.w3.org/2004/02/skos/core#definition>
                "Metered Dose Powder Inhaler" ;
        <http://www.w3.org/2004/02/skos/core#prefLabel>
                "Metered Dose Powder Inhaler" .

v3-orderableDrugForm:SCOOP
        a                owl:Class ;
        rdfs:label       "Scoops" ;
        rdfs:subClassOf  v3-orderableDrugForm:_AdministrableDrugForm ;
        <http://www.w3.org/2004/02/skos/core#definition>
                "Scoops" ;
        <http://www.w3.org/2004/02/skos/core#prefLabel>
                "Scoops" .

v3-orderableDrugForm:ORTROCHE
        a                owl:Class ;
        rdfs:label       "Lozenge/Oral Troche" ;
        rdfs:subClassOf  v3-orderableDrugForm:ORTAB ;
        <http://www.w3.org/2004/02/skos/core#definition>
                "A solid preparation containing one or more medicaments, usually in a flavored, sweetened base which is intended to dissolve or disintegrate slowly in the mouth." ;
        <http://www.w3.org/2004/02/skos/core#prefLabel>
                "Lozenge/Oral Troche" .

v3-orderableDrugForm:_AdministrableDrugForm
        a           owl:Class ;
        rdfs:label  "AdministrableDrugForm" ;
        <http://www.w3.org/2004/02/skos/core#definition>
                "AdministrableDrugForm" ;
        <http://www.w3.org/2004/02/skos/core#prefLabel>
                "AdministrableDrugForm" .

v3-orderableDrugForm:RECPWD
        a                owl:Class ;
        rdfs:label       "Rectal Powder" ;
        rdfs:subClassOf  v3-orderableDrugForm:TOPPWD ;
        <http://www.w3.org/2004/02/skos/core#definition>
                "Rectal Powder" ;
        <http://www.w3.org/2004/02/skos/core#prefLabel>
                "Rectal Powder" .

v3-orderableDrugForm:DISINTAB
        a                owl:Class ;
        rdfs:label       "Disintegrating Tablet" ;
        rdfs:subClassOf  v3-orderableDrugForm:ORTAB ;
        <http://www.w3.org/2004/02/skos/core#definition>
                "A solid dosage form containing medicinal substances which disintegrates rapidly, usually within a matter of seconds, when placed upon the tongue." ;
        <http://www.w3.org/2004/02/skos/core#prefLabel>
                "Disintegrating Tablet" .

v3-orderableDrugForm:ORTAB
        a                owl:Class ;
        rdfs:label       "Oral Tablet" ;
        rdfs:subClassOf  v3-orderableDrugForm:TAB ;
        <http://www.w3.org/2004/02/skos/core#definition>
                "Oral Tablet" ;
        <http://www.w3.org/2004/02/skos/core#prefLabel>
                "Oral Tablet" .

v3-orderableDrugForm:ORALSOL
        a                owl:Class ;
        rdfs:label       "Oral Solution" ;
        rdfs:subClassOf  v3-orderableDrugForm:SOL ;
        <http://www.w3.org/2004/02/skos/core#definition>
                "Oral Solution" ;
        <http://www.w3.org/2004/02/skos/core#prefLabel>
                "Oral Solution" .

v3-orderableDrugForm:OPGEL
        a                owl:Class ;
        rdfs:label       "Ophthalmic Gel" ;
        rdfs:subClassOf  v3-orderableDrugForm:GEL ;
        <http://www.w3.org/2004/02/skos/core#definition>
                "Ophthalmic Gel" ;
        <http://www.w3.org/2004/02/skos/core#prefLabel>
                "Ophthalmic Gel" .

v3-orderableDrugForm:TINC
        a                owl:Class ;
        rdfs:label       "Tincture" ;
        rdfs:subClassOf  v3-orderableDrugForm:TOPSOL ;
        <http://www.w3.org/2004/02/skos/core#definition>
                "Tincture" ;
        <http://www.w3.org/2004/02/skos/core#prefLabel>
                "Tincture" .

v3-orderableDrugForm:BAINHL
        a                owl:Class ;
        rdfs:label       "Breath Activated Inhaler" ;
        rdfs:subClassOf  v3-orderableDrugForm:AER ;
        <http://www.w3.org/2004/02/skos/core#definition>
                "Breath Activated Inhaler" ;
        <http://www.w3.org/2004/02/skos/core#prefLabel>
                "Breath Activated Inhaler" .

v3-orderableDrugForm:INHLPWD
        a                owl:Class ;
        rdfs:label       "Inhalant Powder" ;
        rdfs:subClassOf  v3-orderableDrugForm:INHL ;
        <http://www.w3.org/2004/02/skos/core#definition>
                "Inhalant Powder" ;
        <http://www.w3.org/2004/02/skos/core#prefLabel>
                "Inhalant Powder" .

v3-orderableDrugForm:TPASTE
        a                owl:Class ;
        rdfs:label       "Toothpaste" ;
        rdfs:subClassOf  v3-orderableDrugForm:PASTE ;
        <http://www.w3.org/2004/02/skos/core#definition>
                "A paste formulation intended to clean and/or polish the teeth, and which may contain certain additional agents." ;
        <http://www.w3.org/2004/02/skos/core#prefLabel>
                "Toothpaste" .

v3-orderableDrugForm:ERSUSP12
        a                owl:Class ;
        rdfs:label       "12 Hour Extended-Release Suspension" ;
        rdfs:subClassOf  v3-orderableDrugForm:ERSUSP ;
        <http://www.w3.org/2004/02/skos/core#definition>
                "12 Hour Extended-Release Suspension" ;
        <http://www.w3.org/2004/02/skos/core#prefLabel>
                "12 Hour Extended-Release Suspension" .

v3-orderableDrugForm:TPATH16
        a                owl:Class ;
        rdfs:label       "16 Hour Transdermal Patch" ;
        rdfs:subClassOf  v3-orderableDrugForm:TPATCH ;
        <http://www.w3.org/2004/02/skos/core#definition>
                "16 Hour Transdermal Patch" ;
        <http://www.w3.org/2004/02/skos/core#prefLabel>
                "16 Hour Transdermal Patch" .

v3-orderableDrugForm:PATCH
        a                owl:Class ;
        rdfs:label       "Patch" ;
        rdfs:subClassOf  v3-orderableDrugForm:_SolidDrugForm ;
        <http://www.w3.org/2004/02/skos/core#definition>
                "A drug delivery system that contains an adhesived backing and that permits its ingredients to diffuse from some portion of it (e.g., the backing itself, a reservoir, the adhesive, or some other component) into the body from the external site where it is applied." ;
        <http://www.w3.org/2004/02/skos/core#prefLabel>
                "Patch" .

v3-orderableDrugForm:URETHSUPP
        a                owl:Class ;
        rdfs:label       "Urethral suppository" ;
        rdfs:subClassOf  v3-orderableDrugForm:SUPP ;
        <http://www.w3.org/2004/02/skos/core#definition>
                "Urethral suppository" ;
        <http://www.w3.org/2004/02/skos/core#prefLabel>
                "Urethral suppository" .

v3-orderableDrugForm:NASGEL
        a                owl:Class ;
        rdfs:label       "Nasal Gel" ;
        rdfs:subClassOf  v3-orderableDrugForm:GEL ;
        <http://www.w3.org/2004/02/skos/core#definition>
                "Nasal Gel" ;
        <http://www.w3.org/2004/02/skos/core#prefLabel>
                "Nasal Gel" .

v3-orderableDrugForm:OPDROP
        a                owl:Class ;
        rdfs:label       "Ophthalmic Drops" ;
        rdfs:subClassOf  v3-orderableDrugForm:DROP ;
        <http://www.w3.org/2004/02/skos/core#definition>
                "Ophthalmic Drops" ;
        <http://www.w3.org/2004/02/skos/core#prefLabel>
                "Ophthalmic Drops" .

v3-orderableDrugForm:VAGTAB
        a                owl:Class ;
        rdfs:label       "Vaginal Tablet" ;
        rdfs:subClassOf  v3-orderableDrugForm:TAB ;
        <http://www.w3.org/2004/02/skos/core#definition>
                "Vaginal Tablet" ;
        <http://www.w3.org/2004/02/skos/core#prefLabel>
                "Vaginal Tablet" .

v3-orderableDrugForm:OTGEL
        a                owl:Class ;
        rdfs:label       "Otic Gel" ;
        rdfs:subClassOf  v3-orderableDrugForm:GEL ;
        <http://www.w3.org/2004/02/skos/core#definition>
                "Otic Gel" ;
        <http://www.w3.org/2004/02/skos/core#prefLabel>
                "Otic Gel" .

v3-orderableDrugForm:TPATH24
        a                owl:Class ;
        rdfs:label       "24 Hour Transdermal Patch" ;
        rdfs:subClassOf  v3-orderableDrugForm:TPATCH ;
        <http://www.w3.org/2004/02/skos/core#definition>
                "24 Hour Transdermal Patch" ;
        <http://www.w3.org/2004/02/skos/core#prefLabel>
                "24 Hour Transdermal Patch" .

v3-orderableDrugForm:ERCAP12
        a                owl:Class ;
        rdfs:label       "12 Hour Extended Release Capsule" ;
        rdfs:subClassOf  v3-orderableDrugForm:ERCAP ;
        <http://www.w3.org/2004/02/skos/core#definition>
                "12 Hour Extended Release Capsule" ;
        <http://www.w3.org/2004/02/skos/core#prefLabel>
                "12 Hour Extended Release Capsule" .

v3-orderableDrugForm:_Liquid
        a                owl:Class ;
        rdfs:label       "Liquid" ;
        rdfs:subClassOf  v3-orderableDrugForm:_DispensableDrugForm ;
        <http://www.w3.org/2004/02/skos/core#definition>
                "A state of substance that is an intermediate one entered into as matter goes from solid to gas; liquids are also intermediate in that they have neither the orderliness of a crystal nor the randomness of a gas. (Note: This term should not be used to describe solutions, only pure chemicals in their liquid state.)" ;
        <http://www.w3.org/2004/02/skos/core#prefLabel>
                "Liquid" .

v3-orderableDrugForm:MUCTOPSOL
        a                owl:Class ;
        rdfs:label       "Mucous Membrane Topical Solution" ;
        rdfs:subClassOf  v3-orderableDrugForm:TOPSOL ;
        <http://www.w3.org/2004/02/skos/core#definition>
                "Mucous Membrane Topical Solution" ;
        <http://www.w3.org/2004/02/skos/core#prefLabel>
                "Mucous Membrane Topical Solution" .

v3-orderableDrugForm:ORCRM
        a                owl:Class ;
        rdfs:label       "Oral Cream" ;
        rdfs:subClassOf  v3-orderableDrugForm:CRM ;
        <http://www.w3.org/2004/02/skos/core#definition>
                "Oral Cream" ;
        <http://www.w3.org/2004/02/skos/core#prefLabel>
                "Oral Cream" .

v3-orderableDrugForm:TOPPWD
        a                owl:Class ;
        rdfs:label       "Topical Powder" ;
        rdfs:subClassOf  v3-orderableDrugForm:POWD ;
        <http://www.w3.org/2004/02/skos/core#definition>
                "Topical Powder" ;
        <http://www.w3.org/2004/02/skos/core#prefLabel>
                "Topical Powder" .

v3-orderableDrugForm:RECCRM
        a                owl:Class ;
        rdfs:label       "Rectal Cream" ;
        rdfs:subClassOf  v3-orderableDrugForm:CRM ;
        <http://www.w3.org/2004/02/skos/core#definition>
                "Rectal Cream" ;
        <http://www.w3.org/2004/02/skos/core#prefLabel>
                "Rectal Cream" .

v3-orderableDrugForm:SPRY
        a                owl:Class ;
        rdfs:label       "Sprays" ;
        rdfs:subClassOf  v3-orderableDrugForm:_AdministrableDrugForm ;
        <http://www.w3.org/2004/02/skos/core#definition>
                "Sprays" ;
        <http://www.w3.org/2004/02/skos/core#prefLabel>
                "Sprays" .

v3-orderableDrugForm:ELIXIR
        a                owl:Class ;
        rdfs:label       "Elixir" ;
        rdfs:subClassOf  v3-orderableDrugForm:ORALSOL ;
        <http://www.w3.org/2004/02/skos/core#definition>
                "A clear, pleasantly flavored, sweetened hydroalcoholic liquid containing dissolved medicinal agents; it is intended for oral use." ;
        <http://www.w3.org/2004/02/skos/core#prefLabel>
                "Elixir" .

v3-orderableDrugForm:OINTAPL
        a                owl:Class ;
        rdfs:label       "Ointment with Applicator" ;
        rdfs:subClassOf  v3-orderableDrugForm:OINT ;
        <http://www.w3.org/2004/02/skos/core#definition>
                "Ointment with Applicator" ;
        <http://www.w3.org/2004/02/skos/core#prefLabel>
                "Ointment with Applicator" .

v3-orderableDrugForm:PWDSPRY
        a                owl:Class ;
        rdfs:label       "Powder Spray" ;
        rdfs:subClassOf  v3-orderableDrugForm:_GasSolidSpray ;
        <http://www.w3.org/2004/02/skos/core#definition>
                "Powder Spray" ;
        <http://www.w3.org/2004/02/skos/core#prefLabel>
                "Powder Spray" .

v3-orderableDrugForm:BAINHLPWD
        a                owl:Class ;
        rdfs:label       "Breath Activated Powder Inhaler" ;
        rdfs:subClassOf  v3-orderableDrugForm:INHL ;
        <http://www.w3.org/2004/02/skos/core#definition>
                "Breath Activated Powder Inhaler" ;
        <http://www.w3.org/2004/02/skos/core#prefLabel>
                "Breath Activated Powder Inhaler" .

v3-orderableDrugForm:SYRUP
        a                owl:Class ;
        rdfs:label       "Syrup" ;
        rdfs:subClassOf  v3-orderableDrugForm:ORALSOL ;
        <http://www.w3.org/2004/02/skos/core#definition>
                "An oral solution containing high concentrations of sucrose or other sugars; the term has also been used to include any other liquid dosage form prepared in a sweet and viscid vehicle, including oral suspensions." ;
        <http://www.w3.org/2004/02/skos/core#prefLabel>
                "Syrup" .

v3-orderableDrugForm:VGELAPL
        a                owl:Class ;
        rdfs:label       "Vaginal Gel with Applicator" ;
        rdfs:subClassOf  v3-orderableDrugForm:VAGGEL ;
        <http://www.w3.org/2004/02/skos/core#definition>
                "Vaginal Gel with Applicator" ;
        <http://www.w3.org/2004/02/skos/core#prefLabel>
                "Vaginal Gel with Applicator" .

v3-orderableDrugForm:ERTAB24
        a                owl:Class ;
        rdfs:label       "24 Hour Extended Release Tablet" ;
        rdfs:subClassOf  v3-orderableDrugForm:ERTAB ;
        <http://www.w3.org/2004/02/skos/core#definition>
                "24 Hour Extended Release Tablet" ;
        <http://www.w3.org/2004/02/skos/core#prefLabel>
                "24 Hour Extended Release Tablet" .

v3-orderableDrugForm:
        a                owl:Ontology ;
        rdfs:comment     "  OpenIssue:\r\nMissing description." ;
        rdfs:label       "v3 Code System orderableDrugForm" ;
        owl:versionIRI   "http://hl7.org/fhir/v3/orderableDrugForm/2016-11-11" ;
        owl:versionInfo  "v3 Code System orderableDrugForm(2016-11-11)" .

v3-orderableDrugForm:POWD
        a                owl:Class ;
        rdfs:label       "Powder" ;
        rdfs:subClassOf  v3-orderableDrugForm:_SolidDrugForm ;
        <http://www.w3.org/2004/02/skos/core#definition>
                "An intimate mixture of dry, finely divided drugs and/or chemicals that may be intended for internal or external use." ;
        <http://www.w3.org/2004/02/skos/core#prefLabel>
                "Powder" .

v3-orderableDrugForm:GASINHL
        a                owl:Class ;
        rdfs:label       "Gas for Inhalation" ;
        rdfs:subClassOf  v3-orderableDrugForm:_GasDrugForm ;
        <http://www.w3.org/2004/02/skos/core#definition>
                "Gas for Inhalation" ;
        <http://www.w3.org/2004/02/skos/core#prefLabel>
                "Gas for Inhalation" .

v3-orderableDrugForm:SUPP
        a                owl:Class ;
        rdfs:label       "Suppository" ;
        rdfs:subClassOf  v3-orderableDrugForm:_SolidDrugForm ;
        <http://www.w3.org/2004/02/skos/core#definition>
                "A solid body of various weights and shapes, adapted for introduction into the rectal, vaginal, or urethral orifice of the human body; they usually melt, soften, or dissolve at body temperature." ;
        <http://www.w3.org/2004/02/skos/core#prefLabel>
                "Suppository" .

v3-orderableDrugForm:TPATH2WK
        a                owl:Class ;
        rdfs:label       "Biweekly Transdermal Patch" ;
        rdfs:subClassOf  v3-orderableDrugForm:TPATCH ;
        <http://www.w3.org/2004/02/skos/core#definition>
                "Biweekly Transdermal Patch" ;
        <http://www.w3.org/2004/02/skos/core#prefLabel>
                "Biweekly Transdermal Patch" .

v3-orderableDrugForm:ITSUSP
        a                owl:Class ;
        rdfs:label       "Intrathecal Suspension" ;
        rdfs:subClassOf  v3-orderableDrugForm:SUSP ;
        <http://www.w3.org/2004/02/skos/core#definition>
                "Intrathecal Suspension" ;
        <http://www.w3.org/2004/02/skos/core#prefLabel>
                "Intrathecal Suspension" .

v3-orderableDrugForm:OTDROP
        a                owl:Class ;
        rdfs:label       "Otic Drops" ;
        rdfs:subClassOf  v3-orderableDrugForm:DROP ;
        <http://www.w3.org/2004/02/skos/core#definition>
                "Otic Drops" ;
        <http://www.w3.org/2004/02/skos/core#prefLabel>
                "Otic Drops" .

v3-orderableDrugForm:CAPLET
        a                owl:Class ;
        rdfs:label       "Caplet" ;
        rdfs:subClassOf  v3-orderableDrugForm:ORTAB ;
        <http://www.w3.org/2004/02/skos/core#definition>
                "Caplet" ;
        <http://www.w3.org/2004/02/skos/core#prefLabel>
                "Caplet" .

v3-orderableDrugForm:RINSE
        a                owl:Class ;
        rdfs:label       "Mouthwash/Rinse" ;
        rdfs:subClassOf  v3-orderableDrugForm:ORALSOL ;
        <http://www.w3.org/2004/02/skos/core#definition>
                "An aqueous solution which is most often used for its deodorant, refreshing, or antiseptic effect." ;
        <http://www.w3.org/2004/02/skos/core#prefLabel>
                "Mouthwash/Rinse" .

v3-orderableDrugForm:PILL
        a                owl:Class ;
        rdfs:label       "Pill" ;
        rdfs:subClassOf  v3-orderableDrugForm:_SolidDrugForm ;
        <http://www.w3.org/2004/02/skos/core#definition>
                "A small, round solid dosage form containing a medicinal agent intended for oral administration." ;
        <http://www.w3.org/2004/02/skos/core#prefLabel>
                "Pill" .

v3-orderableDrugForm:OINT
        a                owl:Class ;
        rdfs:label       "Ointment" ;
        rdfs:subClassOf  v3-orderableDrugForm:_LiquidLiquidEmulsion ;
        <http://www.w3.org/2004/02/skos/core#definition>
                "A semisolid preparation intended for external application to the skin or mucous membranes." ;
        <http://www.w3.org/2004/02/skos/core#prefLabel>
                "Ointment" .

v3-orderableDrugForm:OPOINT
        a                owl:Class ;
        rdfs:label       "Ophthalmic Ointment" ;
        rdfs:subClassOf  v3-orderableDrugForm:OINT ;
        <http://www.w3.org/2004/02/skos/core#definition>
                "Ophthalmic Ointment" ;
        <http://www.w3.org/2004/02/skos/core#prefLabel>
                "Ophthalmic Ointment" .

v3-orderableDrugForm:_DispensableDrugForm
        a           owl:Class ;
        rdfs:label  "DispensableDrugForm" ;
        <http://www.w3.org/2004/02/skos/core#definition>
                "DispensableDrugForm" ;
        <http://www.w3.org/2004/02/skos/core#prefLabel>
                "DispensableDrugForm" .

v3-orderableDrugForm:TOPCRM
        a                owl:Class ;
        rdfs:label       "Topical Cream" ;
        rdfs:subClassOf  v3-orderableDrugForm:CRM ;
        <http://www.w3.org/2004/02/skos/core#definition>
                "Topical Cream" ;
        <http://www.w3.org/2004/02/skos/core#prefLabel>
                "Topical Cream" .

v3-orderableDrugForm:RECSPRY
        a                owl:Class ;
        rdfs:label       "Rectal Spray" ;
        rdfs:subClassOf  v3-orderableDrugForm:_GasLiquidMixture ;
        <http://www.w3.org/2004/02/skos/core#definition>
                "Rectal Spray" ;
        <http://www.w3.org/2004/02/skos/core#prefLabel>
                "Rectal Spray" .

v3-orderableDrugForm:CPTAB
        a                owl:Class ;
        rdfs:label       "Coated Particles Tablet" ;
        rdfs:subClassOf  v3-orderableDrugForm:ORTAB ;
        <http://www.w3.org/2004/02/skos/core#definition>
                "Coated Particles Tablet" ;
        <http://www.w3.org/2004/02/skos/core#prefLabel>
                "Coated Particles Tablet" .

v3-orderableDrugForm:WAFER
        a                owl:Class ;
        rdfs:label       "Wafer" ;
        rdfs:subClassOf  v3-orderableDrugForm:_SolidDrugForm ;
        <http://www.w3.org/2004/02/skos/core#definition>
                "A thin slice of material containing a medicinal agent." ;
        <http://www.w3.org/2004/02/skos/core#prefLabel>
                "Wafer" .

v3-orderableDrugForm:SRBUCTAB
        a                owl:Class ;
        rdfs:label       "Sustained Release Buccal Tablet" ;
        rdfs:subClassOf  v3-orderableDrugForm:BUCTAB ;
        <http://www.w3.org/2004/02/skos/core#definition>
                "Sustained Release Buccal Tablet" ;
        <http://www.w3.org/2004/02/skos/core#prefLabel>
                "Sustained Release Buccal Tablet" .

v3-orderableDrugForm:FOAM
        a                owl:Class ;
        rdfs:label       "Foam" ;
        rdfs:subClassOf  v3-orderableDrugForm:_GasLiquidMixture ;
        <http://www.w3.org/2004/02/skos/core#definition>
                "Foam" ;
        <http://www.w3.org/2004/02/skos/core#prefLabel>
                "Foam" .

v3-orderableDrugForm:ERECCAP
        a                owl:Class ;
        rdfs:label       "Extended Release Enteric Coated Capsule" ;
        rdfs:subClassOf  v3-orderableDrugForm:ERCAP ;
        <http://www.w3.org/2004/02/skos/core#definition>
                "Rationale: Duplicate of code ERENTCAP. Use code ERENTCAP instead." ;
        <http://www.w3.org/2004/02/skos/core#prefLabel>
                "Extended Release Enteric Coated Capsule" .

v3-orderableDrugForm:CRM
        a                owl:Class ;
        rdfs:label       "Cream" ;
        rdfs:subClassOf  v3-orderableDrugForm:_LiquidLiquidEmulsion ;
        <http://www.w3.org/2004/02/skos/core#definition>
                "A semisolid dosage form containing one or more drug substances dissolved or dispersed in a suitable base; more recently, the term has been restricted to products consisting of oil-in-water emulsions or aqueous microcrystalline dispersions of long chain fatty acids or alcohols that are water washable and more cosmetically and aesthetically acceptable." ;
        <http://www.w3.org/2004/02/skos/core#prefLabel>
                "Cream" .

v3-orderableDrugForm:PUFF
        a                owl:Class ;
        rdfs:label       "Puff" ;
        rdfs:subClassOf  v3-orderableDrugForm:_AdministrableDrugForm ;
        <http://www.w3.org/2004/02/skos/core#definition>
                "Puff" ;
        <http://www.w3.org/2004/02/skos/core#prefLabel>
                "Puff" .

v3-orderableDrugForm:ERECTAB
        a                owl:Class ;
        rdfs:label       "Extended Release Enteric Coated Tablet" ;
        rdfs:subClassOf  v3-orderableDrugForm:ECTAB ;
        <http://www.w3.org/2004/02/skos/core#definition>
                "Extended Release Enteric Coated Tablet" ;
        <http://www.w3.org/2004/02/skos/core#prefLabel>
                "Extended Release Enteric Coated Tablet" .

v3-orderableDrugForm:VAGFOAMAPL
        a                owl:Class ;
        rdfs:label       "Vaginal foam with applicator" ;
        rdfs:subClassOf  v3-orderableDrugForm:VAGFOAM ;
        <http://www.w3.org/2004/02/skos/core#definition>
                "Vaginal foam with applicator" ;
        <http://www.w3.org/2004/02/skos/core#prefLabel>
                "Vaginal foam with applicator" .

v3-orderableDrugForm:NASINHL
        a                owl:Class ;
        rdfs:label       "Nasal Inhalant" ;
        rdfs:subClassOf  v3-orderableDrugForm:INHL ;
        <http://www.w3.org/2004/02/skos/core#definition>
                "Nasal Inhalant" ;
        <http://www.w3.org/2004/02/skos/core#prefLabel>
                "Nasal Inhalant" .

v3-orderableDrugForm:RECSUPP
        a                owl:Class ;
        rdfs:label       "Rectal Suppository" ;
        rdfs:subClassOf  v3-orderableDrugForm:SUPP ;
        <http://www.w3.org/2004/02/skos/core#definition>
                "Rectal Suppository" ;
        <http://www.w3.org/2004/02/skos/core#prefLabel>
                "Rectal Suppository" .

v3-orderableDrugForm:VAGSPRY
        a                owl:Class ;
        rdfs:label       "Vaginal Spray" ;
        rdfs:subClassOf  v3-orderableDrugForm:_GasLiquidMixture ;
        <http://www.w3.org/2004/02/skos/core#definition>
                "Vaginal Spray" ;
        <http://www.w3.org/2004/02/skos/core#prefLabel>
                "Vaginal Spray" .

v3-orderableDrugForm:GELAPL
        a                owl:Class ;
        rdfs:label       "Gel with Applicator" ;
        rdfs:subClassOf  v3-orderableDrugForm:GEL ;
        <http://www.w3.org/2004/02/skos/core#definition>
                "Gel with Applicator" ;
        <http://www.w3.org/2004/02/skos/core#prefLabel>
                "Gel with Applicator" .

v3-orderableDrugForm:DERMSPRY
        a                owl:Class ;
        rdfs:label       "Dermal Spray" ;
        rdfs:subClassOf  v3-orderableDrugForm:_GasLiquidMixture ;
        <http://www.w3.org/2004/02/skos/core#definition>
                "Dermal Spray" ;
        <http://www.w3.org/2004/02/skos/core#prefLabel>
                "Dermal Spray" .

v3-orderableDrugForm:IPSOL
        a                owl:Class ;
        rdfs:label       "Intraperitoneal Solution" ;
        rdfs:subClassOf  v3-orderableDrugForm:SOL ;
        <http://www.w3.org/2004/02/skos/core#definition>
                "Intraperitoneal Solution" ;
        <http://www.w3.org/2004/02/skos/core#prefLabel>
                "Intraperitoneal Solution" .

v3-orderableDrugForm:TPATH72
        a                owl:Class ;
        rdfs:label       "72 Hour Transdermal Patch" ;
        rdfs:subClassOf  v3-orderableDrugForm:TPATCH ;
        <http://www.w3.org/2004/02/skos/core#definition>
                "72 Hour Transdermal Patch" ;
        <http://www.w3.org/2004/02/skos/core#prefLabel>
                "72 Hour Transdermal Patch" .

v3-orderableDrugForm:ORINHL
        a                owl:Class ;
        rdfs:label       "Oral Inhalant" ;
        rdfs:subClassOf  v3-orderableDrugForm:INHL ;
        <http://www.w3.org/2004/02/skos/core#definition>
                "Oral Inhalant" ;
        <http://www.w3.org/2004/02/skos/core#prefLabel>
                "Oral Inhalant" .

v3-orderableDrugForm:MEDPAD
        a                owl:Class ;
        rdfs:label       "Medicated Pad" ;
        rdfs:subClassOf  v3-orderableDrugForm:PAD ;
        <http://www.w3.org/2004/02/skos/core#definition>
                "Medicated Pad" ;
        <http://www.w3.org/2004/02/skos/core#prefLabel>
                "Medicated Pad" .

v3-orderableDrugForm:LIQCLN
        a                owl:Class ;
        rdfs:label       "Liquid Cleanser" ;
        rdfs:subClassOf  v3-orderableDrugForm:_Liquid ;
        <http://www.w3.org/2004/02/skos/core#definition>
                "Liquid Cleanser" ;
        <http://www.w3.org/2004/02/skos/core#prefLabel>
                "Liquid Cleanser" .

v3-orderableDrugForm:NASSPRY
        a                owl:Class ;
        rdfs:label       "Nasal Spray" ;
        rdfs:subClassOf  v3-orderableDrugForm:AER ;
        <http://www.w3.org/2004/02/skos/core#definition>
                "Nasal Spray" ;
        <http://www.w3.org/2004/02/skos/core#prefLabel>
                "Nasal Spray" .

v3-orderableDrugForm:RECOINT
        a                owl:Class ;
        rdfs:label       "Rectal Ointment" ;
        rdfs:subClassOf  v3-orderableDrugForm:OINT ;
        <http://www.w3.org/2004/02/skos/core#definition>
                "Rectal Ointment" ;
        <http://www.w3.org/2004/02/skos/core#prefLabel>
                "Rectal Ointment" .

v3-orderableDrugForm:GRAN
        a                owl:Class ;
        rdfs:label       "Granules" ;
        rdfs:subClassOf  v3-orderableDrugForm:_SolidDrugForm ;
        <http://www.w3.org/2004/02/skos/core#definition>
                "A small particle or grain." ;
        <http://www.w3.org/2004/02/skos/core#prefLabel>
                "Granules" .

v3-orderableDrugForm:VAGSUPP
        a                owl:Class ;
        rdfs:label       "Vaginal Suppository" ;
        rdfs:subClassOf  v3-orderableDrugForm:SUPP ;
        <http://www.w3.org/2004/02/skos/core#definition>
                "Vaginal Suppository" ;
        <http://www.w3.org/2004/02/skos/core#prefLabel>
                "Vaginal Suppository" .

v3-orderableDrugForm:TOPLTN
        a                owl:Class ;
        rdfs:label       "Topical Lotion" ;
        rdfs:subClassOf  v3-orderableDrugForm:LTN ;
        <http://www.w3.org/2004/02/skos/core#definition>
                "Topical Lotion" ;
        <http://www.w3.org/2004/02/skos/core#prefLabel>
                "Topical Lotion" .

v3-orderableDrugForm:VAGCRMAPL
        a                owl:Class ;
        rdfs:label       "Vaginal Cream with Applicator" ;
        rdfs:subClassOf  v3-orderableDrugForm:VAGCRM ;
        <http://www.w3.org/2004/02/skos/core#definition>
                "Vaginal Cream with Applicator" ;
        <http://www.w3.org/2004/02/skos/core#prefLabel>
                "Vaginal Cream with Applicator" .

v3-orderableDrugForm:MEDBAR
        a                owl:Class ;
        rdfs:label       "Medicated Bar Soap" ;
        rdfs:subClassOf  v3-orderableDrugForm:BARSOAP ;
        <http://www.w3.org/2004/02/skos/core#definition>
                "Medicated Bar Soap" ;
        <http://www.w3.org/2004/02/skos/core#prefLabel>
                "Medicated Bar Soap" .

v3-orderableDrugForm:TOPGEL
        a                owl:Class ;
        rdfs:label       "Topical Gel" ;
        rdfs:subClassOf  v3-orderableDrugForm:GEL ;
        <http://www.w3.org/2004/02/skos/core#definition>
                "Topical Gel" ;
        <http://www.w3.org/2004/02/skos/core#prefLabel>
                "Topical Gel" .

v3-orderableDrugForm:PAD
        a                owl:Class ;
        rdfs:label       "Pad" ;
        rdfs:subClassOf  v3-orderableDrugForm:_SolidDrugForm ;
        <http://www.w3.org/2004/02/skos/core#definition>
                "Pad" ;
        <http://www.w3.org/2004/02/skos/core#prefLabel>
                "Pad" .

v3-orderableDrugForm:FOAMAPL
        a                owl:Class ;
        rdfs:label       "Foam with Applicator" ;
        rdfs:subClassOf  v3-orderableDrugForm:FOAM ;
        <http://www.w3.org/2004/02/skos/core#definition>
                "Foam with Applicator" ;
        <http://www.w3.org/2004/02/skos/core#prefLabel>
                "Foam with Applicator" .

v3-orderableDrugForm:ORSUSP
        a                owl:Class ;
        rdfs:label       "Oral Suspension" ;
        rdfs:subClassOf  v3-orderableDrugForm:SUSP ;
        <http://www.w3.org/2004/02/skos/core#definition>
                "Oral Suspension" ;
        <http://www.w3.org/2004/02/skos/core#prefLabel>
                "Oral Suspension" .

v3-orderableDrugForm:SPRYADAPT
        a                owl:Class ;
        rdfs:label       "Spray with Adaptor" ;
        rdfs:subClassOf  v3-orderableDrugForm:_GasSolidSpray ;
        <http://www.w3.org/2004/02/skos/core#definition>
                "Spray with Adaptor" ;
        <http://www.w3.org/2004/02/skos/core#prefLabel>
                "Spray with Adaptor" .

v3-orderableDrugForm:VAGOINT
        a                owl:Class ;
        rdfs:label       "Vaginal Ointment" ;
        rdfs:subClassOf  v3-orderableDrugForm:OINT ;
        <http://www.w3.org/2004/02/skos/core#definition>
                "Vaginal Ointment" ;
        <http://www.w3.org/2004/02/skos/core#prefLabel>
                "Vaginal Ointment" .

v3-orderableDrugForm:TPATCH
        a                owl:Class ;
        rdfs:label       "Transdermal Patch" ;
        rdfs:subClassOf  v3-orderableDrugForm:PATCH ;
        <http://www.w3.org/2004/02/skos/core#definition>
                "Transdermal Patch" ;
        <http://www.w3.org/2004/02/skos/core#prefLabel>
                "Transdermal Patch" .

v3-orderableDrugForm:BAR
        a                owl:Class ;
        rdfs:label       "Bar" ;
        rdfs:subClassOf  v3-orderableDrugForm:_SolidDrugForm ;
        <http://www.w3.org/2004/02/skos/core#definition>
                "Bar" ;
        <http://www.w3.org/2004/02/skos/core#prefLabel>
                "Bar" .

v3-orderableDrugForm:ERENTCAP
        a                owl:Class ;
        rdfs:label       "Extended Release Enteric Coated Capsule" ;
        rdfs:subClassOf  v3-orderableDrugForm:ENTCAP ;
        <http://www.w3.org/2004/02/skos/core#definition>
                "Extended Release Enteric Coated Capsule" ;
        <http://www.w3.org/2004/02/skos/core#prefLabel>
                "Extended Release Enteric Coated Capsule" .

v3-orderableDrugForm:SHMP
        a                owl:Class ;
        rdfs:label       "Shampoo" ;
        rdfs:subClassOf  v3-orderableDrugForm:LIQCLN ;
        <http://www.w3.org/2004/02/skos/core#definition>
                "A liquid soap or detergent used to clean the hair and scalp and is often used as a vehicle for dermatologic agents." ;
        <http://www.w3.org/2004/02/skos/core#prefLabel>
                "Shampoo" .

v3-orderableDrugForm:FLAKE
        a                owl:Class ;
        rdfs:label       "Flakes" ;
        rdfs:subClassOf  v3-orderableDrugForm:_SolidDrugForm ;
        <http://www.w3.org/2004/02/skos/core#definition>
                "Flakes" ;
        <http://www.w3.org/2004/02/skos/core#prefLabel>
                "Flakes" .

v3-orderableDrugForm:CEMENT
        a                owl:Class ;
        rdfs:label       "Cement" ;
        rdfs:subClassOf  v3-orderableDrugForm:_SolidDrugForm ;
        <http://www.w3.org/2004/02/skos/core#definition>
                "A substance that serves to produce solid union between two surfaces." ;
        <http://www.w3.org/2004/02/skos/core#prefLabel>
                "Cement" .

v3-orderableDrugForm:VAGPWD
        a                owl:Class ;
        rdfs:label       "Vaginal Powder" ;
        rdfs:subClassOf  v3-orderableDrugForm:TOPPWD ;
        <http://www.w3.org/2004/02/skos/core#definition>
                "Vaginal Powder" ;
        <http://www.w3.org/2004/02/skos/core#prefLabel>
                "Vaginal Powder" .

v3-orderableDrugForm:NASOINT
        a                owl:Class ;
        rdfs:label       "Nasal Ointment" ;
        rdfs:subClassOf  v3-orderableDrugForm:OINT ;
        <http://www.w3.org/2004/02/skos/core#definition>
                "Nasal Ointment" ;
        <http://www.w3.org/2004/02/skos/core#prefLabel>
                "Nasal Ointment" .

v3-orderableDrugForm:LTN
        a                owl:Class ;
        rdfs:label       "Lotion" ;
        rdfs:subClassOf  v3-orderableDrugForm:_LiquidLiquidEmulsion ;
        <http://www.w3.org/2004/02/skos/core#definition>
                "The term \"lotion\" has been used to categorize many topical suspensions, solutions and emulsions intended for application to the skin." ;
        <http://www.w3.org/2004/02/skos/core#prefLabel>
                "Lotion" .

v3-orderableDrugForm:LIQSOAP
        a                owl:Class ;
        rdfs:label       "Medicated Liquid Soap" ;
        rdfs:subClassOf  v3-orderableDrugForm:LIQCLN ;
        <http://www.w3.org/2004/02/skos/core#definition>
                "Medicated Liquid Soap" ;
        <http://www.w3.org/2004/02/skos/core#prefLabel>
                "Medicated Liquid Soap" .

v3-orderableDrugForm:DROP
        a                owl:Class ;
        rdfs:label       "Drops" ;
        rdfs:subClassOf  v3-orderableDrugForm:_AdministrableDrugForm ;
        <http://www.w3.org/2004/02/skos/core#definition>
                "Drops" ;
        <http://www.w3.org/2004/02/skos/core#prefLabel>
                "Drops" .

v3-orderableDrugForm:_GasDrugForm
        a                owl:Class ;
        rdfs:label       "GasDrugForm" ;
        rdfs:subClassOf  v3-orderableDrugForm:_DispensableDrugForm ;
        <http://www.w3.org/2004/02/skos/core#definition>
                "Any elastic aeriform fluid in which the molecules are separated from one another and have free paths." ;
        <http://www.w3.org/2004/02/skos/core#prefLabel>
                "GasDrugForm" .

v3-orderableDrugForm:INHL
        a                owl:Class ;
        rdfs:label       "Inhalant" ;
        rdfs:subClassOf  v3-orderableDrugForm:_GasSolidSpray ;
        <http://www.w3.org/2004/02/skos/core#definition>
                "Inhalant" ;
        <http://www.w3.org/2004/02/skos/core#prefLabel>
                "Inhalant" .

v3-orderableDrugForm:CHEWBAR
        a                owl:Class ;
        rdfs:label       "Chewable Bar" ;
        rdfs:subClassOf  v3-orderableDrugForm:BAR ;
        <http://www.w3.org/2004/02/skos/core#definition>
                "A solid dosage form usually in the form of a rectangle that is meant to be chewed." ;
        <http://www.w3.org/2004/02/skos/core#prefLabel>
                "Chewable Bar" .

v3-orderableDrugForm:_GasLiquidMixture
        a                owl:Class ;
        rdfs:label       "GasLiquidMixture" ;
        rdfs:subClassOf  v3-orderableDrugForm:_DispensableDrugForm ;
        <http://www.w3.org/2004/02/skos/core#definition>
                "GasLiquidMixture" ;
        <http://www.w3.org/2004/02/skos/core#prefLabel>
                "GasLiquidMixture" .

v3-orderableDrugForm:ORCAP
        a                owl:Class ;
        rdfs:label       "Oral Capsule" ;
        rdfs:subClassOf  v3-orderableDrugForm:CAP ;
        <http://www.w3.org/2004/02/skos/core#definition>
                "Oral Capsule" ;
        <http://www.w3.org/2004/02/skos/core#prefLabel>
                "Oral Capsule" .

v3-orderableDrugForm:GEL
        a                owl:Class ;
        rdfs:label       "Gel" ;
        rdfs:subClassOf  v3-orderableDrugForm:_LiquidSolidSuspension ;
        <http://www.w3.org/2004/02/skos/core#definition>
                "A semisolid system consisting of either suspensions made up of small inorganic particles or large organic molecules interpenetrated by a liquid." ;
        <http://www.w3.org/2004/02/skos/core#prefLabel>
                "Gel" .

v3-orderableDrugForm:BUCTAB
        a                owl:Class ;
        rdfs:label       "Buccal Tablet" ;
        rdfs:subClassOf  v3-orderableDrugForm:ORTAB ;
        <http://www.w3.org/2004/02/skos/core#definition>
                "Buccal Tablet" ;
        <http://www.w3.org/2004/02/skos/core#prefLabel>
                "Buccal Tablet" .

v3-orderableDrugForm:TOPOINT
        a                owl:Class ;
        rdfs:label       "Topical Ointment" ;
        rdfs:subClassOf  v3-orderableDrugForm:OINT ;
        <http://www.w3.org/2004/02/skos/core#definition>
                "Topical Ointment" ;
        <http://www.w3.org/2004/02/skos/core#prefLabel>
                "Topical Ointment" .

v3-orderableDrugForm:VAGFOAM
        a                owl:Class ;
        rdfs:label       "Vaginal foam" ;
        rdfs:subClassOf  v3-orderableDrugForm:FOAM ;
        <http://www.w3.org/2004/02/skos/core#definition>
                "Vaginal foam" ;
        <http://www.w3.org/2004/02/skos/core#prefLabel>
                "Vaginal foam" .

v3-orderableDrugForm:_LiquidSolidSuspension
        a                owl:Class ;
        rdfs:label       "LiquidSolidSuspension" ;
        rdfs:subClassOf  v3-orderableDrugForm:_DispensableDrugForm ;
        <http://www.w3.org/2004/02/skos/core#definition>
                "A liquid preparation which consists of solid particles dispersed throughout a liquid phase in which the particles are not soluble." ;
        <http://www.w3.org/2004/02/skos/core#prefLabel>
                "LiquidSolidSuspension" .

v3-orderableDrugForm:VAGOINTAPL
        a                owl:Class ;
        rdfs:label       "Vaginal Ointment with Applicator" ;
        rdfs:subClassOf  v3-orderableDrugForm:VAGOINT ;
        <http://www.w3.org/2004/02/skos/core#definition>
                "Vaginal Ointment with Applicator" ;
        <http://www.w3.org/2004/02/skos/core#prefLabel>
                "Vaginal Ointment with Applicator" .

v3-orderableDrugForm:PUD
        a                owl:Class ;
        rdfs:label       "Pudding" ;
        rdfs:subClassOf  v3-orderableDrugForm:PASTE ;
        <http://www.w3.org/2004/02/skos/core#definition>
                "Pudding" ;
        <http://www.w3.org/2004/02/skos/core#prefLabel>
                "Pudding" .

v3-orderableDrugForm:ERTAB12
        a                owl:Class ;
        rdfs:label       "12 Hour Extended Release Tablet" ;
        rdfs:subClassOf  v3-orderableDrugForm:ERTAB ;
        <http://www.w3.org/2004/02/skos/core#definition>
                "12 Hour Extended Release Tablet" ;
        <http://www.w3.org/2004/02/skos/core#prefLabel>
                "12 Hour Extended Release Tablet" .

v3-orderableDrugForm:SUSP
        a                owl:Class ;
        rdfs:label       "Suspension" ;
        rdfs:subClassOf  v3-orderableDrugForm:_LiquidSolidSuspension ;
        <http://www.w3.org/2004/02/skos/core#definition>
                "Suspension" ;
        <http://www.w3.org/2004/02/skos/core#prefLabel>
                "Suspension" .

v3-orderableDrugForm:ERSUSP24
        a                owl:Class ;
        rdfs:label       "24 Hour Extended Release Suspension" ;
        rdfs:subClassOf  v3-orderableDrugForm:ERSUSP ;
        <http://www.w3.org/2004/02/skos/core#definition>
                "24 Hour Extended Release Suspension" ;
        <http://www.w3.org/2004/02/skos/core#prefLabel>
                "24 Hour Extended Release Suspension" .

v3-orderableDrugForm:OPSUSP
        a                owl:Class ;
        rdfs:label       "Ophthalmic Suspension" ;
        rdfs:subClassOf  v3-orderableDrugForm:SUSP ;
        <http://www.w3.org/2004/02/skos/core#definition>
                "Ophthalmic Suspension" ;
        <http://www.w3.org/2004/02/skos/core#prefLabel>
                "Ophthalmic Suspension" .

v3-orderableDrugForm:MDINHL
        a                owl:Class ;
        rdfs:label       "Metered Dose Inhaler" ;
        rdfs:subClassOf  v3-orderableDrugForm:AER ;
        <http://www.w3.org/2004/02/skos/core#definition>
                "Metered Dose Inhaler" ;
        <http://www.w3.org/2004/02/skos/core#prefLabel>
                "Metered Dose Inhaler" .

v3-orderableDrugForm:PASTE
        a                owl:Class ;
        rdfs:label       "Paste" ;
        rdfs:subClassOf  v3-orderableDrugForm:_LiquidSolidSuspension ;
        <http://www.w3.org/2004/02/skos/core#definition>
                "A semisolid dosage form that contains one or more drug substances intended for topical application." ;
        <http://www.w3.org/2004/02/skos/core#prefLabel>
                "Paste" .

v3-orderableDrugForm:BEAD
        a                owl:Class ;
        rdfs:label       "Beads" ;
        rdfs:subClassOf  v3-orderableDrugForm:_SolidDrugForm ;
        <http://www.w3.org/2004/02/skos/core#definition>
                "A solid dosage form in the shape of a small ball." ;
        <http://www.w3.org/2004/02/skos/core#prefLabel>
                "Beads" .

v3-orderableDrugForm:VAGCRM
        a                owl:Class ;
        rdfs:label       "Vaginal Cream" ;
        rdfs:subClassOf  v3-orderableDrugForm:CRM ;
        <http://www.w3.org/2004/02/skos/core#definition>
                "Vaginal Cream" ;
        <http://www.w3.org/2004/02/skos/core#prefLabel>
                "Vaginal Cream" .

v3-orderableDrugForm:CRYS
        a                owl:Class ;
        rdfs:label       "Crystals" ;
        rdfs:subClassOf  v3-orderableDrugForm:_SolidDrugForm ;
        <http://www.w3.org/2004/02/skos/core#definition>
                "A naturally produced angular solid of definite form in which the ultimate units from which it is built up are systematically arranged; they are usually evenly spaced on a regular space lattice." ;
        <http://www.w3.org/2004/02/skos/core#prefLabel>
                "Crystals" .

v3-orderableDrugForm:LIN
        a                owl:Class ;
        rdfs:label       "Liniment" ;
        rdfs:subClassOf  v3-orderableDrugForm:TOPSOL ;
        <http://www.w3.org/2004/02/skos/core#definition>
                "A solution or mixture of various substances in oil, alcoholic solutions of soap, or emulsions intended for external application." ;
        <http://www.w3.org/2004/02/skos/core#prefLabel>
                "Liniment" .

v3-orderableDrugForm:CAKE
        a                owl:Class ;
        rdfs:label       "Cake" ;
        rdfs:subClassOf  v3-orderableDrugForm:_SolidDrugForm ;
        <http://www.w3.org/2004/02/skos/core#definition>
                "Cake" ;
        <http://www.w3.org/2004/02/skos/core#prefLabel>
                "Cake" .

v3-orderableDrugForm:RECSOL
        a                owl:Class ;
        rdfs:label       "Rectal Solution" ;
        rdfs:subClassOf  v3-orderableDrugForm:SOL ;
        <http://www.w3.org/2004/02/skos/core#definition>
                "Rectal Solution" ;
        <http://www.w3.org/2004/02/skos/core#prefLabel>
                "Rectal Solution" .

v3-orderableDrugForm:DISK
        a                owl:Class ;
        rdfs:label       "Disk" ;
        rdfs:subClassOf  v3-orderableDrugForm:_SolidDrugForm ;
        <http://www.w3.org/2004/02/skos/core#definition>
                "A circular plate-like organ or structure." ;
        <http://www.w3.org/2004/02/skos/core#prefLabel>
                "Disk" .

v3-orderableDrugForm:ECTAB
        a                owl:Class ;
        rdfs:label       "Enteric Coated Tablet" ;
        rdfs:subClassOf  v3-orderableDrugForm:ORTAB ;
        <http://www.w3.org/2004/02/skos/core#definition>
                "Enteric Coated Tablet" ;
        <http://www.w3.org/2004/02/skos/core#prefLabel>
                "Enteric Coated Tablet" .

v3-orderableDrugForm:IRSOL
        a                owl:Class ;
        rdfs:label       "Irrigation Solution" ;
        rdfs:subClassOf  v3-orderableDrugForm:SOL ;
        <http://www.w3.org/2004/02/skos/core#definition>
                "A sterile solution intended to bathe or flush open wounds or body cavities; they're used topically, never parenterally." ;
        <http://www.w3.org/2004/02/skos/core#prefLabel>
                "Irrigation Solution" .

v3-orderableDrugForm:ERCAP24
        a                owl:Class ;
        rdfs:label       "24 Hour Extended Release Capsule" ;
        rdfs:subClassOf  v3-orderableDrugForm:ERCAP ;
        <http://www.w3.org/2004/02/skos/core#definition>
                "24 Hour Extended Release Capsule" ;
        <http://www.w3.org/2004/02/skos/core#prefLabel>
                "24 Hour Extended Release Capsule" .

v3-orderableDrugForm:INHLSOL
        a                owl:Class ;
        rdfs:label       "Inhalant Solution" ;
        rdfs:subClassOf  v3-orderableDrugForm:AER ;
        <http://www.w3.org/2004/02/skos/core#definition>
                "Inhalant Solution" ;
        <http://www.w3.org/2004/02/skos/core#prefLabel>
                "Inhalant Solution" .

v3-orderableDrugForm:OPIRSOL
        a                owl:Class ;
        rdfs:label       "Ophthalmic Irrigation Solution" ;
        rdfs:subClassOf  v3-orderableDrugForm:IRSOL ;
        <http://www.w3.org/2004/02/skos/core#definition>
                "Ophthalmic Irrigation Solution" ;
        <http://www.w3.org/2004/02/skos/core#prefLabel>
                "Ophthalmic Irrigation Solution" .
