@prefix v3-ActExposureLevelCode: <http://hl7.org/fhir/v3/ActExposureLevelCode/> .
@prefix fhir:  <http://hl7.org/fhir/> .
@prefix rdf:   <http://www.w3.org/1999/02/22-rdf-syntax-ns#> .
@prefix owl:   <http://www.w3.org/2002/07/owl#> .
@prefix xsd:   <http://www.w3.org/2001/XMLSchema#> .
@prefix rdfs:  <http://www.w3.org/2000/01/rdf-schema#> .
@prefix w5:    <http://hl7.org/fhir/w5#> .

v3-ActExposureLevelCode:HIGH
        a                owl:Class ;
        rdfs:label       "high" ;
        rdfs:subClassOf  v3-ActExposureLevelCode:_ActExposureLevelCode ;
        <http://www.w3.org/2004/02/skos/core#definition>
                "Description: Exposure to an agent at a relatively high level above background." ;
        <http://www.w3.org/2004/02/skos/core#prefLabel>
                "high" .

v3-ActExposureLevelCode:_ActExposureLevelCode
        a           owl:Class ;
        rdfs:label  "ActExposureLevelCode" ;
        <http://www.w3.org/2004/02/skos/core#definition>
                "A qualitative measure of the degree of exposure to the causative agent.  This includes concepts such as \"low\", \"medium\" and \"high\".  This quantifies how the quantity that was available to be administered to the target differs from typical or background levels of the substance." ;
        <http://www.w3.org/2004/02/skos/core#prefLabel>
                "ActExposureLevelCode" .

v3-ActExposureLevelCode:LOW
        a                owl:Class ;
        rdfs:label       "low" ;
        rdfs:subClassOf  v3-ActExposureLevelCode:_ActExposureLevelCode ;
        <http://www.w3.org/2004/02/skos/core#definition>
                "Description: Exposure to an agent at a relatively low level above background." ;
        <http://www.w3.org/2004/02/skos/core#prefLabel>
                "low" .

v3-ActExposureLevelCode:
        a                owl:Ontology ;
        rdfs:comment     " A qualitative measure of the degree of exposure to the causative agent.  This includes concepts such as \"low\", \"medium\" and \"high\".  This quantifies how the quantity that was available to be administered to the target differs from typical or background levels of the substance." ;
        rdfs:label       "v3 Code System ActExposureLevelCode" ;
        owl:versionIRI   "http://hl7.org/fhir/v3/ActExposureLevelCode/2016-11-11" ;
        owl:versionInfo  "v3 Code System ActExposureLevelCode(2016-11-11)" .

v3-ActExposureLevelCode:MEDIUM
        a                owl:Class ;
        rdfs:label       "medium" ;
        rdfs:subClassOf  v3-ActExposureLevelCode:_ActExposureLevelCode ;
        <http://www.w3.org/2004/02/skos/core#definition>
                "Description: Exposure to an agent at a relatively moderate level above background.A" ;
        <http://www.w3.org/2004/02/skos/core#prefLabel>
                "medium" .
