@prefix referencerange-meaning: <http://hl7.org/fhir/referencerange-meaning/> .
@prefix fhir:  <http://hl7.org/fhir/> .
@prefix rdf:   <http://www.w3.org/1999/02/22-rdf-syntax-ns#> .
@prefix owl:   <http://www.w3.org/2002/07/owl#> .
@prefix xsd:   <http://www.w3.org/2001/XMLSchema#> .
@prefix rdfs:  <http://www.w3.org/2000/01/rdf-schema#> .
@prefix w5:    <http://hl7.org/fhir/w5#> .

referencerange-meaning:recommended
        a                owl:Class ;
        rdfs:label       "Recommended Range" ;
        rdfs:subClassOf  referencerange-meaning:type ;
        <http://www.w3.org/2004/02/skos/core#definition>
                "The range that is recommended by a relevant professional body." ;
        <http://www.w3.org/2004/02/skos/core#prefLabel>
                "Recommended Range" .

referencerange-meaning:postmeopausal
        a                owl:Class ;
        rdfs:label       "Post-Menopause" ;
        rdfs:subClassOf  referencerange-meaning:endocrine ;
        <http://www.w3.org/2004/02/skos/core#definition>
                "An expected range in an individual post-menopause." ;
        <http://www.w3.org/2004/02/skos/core#prefLabel>
                "Post-Menopause" .

referencerange-meaning:therapeutic
        a                owl:Class ;
        rdfs:label       "Therapeutic Desired Level" ;
        rdfs:subClassOf  referencerange-meaning:type ;
        <http://www.w3.org/2004/02/skos/core#definition>
                "The optimal range for best therapeutic outcomes." ;
        <http://www.w3.org/2004/02/skos/core#prefLabel>
                "Therapeutic Desired Level" .

referencerange-meaning:luteal
        a                owl:Class ;
        rdfs:label       "Luteal" ;
        rdfs:subClassOf  referencerange-meaning:endocrine ;
        <http://www.w3.org/2004/02/skos/core#definition>
                "An expected range in an individual during the luteal stage of the cycle." ;
        <http://www.w3.org/2004/02/skos/core#prefLabel>
                "Luteal" .

referencerange-meaning:midcycle
        a                owl:Class ;
        rdfs:label       "MidCycle" ;
        rdfs:subClassOf  referencerange-meaning:endocrine ;
        <http://www.w3.org/2004/02/skos/core#definition>
                "An expected range in an individual during the follicular stage of the cycle." ;
        <http://www.w3.org/2004/02/skos/core#prefLabel>
                "MidCycle" .

referencerange-meaning:pre-puberty
        a                owl:Class ;
        rdfs:label       "Pre-Puberty" ;
        rdfs:subClassOf  referencerange-meaning:endocrine ;
        <http://www.w3.org/2004/02/skos/core#definition>
                "An expected range in an individual prior to puberty." ;
        <http://www.w3.org/2004/02/skos/core#prefLabel>
                "Pre-Puberty" .

referencerange-meaning:post
        a                owl:Class ;
        rdfs:label       "Post Therapeutic Desired Level" ;
        rdfs:subClassOf  referencerange-meaning:therapeutic ;
        <http://www.w3.org/2004/02/skos/core#definition>
                "The optimal range for best therapeutic outcomes for a specimen taken immediately after administration." ;
        <http://www.w3.org/2004/02/skos/core#prefLabel>
                "Post Therapeutic Desired Level" .

referencerange-meaning:normal
        a                owl:Class ;
        rdfs:label       "Normal Range" ;
        rdfs:subClassOf  referencerange-meaning:type ;
        <http://www.w3.org/2004/02/skos/core#definition>
                "Based on 95th percentile for the relevant control population." ;
        <http://www.w3.org/2004/02/skos/core#prefLabel>
                "Normal Range" .

referencerange-meaning:pre
        a                owl:Class ;
        rdfs:label       "Pre Therapeutic Desired Level" ;
        rdfs:subClassOf  referencerange-meaning:therapeutic ;
        <http://www.w3.org/2004/02/skos/core#definition>
                "The optimal range for best therapeutic outcomes for a specimen taken immediately before administration." ;
        <http://www.w3.org/2004/02/skos/core#prefLabel>
                "Pre Therapeutic Desired Level" .

referencerange-meaning:follicular
        a                owl:Class ;
        rdfs:label       "Follicular Stage" ;
        rdfs:subClassOf  referencerange-meaning:endocrine ;
        <http://www.w3.org/2004/02/skos/core#definition>
                "An expected range in an individual during the follicular stage of the cycle." ;
        <http://www.w3.org/2004/02/skos/core#prefLabel>
                "Follicular Stage" .

referencerange-meaning:
        a                owl:Ontology ;
        rdfs:comment     "This value set defines a set of codes that can be used to indicate the meaning/use of a reference range for a particular target population." ;
        rdfs:label       "Observation Reference Range Meaning Codes" ;
        owl:versionIRI   "http://hl7.org/fhir/referencerange-meaning/3.1.0" ;
        owl:versionInfo  "Observation Reference Range Meaning Codes(3.1.0)" .

referencerange-meaning:type
        a           owl:Class ;
        rdfs:label  "Type" ;
        <http://www.w3.org/2004/02/skos/core#definition>
                "General types of reference range." ;
        <http://www.w3.org/2004/02/skos/core#prefLabel>
                "Type" .

referencerange-meaning:endocrine
        a           owl:Class ;
        rdfs:label  "Endocrine" ;
        <http://www.w3.org/2004/02/skos/core#definition>
                "Endocrine related states that change the expected value." ;
        <http://www.w3.org/2004/02/skos/core#prefLabel>
                "Endocrine" .

referencerange-meaning:treatment
        a                owl:Class ;
        rdfs:label       "Treatment Range" ;
        rdfs:subClassOf  referencerange-meaning:type ;
        <http://www.w3.org/2004/02/skos/core#definition>
                "The range at which treatment would/should be considered." ;
        <http://www.w3.org/2004/02/skos/core#prefLabel>
                "Treatment Range" .
