@prefix item-type: <http://hl7.org/fhir/item-type/> .
@prefix fhir:  <http://hl7.org/fhir/> .
@prefix rdf:   <http://www.w3.org/1999/02/22-rdf-syntax-ns#> .
@prefix owl:   <http://www.w3.org/2002/07/owl#> .
@prefix xsd:   <http://www.w3.org/2001/XMLSchema#> .
@prefix rdfs:  <http://www.w3.org/2000/01/rdf-schema#> .
@prefix w5:    <http://hl7.org/fhir/w5#> .

item-type:quantity  a    owl:Class ;
        rdfs:label       "Quantity" ;
        rdfs:subClassOf  item-type:question ;
        <http://www.w3.org/2004/02/skos/core#definition>
                "Question with a combination of a numeric value and unit, potentially with a comparator (<, >, etc.) as an answer. (valueQuantity)\nThere is an extension 'http://hl7.org/fhir/StructureDefinition/questionnaire-unit' that can be used to define what unit whould be captured (or the a unit that has a ucum conversion from the provided unit)" ;
        <http://www.w3.org/2004/02/skos/core#prefLabel>
                "Quantity" .

item-type:string  a      owl:Class ;
        rdfs:label       "String" ;
        rdfs:subClassOf  item-type:question ;
        <http://www.w3.org/2004/02/skos/core#definition>
                "Question with a short (few words to short sentence) free-text entry answer (valueString)" ;
        <http://www.w3.org/2004/02/skos/core#prefLabel>
                "String" .

item-type:date  a        owl:Class ;
        rdfs:label       "Date" ;
        rdfs:subClassOf  item-type:question ;
        <http://www.w3.org/2004/02/skos/core#definition>
                "Question with a date answer (valueDate)" ;
        <http://www.w3.org/2004/02/skos/core#prefLabel>
                "Date" .

item-type:attachment  a  owl:Class ;
        rdfs:label       "Attachment" ;
        rdfs:subClassOf  item-type:question ;
        <http://www.w3.org/2004/02/skos/core#definition>
                "Question with binary content such as a image, PDF, etc. as an answer (valueAttachment)" ;
        <http://www.w3.org/2004/02/skos/core#prefLabel>
                "Attachment" .

item-type:choice  a      owl:Class ;
        rdfs:label       "Choice" ;
        rdfs:subClassOf  item-type:question ;
        <http://www.w3.org/2004/02/skos/core#definition>
                "Question with a Coding drawn from a list of options (specified in either the option property, or via the valueset referenced in the options property) as an answer (valueCoding)" ;
        <http://www.w3.org/2004/02/skos/core#prefLabel>
                "Choice" .

item-type:decimal  a     owl:Class ;
        rdfs:label       "Decimal" ;
        rdfs:subClassOf  item-type:question ;
        <http://www.w3.org/2004/02/skos/core#definition>
                "Question with is a real number answer (valueDecimal)" ;
        <http://www.w3.org/2004/02/skos/core#prefLabel>
                "Decimal" .

item-type:boolean  a     owl:Class ;
        rdfs:label       "Boolean" ;
        rdfs:subClassOf  item-type:question ;
        <http://www.w3.org/2004/02/skos/core#definition>
                "Question with a yes/no answer (valueBoolean)" ;
        <http://www.w3.org/2004/02/skos/core#prefLabel>
                "Boolean" .

item-type:integer  a     owl:Class ;
        rdfs:label       "Integer" ;
        rdfs:subClassOf  item-type:question ;
        <http://www.w3.org/2004/02/skos/core#definition>
                "Question with an integer answer (valueInteger)" ;
        <http://www.w3.org/2004/02/skos/core#prefLabel>
                "Integer" .

item-type:open-choice
        a                owl:Class ;
        rdfs:label       "Open Choice" ;
        rdfs:subClassOf  item-type:question ;
        <http://www.w3.org/2004/02/skos/core#definition>
                "Answer is a Coding drawn from a list of options (as with the choice type) or a free-text entry in a string (valueCoding or valueString)" ;
        <http://www.w3.org/2004/02/skos/core#prefLabel>
                "Open Choice" .

item-type:  a            owl:Ontology ;
        rdfs:comment     "Distinguishes groups from questions and display text and indicates data type for questions" ;
        rdfs:label       "QuestionnaireItemType" ;
        owl:versionIRI   "http://hl7.org/fhir/item-type/3.1.0" ;
        owl:versionInfo  "QuestionnaireItemType(3.1.0)" .

item-type:display  a  owl:Class ;
        rdfs:label  "Display" ;
        <http://www.w3.org/2004/02/skos/core#definition>
                "Text for display that will not capture an answer or have child items." ;
        <http://www.w3.org/2004/02/skos/core#prefLabel>
                "Display" .

item-type:text  a        owl:Class ;
        rdfs:label       "Text" ;
        rdfs:subClassOf  item-type:question ;
        <http://www.w3.org/2004/02/skos/core#definition>
                "Question with a long (potentially multi-paragraph) free-text entry answer (valueString)" ;
        <http://www.w3.org/2004/02/skos/core#prefLabel>
                "Text" .

item-type:time  a        owl:Class ;
        rdfs:label       "Time" ;
        rdfs:subClassOf  item-type:question ;
        <http://www.w3.org/2004/02/skos/core#definition>
                "Question with a time (hour:minute:second) answer independent of date. (valueTime)" ;
        <http://www.w3.org/2004/02/skos/core#prefLabel>
                "Time" .

item-type:dateTime  a    owl:Class ;
        rdfs:label       "Date Time" ;
        rdfs:subClassOf  item-type:question ;
        <http://www.w3.org/2004/02/skos/core#definition>
                "Question with a date and time answer (valueDateTime)" ;
        <http://www.w3.org/2004/02/skos/core#prefLabel>
                "Date Time" .

item-type:group  a  owl:Class ;
        rdfs:label  "Group" ;
        <http://www.w3.org/2004/02/skos/core#definition>
                "An item with no direct answer but should have at least one child item." ;
        <http://www.w3.org/2004/02/skos/core#prefLabel>
                "Group" .

item-type:url  a         owl:Class ;
        rdfs:label       "Url" ;
        rdfs:subClassOf  item-type:question ;
        <http://www.w3.org/2004/02/skos/core#definition>
                "Question with a URL (website, FTP site, etc.) answer (valueUri)" ;
        <http://www.w3.org/2004/02/skos/core#prefLabel>
                "Url" .

item-type:question  a  owl:Class ;
        rdfs:label  "Question" ;
        <http://www.w3.org/2004/02/skos/core#definition>
                "An item that defines a specific answer to be captured, and may have child items.\n(the answer provided in the QuestionnaireResponse should be of the defined datatype)" ;
        <http://www.w3.org/2004/02/skos/core#prefLabel>
                "Question" .

item-type:reference  a   owl:Class ;
        rdfs:label       "Reference" ;
        rdfs:subClassOf  item-type:question ;
        <http://www.w3.org/2004/02/skos/core#definition>
                "Question with a reference to another resource (practitioner, organization, etc.) as an answer (valueReference)" ;
        <http://www.w3.org/2004/02/skos/core#prefLabel>
                "Reference" .
