@prefix fhir:  <http://hl7.org/fhir/> .
@prefix rdf:   <http://www.w3.org/1999/02/22-rdf-syntax-ns#> .
@prefix owl:   <http://www.w3.org/2002/07/owl#> .
@prefix xsd:   <http://www.w3.org/2001/XMLSchema#> .
@prefix rdfs:  <http://www.w3.org/2000/01/rdf-schema#> .
@prefix condition-clinical: <http://hl7.org/fhir/condition-clinical/> .
@prefix w5:    <http://hl7.org/fhir/w5#> .

condition-clinical:remission
        a                owl:Class ;
        rdfs:label       "Remission" ;
        rdfs:subClassOf  condition-clinical:inactive ;
        <http://www.w3.org/2004/02/skos/core#definition>
                "The subject is no longer experiencing the symptoms of the condition, but there is a risk of the symptoms returning." ;
        <http://www.w3.org/2004/02/skos/core#prefLabel>
                "Remission" .

condition-clinical:well-controlled
        a                owl:Class ;
        rdfs:label       "Well-Controlled" ;
        rdfs:subClassOf  condition-clinical:active ;
        <http://www.w3.org/2004/02/skos/core#definition>
                "The subject's condition is adequately or well managed such that the recommended evidence-based clinical outcome targets are met." ;
        <http://www.w3.org/2004/02/skos/core#prefLabel>
                "Well-Controlled" .

condition-clinical:poorly-controlled
        a                owl:Class ;
        rdfs:label       "Poorly-Controlled" ;
        rdfs:subClassOf  condition-clinical:active ;
        <http://www.w3.org/2004/02/skos/core#definition>
                "The subject's condition is inadequately/poorly managed such that the recommended evidence-based clinical outcome targets are not met." ;
        <http://www.w3.org/2004/02/skos/core#prefLabel>
                "Poorly-Controlled" .

condition-clinical:active
        a           owl:Class ;
        rdfs:label  "Active" ;
        <http://www.w3.org/2004/02/skos/core#definition>
                "The subject is currently experiencing the symptoms of the condition or there is evidence of the condition." ;
        <http://www.w3.org/2004/02/skos/core#prefLabel>
                "Active" .

condition-clinical:  a   owl:Ontology ;
        rdfs:comment     "Preferred value set for Condition Clinical Status." ;
        rdfs:label       "Condition Clinical Status Codes" ;
        owl:versionIRI   "http://hl7.org/fhir/condition-clinical/3.1.0" ;
        owl:versionInfo  "Condition Clinical Status Codes(3.1.0)" .

condition-clinical:resolved
        a                owl:Class ;
        rdfs:label       "Resolved" ;
        rdfs:subClassOf  condition-clinical:inactive ;
        <http://www.w3.org/2004/02/skos/core#definition>
                "The subject is no longer experiencing the symptoms of the condition and there is a negligible perceived risk of the symptoms returning." ;
        <http://www.w3.org/2004/02/skos/core#prefLabel>
                "Resolved" .

condition-clinical:relapse
        a                owl:Class ;
        rdfs:label       "Relapse" ;
        rdfs:subClassOf  condition-clinical:active ;
        <http://www.w3.org/2004/02/skos/core#definition>
                "The subject is experiencing a return of a condition, or signs and symptoms after a period of improvement or remission, e.g. relapse of cancer, multiple sclerosis, rheumatoid arthritis, systemic lupus erythematosus, bipolar disorder, [psychotic relapse of] schizophrenia, etc." ;
        <http://www.w3.org/2004/02/skos/core#prefLabel>
                "Relapse" .

condition-clinical:inactive
        a           owl:Class ;
        rdfs:label  "Inactive" ;
        <http://www.w3.org/2004/02/skos/core#definition>
                "The subject is no longer experiencing the symptoms of the condition or there is no longer evidence of the condition." ;
        <http://www.w3.org/2004/02/skos/core#prefLabel>
                "Inactive" .

condition-clinical:recurrence
        a                owl:Class ;
        rdfs:label       "Recurrence" ;
        rdfs:subClassOf  condition-clinical:active ;
        <http://www.w3.org/2004/02/skos/core#definition>
                "The subject is experiencing a re-occurence or repeating of a previously resolved condition, e.g. urinary tract infection, pancreatitis, cholangitis, conjunctivitis." ;
        <http://www.w3.org/2004/02/skos/core#prefLabel>
                "Recurrence" .
