@prefix fhir:  <http://hl7.org/fhir/> .
@prefix rdf:   <http://www.w3.org/1999/02/22-rdf-syntax-ns#> .
@prefix owl:   <http://www.w3.org/2002/07/owl#> .
@prefix xsd:   <http://www.w3.org/2001/XMLSchema#> .
@prefix issue-type: <http://hl7.org/fhir/issue-type/> .
@prefix rdfs:  <http://www.w3.org/2000/01/rdf-schema#> .
@prefix w5:    <http://hl7.org/fhir/w5#> .

issue-type:suppressed
        a                owl:Class ;
        rdfs:label       "Information  Suppressed" ;
        rdfs:subClassOf  issue-type:security ;
        <http://www.w3.org/2004/02/skos/core#definition>
                "Some information was not or may not have been returned due to business rules, consent or privacy rules, or access permission constraints.  This information may be accessible through alternate processes." ;
        <http://www.w3.org/2004/02/skos/core#prefLabel>
                "Information  Suppressed" .

issue-type:security  a  owl:Class ;
        rdfs:label  "Security Problem" ;
        <http://www.w3.org/2004/02/skos/core#definition>
                "An authentication/authorization/permissions issue of some kind." ;
        <http://www.w3.org/2004/02/skos/core#prefLabel>
                "Security Problem" .

issue-type:timeout  a    owl:Class ;
        rdfs:label       "Timeout" ;
        rdfs:subClassOf  issue-type:transient ;
        <http://www.w3.org/2004/02/skos/core#definition>
                "An internal timeout has occurred." ;
        <http://www.w3.org/2004/02/skos/core#prefLabel>
                "Timeout" .

issue-type:processing
        a           owl:Class ;
        rdfs:label  "Processing Failure" ;
        <http://www.w3.org/2004/02/skos/core#definition>
                "Processing issues. These are expected to be final e.g. there is no point resubmitting the same content unchanged." ;
        <http://www.w3.org/2004/02/skos/core#prefLabel>
                "Processing Failure" .

issue-type:business-rule
        a                owl:Class ;
        rdfs:label       "Business Rule Violation" ;
        rdfs:subClassOf  issue-type:processing ;
        <http://www.w3.org/2004/02/skos/core#definition>
                "The content/operation failed to pass some business rule, and so could not proceed." ;
        <http://www.w3.org/2004/02/skos/core#prefLabel>
                "Business Rule Violation" .

issue-type:too-costly
        a                owl:Class ;
        rdfs:label       "Operation Too Costly" ;
        rdfs:subClassOf  issue-type:processing ;
        <http://www.w3.org/2004/02/skos/core#definition>
                "The operation was stopped to protect server resources; e.g. a request for a value set expansion on all of SNOMED CT." ;
        <http://www.w3.org/2004/02/skos/core#prefLabel>
                "Operation Too Costly" .

issue-type:login  a      owl:Class ;
        rdfs:label       "Login Required" ;
        rdfs:subClassOf  issue-type:security ;
        <http://www.w3.org/2004/02/skos/core#definition>
                "The client needs to initiate an authentication process." ;
        <http://www.w3.org/2004/02/skos/core#prefLabel>
                "Login Required" .

issue-type:lock-error
        a                owl:Class ;
        rdfs:label       "Lock Error" ;
        rdfs:subClassOf  issue-type:transient ;
        <http://www.w3.org/2004/02/skos/core#definition>
                "A resource/record locking failure (usually in an underlying database)." ;
        <http://www.w3.org/2004/02/skos/core#prefLabel>
                "Lock Error" .

issue-type:expired  a    owl:Class ;
        rdfs:label       "Session Expired" ;
        rdfs:subClassOf  issue-type:security ;
        <http://www.w3.org/2004/02/skos/core#definition>
                "User session expired; a login may be required." ;
        <http://www.w3.org/2004/02/skos/core#prefLabel>
                "Session Expired" .

issue-type:not-found  a  owl:Class ;
        rdfs:label       "Not Found" ;
        rdfs:subClassOf  issue-type:processing ;
        <http://www.w3.org/2004/02/skos/core#definition>
                "The reference provided was not found. In a pure RESTful environment, this would be an HTTP 404 error, but this code may be used where the content is not found further into the application architecture." ;
        <http://www.w3.org/2004/02/skos/core#prefLabel>
                "Not Found" .

issue-type:too-long  a   owl:Class ;
        rdfs:label       "Content Too Long" ;
        rdfs:subClassOf  issue-type:processing ;
        <http://www.w3.org/2004/02/skos/core#definition>
                "Provided content is too long (typically, this is a denial of service protection type of error)." ;
        <http://www.w3.org/2004/02/skos/core#prefLabel>
                "Content Too Long" .

issue-type:not-supported
        a                owl:Class ;
        rdfs:label       "Content not supported" ;
        rdfs:subClassOf  issue-type:processing ;
        <http://www.w3.org/2004/02/skos/core#definition>
                "The resource or profile is not supported." ;
        <http://www.w3.org/2004/02/skos/core#prefLabel>
                "Content not supported" .

issue-type:exception  a  owl:Class ;
        rdfs:label       "Exception" ;
        rdfs:subClassOf  issue-type:transient ;
        <http://www.w3.org/2004/02/skos/core#definition>
                "An unexpected internal error has occurred." ;
        <http://www.w3.org/2004/02/skos/core#prefLabel>
                "Exception" .

issue-type:duplicate  a  owl:Class ;
        rdfs:label       "Duplicate" ;
        rdfs:subClassOf  issue-type:processing ;
        <http://www.w3.org/2004/02/skos/core#definition>
                "An attempt was made to create a duplicate record." ;
        <http://www.w3.org/2004/02/skos/core#prefLabel>
                "Duplicate" .

issue-type:no-store  a   owl:Class ;
        rdfs:label       "No Store Available" ;
        rdfs:subClassOf  issue-type:transient ;
        <http://www.w3.org/2004/02/skos/core#definition>
                "The persistent store is unavailable; e.g. the database is down for maintenance or similar action." ;
        <http://www.w3.org/2004/02/skos/core#prefLabel>
                "No Store Available" .

issue-type:invalid  a  owl:Class ;
        rdfs:label  "Invalid Content" ;
        <http://www.w3.org/2004/02/skos/core#definition>
                "Content invalid against the specification or a profile." ;
        <http://www.w3.org/2004/02/skos/core#prefLabel>
                "Invalid Content" .

issue-type:invariant  a  owl:Class ;
        rdfs:label       "Validation rule failed" ;
        rdfs:subClassOf  issue-type:invalid ;
        <http://www.w3.org/2004/02/skos/core#definition>
                "A content validation rule failed - e.g. a schematron rule." ;
        <http://www.w3.org/2004/02/skos/core#prefLabel>
                "Validation rule failed" .

issue-type:informational
        a           owl:Class ;
        rdfs:label  "Informational Note" ;
        <http://www.w3.org/2004/02/skos/core#definition>
                "A message unrelated to the processing success of the completed operation (examples of the latter include things like reminders of password expiry, system maintenance times, etc.)." ;
        <http://www.w3.org/2004/02/skos/core#prefLabel>
                "Informational Note" .

issue-type:unknown  a    owl:Class ;
        rdfs:label       "Unknown User" ;
        rdfs:subClassOf  issue-type:security ;
        <http://www.w3.org/2004/02/skos/core#definition>
                "The user or system was not able to be authenticated (either there is no process, or the proferred token is unacceptable)." ;
        <http://www.w3.org/2004/02/skos/core#prefLabel>
                "Unknown User" .

issue-type:incomplete
        a                owl:Class ;
        rdfs:label       "Incomplete Results" ;
        rdfs:subClassOf  issue-type:processing ;
        <http://www.w3.org/2004/02/skos/core#definition>
                "Not all data sources typically accessed could be reached, or responded in time, so the returned information may not be complete." ;
        <http://www.w3.org/2004/02/skos/core#prefLabel>
                "Incomplete Results" .

issue-type:value  a      owl:Class ;
        rdfs:label       "Element value invalid" ;
        rdfs:subClassOf  issue-type:invalid ;
        <http://www.w3.org/2004/02/skos/core#definition>
                "An element value is invalid." ;
        <http://www.w3.org/2004/02/skos/core#prefLabel>
                "Element value invalid" .

issue-type:throttled  a  owl:Class ;
        rdfs:label       "Throttled" ;
        rdfs:subClassOf  issue-type:transient ;
        <http://www.w3.org/2004/02/skos/core#definition>
                "The system is not prepared to handle this request due to load management." ;
        <http://www.w3.org/2004/02/skos/core#prefLabel>
                "Throttled" .

issue-type:forbidden  a  owl:Class ;
        rdfs:label       "Forbidden" ;
        rdfs:subClassOf  issue-type:security ;
        <http://www.w3.org/2004/02/skos/core#definition>
                "The user does not have the rights to perform this action." ;
        <http://www.w3.org/2004/02/skos/core#prefLabel>
                "Forbidden" .

issue-type:structure  a  owl:Class ;
        rdfs:label       "Structural Issue" ;
        rdfs:subClassOf  issue-type:invalid ;
        <http://www.w3.org/2004/02/skos/core#definition>
                "A structural issue in the content such as wrong namespace, or unable to parse the content completely, or invalid json syntax." ;
        <http://www.w3.org/2004/02/skos/core#prefLabel>
                "Structural Issue" .

issue-type:  a           owl:Ontology ;
        rdfs:comment     "A code that describes the type of issue." ;
        rdfs:label       "IssueType" ;
        owl:versionIRI   "http://hl7.org/fhir/issue-type/3.1.0" ;
        owl:versionInfo  "IssueType(3.1.0)" .

issue-type:required  a   owl:Class ;
        rdfs:label       "Required element missing" ;
        rdfs:subClassOf  issue-type:invalid ;
        <http://www.w3.org/2004/02/skos/core#definition>
                "A required element is missing." ;
        <http://www.w3.org/2004/02/skos/core#prefLabel>
                "Required element missing" .

issue-type:transient  a  owl:Class ;
        rdfs:label  "Transient Issue" ;
        <http://www.w3.org/2004/02/skos/core#definition>
                "Transient processing issues. The system receiving the error may be able to resubmit the same content once an underlying issue is resolved." ;
        <http://www.w3.org/2004/02/skos/core#prefLabel>
                "Transient Issue" .

issue-type:code-invalid
        a                owl:Class ;
        rdfs:label       "Invalid Code" ;
        rdfs:subClassOf  issue-type:processing ;
        <http://www.w3.org/2004/02/skos/core#definition>
                "The code or system could not be understood, or it was not valid in the context of a particular ValueSet.code." ;
        <http://www.w3.org/2004/02/skos/core#prefLabel>
                "Invalid Code" .

issue-type:conflict  a   owl:Class ;
        rdfs:label       "Edit Version Conflict" ;
        rdfs:subClassOf  issue-type:processing ;
        <http://www.w3.org/2004/02/skos/core#definition>
                "Content could not be accepted because of an edit conflict (i.e. version aware updates) (In a pure RESTful environment, this would be an HTTP 404 error, but this code may be used where the conflict is discovered further into the application architecture.)" ;
        <http://www.w3.org/2004/02/skos/core#prefLabel>
                "Edit Version Conflict" .

issue-type:extension  a  owl:Class ;
        rdfs:label       "Unacceptable Extension" ;
        rdfs:subClassOf  issue-type:processing ;
        <http://www.w3.org/2004/02/skos/core#definition>
                "An extension was found that was not acceptable, could not be resolved, or a modifierExtension was not recognized." ;
        <http://www.w3.org/2004/02/skos/core#prefLabel>
                "Unacceptable Extension" .
