@prefix v3-RoleLinkStatus: <http://hl7.org/fhir/v3/RoleLinkStatus/> .
@prefix fhir:  <http://hl7.org/fhir/> .
@prefix rdf:   <http://www.w3.org/1999/02/22-rdf-syntax-ns#> .
@prefix owl:   <http://www.w3.org/2002/07/owl#> .
@prefix xsd:   <http://www.w3.org/2001/XMLSchema#> .
@prefix rdfs:  <http://www.w3.org/2000/01/rdf-schema#> .
@prefix w5:    <http://hl7.org/fhir/w5#> .

v3-RoleLinkStatus:NULLIFIED
        a           owl:Class ;
        rdfs:label  "nullified" ;
        <http://www.w3.org/2004/02/skos/core#definition>
                "Description: The state representing the termination of a RoleLink instance that was created in error." ;
        <http://www.w3.org/2004/02/skos/core#prefLabel>
                "nullified" .

v3-RoleLinkStatus:CANCELLED
        a                owl:Class ;
        rdfs:label       "cancelled" ;
        rdfs:subClassOf  v3-RoleLinkStatus:NORMAL ;
        <http://www.w3.org/2004/02/skos/core#definition>
                "Description: The terminal state resulting from abandoning the RoleLink prior to or after activation." ;
        <http://www.w3.org/2004/02/skos/core#prefLabel>
                "cancelled" .

v3-RoleLinkStatus:COMPLETED
        a                owl:Class ;
        rdfs:label       "completed" ;
        rdfs:subClassOf  v3-RoleLinkStatus:NORMAL ;
        <http://www.w3.org/2004/02/skos/core#definition>
                "Description: The terminal state representing the successful completion of the RoleLink." ;
        <http://www.w3.org/2004/02/skos/core#prefLabel>
                "completed" .

v3-RoleLinkStatus:NORMAL
        a           owl:Class ;
        rdfs:label  "normal" ;
        <http://www.w3.org/2004/02/skos/core#definition>
                "Description: The 'typical' state. Excludes \"nullified\" which represents the termination state of a RoleLink instance that was created in error." ;
        <http://www.w3.org/2004/02/skos/core#prefLabel>
                "normal" .

v3-RoleLinkStatus:PENDING
        a                owl:Class ;
        rdfs:label       "pending" ;
        rdfs:subClassOf  v3-RoleLinkStatus:NORMAL ;
        <http://www.w3.org/2004/02/skos/core#definition>
                "Description: The state indicates the RoleLink has not yet become active." ;
        <http://www.w3.org/2004/02/skos/core#prefLabel>
                "pending" .

v3-RoleLinkStatus:  a    owl:Ontology ;
        rdfs:comment     "  Description:\r\nCodes representing possible states of a RoleLink, as defined by the RoleLink class state machine." ;
        rdfs:label       "v3 Code System RoleLinkStatus" ;
        owl:versionIRI   "http://hl7.org/fhir/v3/RoleLinkStatus/2016-11-11" ;
        owl:versionInfo  "v3 Code System RoleLinkStatus(2016-11-11)" .

v3-RoleLinkStatus:ACTIVE
        a                owl:Class ;
        rdfs:label       "active" ;
        rdfs:subClassOf  v3-RoleLinkStatus:NORMAL ;
        <http://www.w3.org/2004/02/skos/core#definition>
                "Description: The state indicates the RoleLink is in progress." ;
        <http://www.w3.org/2004/02/skos/core#prefLabel>
                "active" .
