@prefix v3-EntityCode: <http://hl7.org/fhir/v3/EntityCode/> .
@prefix fhir:  <http://hl7.org/fhir/> .
@prefix rdf:   <http://www.w3.org/1999/02/22-rdf-syntax-ns#> .
@prefix owl:   <http://www.w3.org/2002/07/owl#> .
@prefix xsd:   <http://www.w3.org/2001/XMLSchema#> .
@prefix rdfs:  <http://www.w3.org/2000/01/rdf-schema#> .
@prefix w5:    <http://hl7.org/fhir/w5#> .

v3-EntityCode:CHLTM  a   owl:Class ;
        rdfs:label       "Chlamydia transport medium" ;
        rdfs:subClassOf  v3-EntityCode:_SpecimenAdditiveEntity ;
        <http://www.w3.org/2004/02/skos/core#definition>
                "Any of a number of non-nutritive buffered media used to maintain Chlamydia viability during transportation to the laboratory" ;
        <http://www.w3.org/2004/02/skos/core#prefLabel>
                "Chlamydia transport medium" .

v3-EntityCode:VCCNE  a   owl:Class ;
        rdfs:label       "Vaccine" ;
        rdfs:subClassOf  v3-EntityCode:_MaterialEntityClassType ;
        <http://www.w3.org/2004/02/skos/core#definition>
                "A Type of medicine that creates an immune protection without the recipient experiencing the disease." ;
        <http://www.w3.org/2004/02/skos/core#prefLabel>
                "Vaccine" .

v3-EntityCode:NDA02  a   owl:Class ;
        rdfs:label       "fish" ;
        rdfs:subClassOf  v3-EntityCode:_NonDrugAgentEntity ;
        <http://www.w3.org/2004/02/skos/core#definition>
                "fish" ;
        <http://www.w3.org/2004/02/skos/core#prefLabel>
                "fish" .

v3-EntityCode:NDA15  a   owl:Class ;
        rdfs:label       "tomatoes" ;
        rdfs:subClassOf  v3-EntityCode:_NonDrugAgentEntity ;
        <http://www.w3.org/2004/02/skos/core#definition>
                "tomatoes" ;
        <http://www.w3.org/2004/02/skos/core#prefLabel>
                "tomatoes" .

v3-EntityCode:BACTM  a   owl:Class ;
        rdfs:label       "Bacterial Transport medium" ;
        rdfs:subClassOf  v3-EntityCode:_SpecimenAdditiveEntity ;
        <http://www.w3.org/2004/02/skos/core#definition>
                "Any medium used to maintain bacterial viability (e.g. Stuart's, Cary-Blair, Amies)" ;
        <http://www.w3.org/2004/02/skos/core#prefLabel>
                "Bacterial Transport medium" .

v3-EntityCode:CARS  a    owl:Class ;
        rdfs:label       "Carson's Modified 10% formalin" ;
        rdfs:subClassOf  v3-EntityCode:_SpecimenAdditiveEntity ;
        <http://www.w3.org/2004/02/skos/core#definition>
                "A modification of buffered 10% formalin used as a general tissue preservative." ;
        <http://www.w3.org/2004/02/skos/core#prefLabel>
                "Carson's Modified 10% formalin" .

v3-EntityCode:SILICA  a  owl:Class ;
        rdfs:label       "Siliceous earth" ;
        rdfs:subClassOf  v3-EntityCode:_SpecimenAdditiveEntity ;
        <http://www.w3.org/2004/02/skos/core#definition>
                "Diatomaceous earth. For glucose determination blood samples" ;
        <http://www.w3.org/2004/02/skos/core#prefLabel>
                "Siliceous earth" .

v3-EntityCode:SYR  a     owl:Class ;
        rdfs:label       "Syringe" ;
        rdfs:subClassOf  v3-EntityCode:_InjectionMedicalDevice ;
        <http://www.w3.org/2004/02/skos/core#definition>
                "A barrel with a plunger." ;
        <http://www.w3.org/2004/02/skos/core#prefLabel>
                "Syringe" .

v3-EntityCode:MMDTM  a   owl:Class ;
        rdfs:label       "MMD transport medium" ;
        rdfs:subClassOf  v3-EntityCode:_SpecimenAdditiveEntity ;
        <http://www.w3.org/2004/02/skos/core#definition>
                "A buffered medium with ammonium sulfate added to preserve antigens for Immunofluorescence procedures" ;
        <http://www.w3.org/2004/02/skos/core#prefLabel>
                "MMD transport medium" .

v3-EntityCode:M4  a      owl:Class ;
        rdfs:label       "M4" ;
        rdfs:subClassOf  v3-EntityCode:_SpecimenAdditiveEntity ;
        <http://www.w3.org/2004/02/skos/core#definition>
                "Modified Hank's balanced salt solution supplemented with bovine serum albumin, gelatin, sucrose and glutamic acid. It is buffered to pH 7.3+ or - 0.2 with HEPES buffer. Phenol red is used to indicate pH. Vancomycin, Amphotericin B and Colistin are used to" ;
        <http://www.w3.org/2004/02/skos/core#prefLabel>
                "M4" .

v3-EntityCode:BF10  a    owl:Class ;
        rdfs:label       "Buffered 10% formalin" ;
        rdfs:subClassOf  v3-EntityCode:_SpecimenAdditiveEntity ;
        <http://www.w3.org/2004/02/skos/core#definition>
                "Formaldehyde 4% w/v; methyl alcohol 1% w/v; phosphate buffering salts. Tissue preservative" ;
        <http://www.w3.org/2004/02/skos/core#prefLabel>
                "Buffered 10% formalin" .

v3-EntityCode:_IndividualPackageEntityType
        a                owl:Class ;
        rdfs:label       "IndividualPackageEntityType" ;
        rdfs:subClassOf  v3-EntityCode:_RigidContainerEntityType ;
        <http://www.w3.org/2004/02/skos/core#definition>
                "Container intended to contain sufficient material for only one use." ;
        <http://www.w3.org/2004/02/skos/core#prefLabel>
                "IndividualPackageEntityType" .

v3-EntityCode:OVUL  a    owl:Class ;
        rdfs:label       "Ovule" ;
        rdfs:subClassOf  v3-EntityCode:_IndividualPackageEntityType ;
        <http://www.w3.org/2004/02/skos/core#definition>
                "A container either glass or plastic and a narrow neck, for storing liquid." ;
        <http://www.w3.org/2004/02/skos/core#prefLabel>
                "Ovule" .

v3-EntityCode:VIAL  a    owl:Class ;
        rdfs:label       "Vial" ;
        rdfs:subClassOf  v3-EntityCode:_MultiUseContainerEntityType ;
        <http://www.w3.org/2004/02/skos/core#definition>
                "A small cylindrical glass for holding liquid medicines." ;
        <http://www.w3.org/2004/02/skos/core#prefLabel>
                "Vial" .

v3-EntityCode:FLOOR  a   owl:Class ;
        rdfs:label       "Floor Location" ;
        rdfs:subClassOf  v3-EntityCode:_PlaceEntityType ;
        <http://www.w3.org/2004/02/skos/core#definition>
                "The location of a floor of a building" ;
        <http://www.w3.org/2004/02/skos/core#prefLabel>
                "Floor Location" .

v3-EntityCode:JUG  a     owl:Class ;
        rdfs:label       "Jug" ;
        rdfs:subClassOf  v3-EntityCode:_MultiUseContainerEntityType ;
        <http://www.w3.org/2004/02/skos/core#definition>
                "A deep vessel  for holding liquids, with a handle and often with a spout or lip shape for pouring." ;
        <http://www.w3.org/2004/02/skos/core#prefLabel>
                "Jug" .

v3-EntityCode:BOX  a     owl:Class ;
        rdfs:label       "Box" ;
        rdfs:subClassOf  v3-EntityCode:_MultiUseContainerEntityType ;
        <http://www.w3.org/2004/02/skos/core#definition>
                "A 6-sided container commonly made from paper or cardboard used for solid forms." ;
        <http://www.w3.org/2004/02/skos/core#prefLabel>
                "Box" .

v3-EntityCode:INH  a     owl:Class ;
        rdfs:label       "Inhaler" ;
        rdfs:subClassOf  v3-EntityCode:_AdministrationMedicalDevice ;
        <http://www.w3.org/2004/02/skos/core#definition>
                "A small device used for inhaling medicine in the form of a vapour or gas in order to ease a respiratory condition such as asthma or to relieve nasal congestion." ;
        <http://www.w3.org/2004/02/skos/core#prefLabel>
                "Inhaler" .

v3-EntityCode:NDA07  a   owl:Class ;
        rdfs:label       "wheat or gluten" ;
        rdfs:subClassOf  v3-EntityCode:_NonDrugAgentEntity ;
        <http://www.w3.org/2004/02/skos/core#definition>
                "wheat or gluten" ;
        <http://www.w3.org/2004/02/skos/core#prefLabel>
                "wheat or gluten" .

v3-EntityCode:SYSTM  a   owl:Class ;
        rdfs:label       "System" ;
        rdfs:subClassOf  v3-EntityCode:KIT ;
        <http://www.w3.org/2004/02/skos/core#definition>
                "A kit in which the components are interconnected." ;
        <http://www.w3.org/2004/02/skos/core#prefLabel>
                "System" .

v3-EntityCode:THROM  a   owl:Class ;
        rdfs:label       "Thrombin" ;
        rdfs:subClassOf  v3-EntityCode:_SpecimenAdditiveEntity ;
        <http://www.w3.org/2004/02/skos/core#definition>
                "Thrombin. Accelerates clotting." ;
        <http://www.w3.org/2004/02/skos/core#prefLabel>
                "Thrombin" .

v3-EntityCode:BED  a     owl:Class ;
        rdfs:label       "Bed Location" ;
        rdfs:subClassOf  v3-EntityCode:_PlaceEntityType ;
        <http://www.w3.org/2004/02/skos/core#definition>
                "The location of a bed" ;
        <http://www.w3.org/2004/02/skos/core#prefLabel>
                "Bed Location" .

v3-EntityCode:ENT  a     owl:Class ;
        rdfs:label       "Enteric bacteria transport medium" ;
        rdfs:subClassOf  v3-EntityCode:_SpecimenAdditiveEntity ;
        <http://www.w3.org/2004/02/skos/core#definition>
                "Any of a number of non-nutritive buffered media used to maintain enteric bacterial viability during transportation to the laboratory" ;
        <http://www.w3.org/2004/02/skos/core#prefLabel>
                "Enteric bacteria transport medium" .

v3-EntityCode:FL100  a   owl:Class ;
        rdfs:label       "Sodium Fluoride, 100mg" ;
        rdfs:subClassOf  v3-EntityCode:_SpecimenAdditiveEntity ;
        <http://www.w3.org/2004/02/skos/core#definition>
                "Sodium fluoride, 100mg added as a urine preservative." ;
        <http://www.w3.org/2004/02/skos/core#prefLabel>
                "Sodium Fluoride, 100mg" .

v3-EntityCode:BOR  a     owl:Class ;
        rdfs:label       "Boric Acid" ;
        rdfs:subClassOf  v3-EntityCode:_SpecimenAdditiveEntity ;
        <http://www.w3.org/2004/02/skos/core#definition>
                "Powdered boric acid (usually 10 g) added to 24-hour urine collections as a preservative." ;
        <http://www.w3.org/2004/02/skos/core#prefLabel>
                "Boric Acid" .

v3-EntityCode:DIALPK  a  owl:Class ;
        rdfs:label       "Dial Pack" ;
        rdfs:subClassOf  v3-EntityCode:COMPPKG ;
        <http://www.w3.org/2004/02/skos/core#definition>
                "Rotatable dispenser.  Eg. Birth control package." ;
        <http://www.w3.org/2004/02/skos/core#prefLabel>
                "Dial Pack" .

v3-EntityCode:CAN  a     owl:Class ;
        rdfs:label       "Can" ;
        rdfs:subClassOf  v3-EntityCode:_MultiUseContainerEntityType ;
        <http://www.w3.org/2004/02/skos/core#definition>
                "A metal container in which a material is hermetically sealed to enable storage over long periods." ;
        <http://www.w3.org/2004/02/skos/core#prefLabel>
                "Can" .

v3-EntityCode:APLCTR  a  owl:Class ;
        rdfs:label       "Applicator" ;
        rdfs:subClassOf  v3-EntityCode:_AdministrationMedicalDevice ;
        <http://www.w3.org/2004/02/skos/core#definition>
                "A device used to apply a liquid or powder to a surface." ;
        <http://www.w3.org/2004/02/skos/core#prefLabel>
                "Applicator" .

v3-EntityCode:BLDG  a    owl:Class ;
        rdfs:label       "Building Location" ;
        rdfs:subClassOf  v3-EntityCode:_PlaceEntityType ;
        <http://www.w3.org/2004/02/skos/core#definition>
                "The location of a building" ;
        <http://www.w3.org/2004/02/skos/core#prefLabel>
                "Building Location" .

v3-EntityCode:NAF  a     owl:Class ;
        rdfs:label       "Sodium Fluoride" ;
        rdfs:subClassOf  v3-EntityCode:_SpecimenAdditiveEntity ;
        <http://www.w3.org/2004/02/skos/core#definition>
                "Sodium fluoride" ;
        <http://www.w3.org/2004/02/skos/core#prefLabel>
                "Sodium Fluoride" .

v3-EntityCode:STRIP  a   owl:Class ;
        rdfs:label       "Strip" ;
        rdfs:subClassOf  v3-EntityCode:COMPPKG ;
        <http://www.w3.org/2004/02/skos/core#definition>
                "A continuous strip of plastic sectioned into individual pouches, each one containing the quantity of 1 or more medications intended to be administered at a specific time" ;
        <http://www.w3.org/2004/02/skos/core#prefLabel>
                "Strip" .

v3-EntityCode:NDA01  a   owl:Class ;
        rdfs:label       "egg" ;
        rdfs:subClassOf  v3-EntityCode:_NonDrugAgentEntity ;
        <http://www.w3.org/2004/02/skos/core#definition>
                "egg" ;
        <http://www.w3.org/2004/02/skos/core#prefLabel>
                "egg" .

v3-EntityCode:NDA14  a   owl:Class ;
        rdfs:label       "strawberries" ;
        rdfs:subClassOf  v3-EntityCode:_NonDrugAgentEntity ;
        <http://www.w3.org/2004/02/skos/core#definition>
                "strawberries" ;
        <http://www.w3.org/2004/02/skos/core#prefLabel>
                "strawberries" .

v3-EntityCode:THYMOL  a  owl:Class ;
        rdfs:label       "Thymol" ;
        rdfs:subClassOf  v3-EntityCode:_SpecimenAdditiveEntity ;
        <http://www.w3.org/2004/02/skos/core#definition>
                "2-Isopropyl-5-methyl phenol. A preservative for 24 Hr Urine samples" ;
        <http://www.w3.org/2004/02/skos/core#prefLabel>
                "Thymol" .

v3-EntityCode:KIT  a     owl:Class ;
        rdfs:label       "Kit" ;
        rdfs:subClassOf  v3-EntityCode:PKG ;
        <http://www.w3.org/2004/02/skos/core#definition>
                "A container for a diverse collection of products intended to be used together for some purpose (e.g. Medicinal kits often contain a syringe, a needle and the injectable medication)." ;
        <http://www.w3.org/2004/02/skos/core#prefLabel>
                "Kit" .

v3-EntityCode:DSKUNH  a  owl:Class ;
        rdfs:label       "Diskhaler" ;
        rdfs:subClassOf  v3-EntityCode:INH ;
        <http://www.w3.org/2004/02/skos/core#definition>
                "The device used to inhale the doses of medication contained in the disk form." ;
        <http://www.w3.org/2004/02/skos/core#prefLabel>
                "Diskhaler" .

v3-EntityCode:JAR  a     owl:Class ;
        rdfs:label       "Jar" ;
        rdfs:subClassOf  v3-EntityCode:_MultiUseContainerEntityType ;
        <http://www.w3.org/2004/02/skos/core#definition>
                "A container of glass, earthenware, plastic, etc.  Top of the container has a diameter of similar size to the diameter of the container as a whole" ;
        <http://www.w3.org/2004/02/skos/core#prefLabel>
                "Jar" .

v3-EntityCode:SACH  a    owl:Class ;
        rdfs:label       "Sachet" ;
        rdfs:subClassOf  v3-EntityCode:_NonRigidContainerEntityType ;
        <http://www.w3.org/2004/02/skos/core#definition>
                "A small bag or packet containing a small portion of a substance." ;
        <http://www.w3.org/2004/02/skos/core#prefLabel>
                "Sachet" .

v3-EntityCode:HNO3  a    owl:Class ;
        rdfs:label       "Nitric Acid" ;
        rdfs:subClassOf  v3-EntityCode:_SpecimenAdditiveEntity ;
        <http://www.w3.org/2004/02/skos/core#definition>
                "6N Nitric acid used to preserve urine for heavy metal analysis." ;
        <http://www.w3.org/2004/02/skos/core#prefLabel>
                "Nitric Acid" .

v3-EntityCode:HHOLD  a   owl:Class ;
        rdfs:label       "household" ;
        rdfs:subClassOf  v3-EntityCode:_OrganizationEntityType ;
        <http://www.w3.org/2004/02/skos/core#definition>
                "The group of persons who occupy a single housing unit." ;
        <http://www.w3.org/2004/02/skos/core#prefLabel>
                "household" .

v3-EntityCode:BOTP  a    owl:Class ;
        rdfs:label       "Plastic Bottle" ;
        rdfs:subClassOf  v3-EntityCode:BOT ;
        <http://www.w3.org/2004/02/skos/core#definition>
                "A bottle made of plastic" ;
        <http://www.w3.org/2004/02/skos/core#prefLabel>
                "Plastic Bottle" .

v3-EntityCode:TOLU  a    owl:Class ;
        rdfs:label       "Toluene" ;
        rdfs:subClassOf  v3-EntityCode:_SpecimenAdditiveEntity ;
        <http://www.w3.org/2004/02/skos/core#definition>
                "Also known as Methylbenzene; Toluol; Phenylmethane. A preservative for 24 Hr Urine samples" ;
        <http://www.w3.org/2004/02/skos/core#prefLabel>
                "Toluene" .

v3-EntityCode:_MedicalDevice
        a                owl:Class ;
        rdfs:label       "MedicalDevice" ;
        rdfs:subClassOf  v3-EntityCode:_MaterialEntityClassType ;
        <http://www.w3.org/2004/02/skos/core#definition>
                "A device with direct or indirect therapeutic purpose.  Values for EntityCode when EntityClass = \"DEV\"" ;
        <http://www.w3.org/2004/02/skos/core#prefLabel>
                "MedicalDevice" .

v3-EntityCode:LINE  a    owl:Class ;
        rdfs:label       "Line" ;
        rdfs:subClassOf  v3-EntityCode:_AccessMedicalDevice ;
        <http://www.w3.org/2004/02/skos/core#definition>
                "A hollow tube used to administer a substance into a vein, artery or body cavity" ;
        <http://www.w3.org/2004/02/skos/core#prefLabel>
                "Line" .

v3-EntityCode:KARN  a    owl:Class ;
        rdfs:label       "Karnovsky's fixative" ;
        rdfs:subClassOf  v3-EntityCode:_SpecimenAdditiveEntity ;
        <http://www.w3.org/2004/02/skos/core#definition>
                "5% Glutaraldehyde, 4% Formaldehyde in 0.08M buffer. Tissue preservation" ;
        <http://www.w3.org/2004/02/skos/core#prefLabel>
                "Karnovsky's fixative" .

v3-EntityCode:PAGE  a    owl:Class ;
        rdfs:label       "Page's Saline" ;
        rdfs:subClassOf  v3-EntityCode:_SpecimenAdditiveEntity ;
        <http://www.w3.org/2004/02/skos/core#definition>
                "0.12 g NaCl, 0.004 g MgSO, 0.004 g, CaCl, 0.142 g Na2HPO4 and 0.136 g KH2PO4 per liter of distilled water. Maintain Acanthaoemba viability." ;
        <http://www.w3.org/2004/02/skos/core#prefLabel>
                "Page's Saline" .

v3-EntityCode:_PlaceEntityType
        a           owl:Class ;
        rdfs:label  "PlaceEntityType" ;
        <http://www.w3.org/2004/02/skos/core#definition>
                "Types of places for EntityClass \"PLC\"" ;
        <http://www.w3.org/2004/02/skos/core#prefLabel>
                "PlaceEntityType" .

v3-EntityCode:NDA06  a   owl:Class ;
        rdfs:label       "sulfites" ;
        rdfs:subClassOf  v3-EntityCode:_NonDrugAgentEntity ;
        <http://www.w3.org/2004/02/skos/core#definition>
                "sulfites" ;
        <http://www.w3.org/2004/02/skos/core#prefLabel>
                "sulfites" .

v3-EntityCode:EDTK15  a  owl:Class ;
        rdfs:label       "Potassium/K EDTA 15%" ;
        rdfs:subClassOf  v3-EntityCode:_SpecimenAdditiveEntity ;
        <http://www.w3.org/2004/02/skos/core#definition>
                "Potassium EDTA 15% solution in water" ;
        <http://www.w3.org/2004/02/skos/core#prefLabel>
                "Potassium/K EDTA 15%" .

v3-EntityCode:URETM  a   owl:Class ;
        rdfs:label       "Ureaplasma transport medium" ;
        rdfs:subClassOf  v3-EntityCode:_SpecimenAdditiveEntity ;
        <http://www.w3.org/2004/02/skos/core#definition>
                "A buffered salt solution with antifungal agents added for the collection and transport of Ureaplasma specimens." ;
        <http://www.w3.org/2004/02/skos/core#prefLabel>
                "Ureaplasma transport medium" .

v3-EntityCode:BOTPLY  a  owl:Class ;
        rdfs:label       "Polyethylene Bottle" ;
        rdfs:subClassOf  v3-EntityCode:BOTP ;
        <http://www.w3.org/2004/02/skos/core#definition>
                "A bottle made of polyethylene" ;
        <http://www.w3.org/2004/02/skos/core#prefLabel>
                "Polyethylene Bottle" .

v3-EntityCode:AINJ  a    owl:Class ;
        rdfs:label       "AutoInjector" ;
        rdfs:subClassOf  v3-EntityCode:_InjectionMedicalDevice ;
        <http://www.w3.org/2004/02/skos/core#definition>
                "Automatically injects medication." ;
        <http://www.w3.org/2004/02/skos/core#prefLabel>
                "AutoInjector" .

v3-EntityCode:FDP  a     owl:Class ;
        rdfs:label       "Thrombin NIH; soybean trypsin inhibitor" ;
        rdfs:subClassOf  v3-EntityCode:_SpecimenAdditiveEntity ;
        <http://www.w3.org/2004/02/skos/core#definition>
                "Thrombin plus soybean trypsin inhibitor.  For use in identifying fibrn degredation products." ;
        <http://www.w3.org/2004/02/skos/core#prefLabel>
                "Thrombin NIH; soybean trypsin inhibitor" .

v3-EntityCode:BOTD  a    owl:Class ;
        rdfs:label       "Dropper Bottle" ;
        rdfs:subClassOf  v3-EntityCode:BOT ;
        <http://www.w3.org/2004/02/skos/core#definition>
                "A bottle with a cap designed to release the contained liquid in droplets of a specific size." ;
        <http://www.w3.org/2004/02/skos/core#prefLabel>
                "Dropper Bottle" .

v3-EntityCode:HEPN  a    owl:Class ;
        rdfs:label       "Sodium/Na Heparin" ;
        rdfs:subClassOf  v3-EntityCode:_SpecimenAdditiveEntity ;
        <http://www.w3.org/2004/02/skos/core#definition>
                "Sodium heparin salt" ;
        <http://www.w3.org/2004/02/skos/core#prefLabel>
                "Sodium/Na Heparin" .

v3-EntityCode:_ClinicalDrug
        a                owl:Class ;
        rdfs:label       "ClinicalDrug" ;
        rdfs:subClassOf  v3-EntityCode:_DrugEntity ;
        <http://www.w3.org/2004/02/skos/core#definition>
                "Any substance or mixture of substances manufactured, sold or represented for use in: (a) the diagnosis, treatment, mitigation or prevention of a disease, disorder, abnormal physical state, or its symptoms, in human beings or animals; (b) restoring, correcting or modifying organic functions in human beings or animals." ;
        <http://www.w3.org/2004/02/skos/core#prefLabel>
                "ClinicalDrug" .

v3-EntityCode:_OrganizationEntityType
        a           owl:Class ;
        rdfs:label  "OrganizationEntityType" ;
        <http://www.w3.org/2004/02/skos/core#definition>
                "Further classifies entities of classCode ORG." ;
        <http://www.w3.org/2004/02/skos/core#prefLabel>
                "OrganizationEntityType" .

v3-EntityCode:NDA13  a   owl:Class ;
        rdfs:label       "shellfish" ;
        rdfs:subClassOf  v3-EntityCode:_NonDrugAgentEntity ;
        <http://www.w3.org/2004/02/skos/core#definition>
                "shellfish" ;
        <http://www.w3.org/2004/02/skos/core#prefLabel>
                "shellfish" .

v3-EntityCode:C38  a     owl:Class ;
        rdfs:label       "3.8% Citrate" ;
        rdfs:subClassOf  v3-EntityCode:_SpecimenAdditiveEntity ;
        <http://www.w3.org/2004/02/skos/core#definition>
                "A 3.8% solution of Sodium Citrate in water. Used as a blood preservative" ;
        <http://www.w3.org/2004/02/skos/core#prefLabel>
                "3.8% Citrate" .

v3-EntityCode:AMIES  a   owl:Class ;
        rdfs:label       "Amies transport medium" ;
        rdfs:subClassOf  v3-EntityCode:_SpecimenAdditiveEntity ;
        <http://www.w3.org/2004/02/skos/core#definition>
                "Sodium Chloride 3.0g, Potassium Chloride 0.2g, Calcium Chloride 0.1g, Magnesium Chloride 0.1g, Monopotassium Phosphate 0.2g, Disodium Phosphate 1.15g, Sodium Thiogly collate 1.0g, Distilled Water 1 liter" ;
        <http://www.w3.org/2004/02/skos/core#prefLabel>
                "Amies transport medium" .

v3-EntityCode:TUBE  a    owl:Class ;
        rdfs:label       "Tube" ;
        rdfs:subClassOf  v3-EntityCode:_MultiUseContainerEntityType ;
        <http://www.w3.org/2004/02/skos/core#definition>
                "A long hollow rigid or flexible cylinder.  Material is extruded by squeezing the container." ;
        <http://www.w3.org/2004/02/skos/core#prefLabel>
                "Tube" .

v3-EntityCode:_ContainerEntityType
        a                owl:Class ;
        rdfs:label       "ContainerEntityType" ;
        rdfs:subClassOf  v3-EntityCode:_MaterialEntityClassType ;
        <http://www.w3.org/2004/02/skos/core#definition>
                "Material intended to hold another material for purpose of storage or transport." ;
        <http://www.w3.org/2004/02/skos/core#prefLabel>
                "ContainerEntityType" .

v3-EntityCode:SST  a     owl:Class ;
        rdfs:label       "Serum Separator Tube" ;
        rdfs:subClassOf  v3-EntityCode:_SpecimenAdditiveEntity ;
        <http://www.w3.org/2004/02/skos/core#definition>
                "Polymer separator gel with clot activator" ;
        <http://www.w3.org/2004/02/skos/core#prefLabel>
                "Serum Separator Tube" .

v3-EntityCode:IALINE  a  owl:Class ;
        rdfs:label       "Intra-arterial Line" ;
        rdfs:subClassOf  v3-EntityCode:LINE ;
        <http://www.w3.org/2004/02/skos/core#definition>
                "A line used to administer a substance into an artery" ;
        <http://www.w3.org/2004/02/skos/core#prefLabel>
                "Intra-arterial Line" .

v3-EntityCode:PKG  a     owl:Class ;
        rdfs:label       "Package" ;
        rdfs:subClassOf  v3-EntityCode:_ContainerEntityType ;
        <http://www.w3.org/2004/02/skos/core#definition>
                "A material intended to hold other materials for purposes of storage or transportation" ;
        <http://www.w3.org/2004/02/skos/core#prefLabel>
                "Package" .

v3-EntityCode:C32  a     owl:Class ;
        rdfs:label       "3.2% Citrate" ;
        rdfs:subClassOf  v3-EntityCode:_SpecimenAdditiveEntity ;
        <http://www.w3.org/2004/02/skos/core#definition>
                "A 3.2% solution of Sodium Citrate in water.  Used as a blood preservative" ;
        <http://www.w3.org/2004/02/skos/core#prefLabel>
                "3.2% Citrate" .

v3-EntityCode:BAG  a     owl:Class ;
        rdfs:label       "Bag" ;
        rdfs:subClassOf  v3-EntityCode:_NonRigidContainerEntityType ;
        <http://www.w3.org/2004/02/skos/core#definition>
                "A pouched or pendulous container." ;
        <http://www.w3.org/2004/02/skos/core#prefLabel>
                "Bag" .

v3-EntityCode:AMP  a     owl:Class ;
        rdfs:label       "Ampule" ;
        rdfs:subClassOf  v3-EntityCode:_IndividualPackageEntityType ;
        <http://www.w3.org/2004/02/skos/core#definition>
                "A small sealed glass container that holds a measured amount of a medicinal substance." ;
        <http://www.w3.org/2004/02/skos/core#prefLabel>
                "Ampule" .

v3-EntityCode:M4RT  a    owl:Class ;
        rdfs:label       "M4-RT" ;
        rdfs:subClassOf  v3-EntityCode:_SpecimenAdditiveEntity ;
        <http://www.w3.org/2004/02/skos/core#definition>
                "Modified Hank's balanced salt solution supplemented with bovine serum albumin, gelatin, sucrose and glutamic acid. It is buffered to pH 7.3+ or - 0.2 with Hepes buffer. Phenol red is used to indicate pH. Gentamicin and amphotericin B are used to inhibit c" ;
        <http://www.w3.org/2004/02/skos/core#prefLabel>
                "M4-RT" .

v3-EntityCode:CNSTR  a   owl:Class ;
        rdfs:label       "Canister" ;
        rdfs:subClassOf  v3-EntityCode:_MultiUseContainerEntityType ;
        <http://www.w3.org/2004/02/skos/core#definition>
                "A pressurized metal container holding a substance released as a spray or aerosol." ;
        <http://www.w3.org/2004/02/skos/core#prefLabel>
                "Canister" .

v3-EntityCode:HCL6  a    owl:Class ;
        rdfs:label       "6N HCL" ;
        rdfs:subClassOf  v3-EntityCode:_SpecimenAdditiveEntity ;
        <http://www.w3.org/2004/02/skos/core#definition>
                "A solution of HCl containing 6moles of hydrogen ion/L. Used as a Urine Preservative." ;
        <http://www.w3.org/2004/02/skos/core#prefLabel>
                "6N HCL" .

v3-EntityCode:NDA05  a   owl:Class ;
        rdfs:label       "soy" ;
        rdfs:subClassOf  v3-EntityCode:_NonDrugAgentEntity ;
        <http://www.w3.org/2004/02/skos/core#definition>
                "soy" ;
        <http://www.w3.org/2004/02/skos/core#prefLabel>
                "soy" .

v3-EntityCode:_RigidContainerEntityType
        a                owl:Class ;
        rdfs:label       "RigidContainerEntityType" ;
        rdfs:subClassOf  v3-EntityCode:PKG ;
        <http://www.w3.org/2004/02/skos/core#definition>
                "A container having a fixed and inflexible dimensions and volume" ;
        <http://www.w3.org/2004/02/skos/core#prefLabel>
                "RigidContainerEntityType" .

v3-EntityCode:  a        owl:Ontology ;
        rdfs:comment     "  OpenIssue:\r\nMissing description." ;
        rdfs:label       "v3 Code System EntityCode" ;
        owl:versionIRI   "http://hl7.org/fhir/v3/EntityCode/2016-11-11" ;
        owl:versionInfo  "v3 Code System EntityCode(2016-11-11)" .

v3-EntityCode:PVA  a     owl:Class ;
        rdfs:label       "Polyvinylalcohol" ;
        rdfs:subClassOf  v3-EntityCode:_SpecimenAdditiveEntity ;
        <http://www.w3.org/2004/02/skos/core#definition>
                "Polyvinyl alcohol" ;
        <http://www.w3.org/2004/02/skos/core#prefLabel>
                "Polyvinylalcohol" .

v3-EntityCode:ACDB  a    owl:Class ;
        rdfs:label       "ACD Solution B" ;
        rdfs:subClassOf  v3-EntityCode:_SpecimenAdditiveEntity ;
        <http://www.w3.org/2004/02/skos/core#definition>
                "ACD Solution B of trisodium citrate, 13.2g/L; citric acid, 4.8 g/L; and dextrose 14.7 g/L. Used in Blood banking and histocompatibilty testing." ;
        <http://www.w3.org/2004/02/skos/core#prefLabel>
                "ACD Solution B" .

v3-EntityCode:LIA  a     owl:Class ;
        rdfs:label       "Lithium iodoacetate" ;
        rdfs:subClassOf  v3-EntityCode:_SpecimenAdditiveEntity ;
        <http://www.w3.org/2004/02/skos/core#definition>
                "Iodoacetate lithium salt" ;
        <http://www.w3.org/2004/02/skos/core#prefLabel>
                "Lithium iodoacetate" .

v3-EntityCode:MICHTM  a  owl:Class ;
        rdfs:label       "Michel's transport medium" ;
        rdfs:subClassOf  v3-EntityCode:_SpecimenAdditiveEntity ;
        <http://www.w3.org/2004/02/skos/core#definition>
                "1M potassium citrate, pH 7.0 2.5 ml, 0.1M magnesium sulfate 5.0 ml, 0.1M N-ethyl malemide  5.0 ml, dH2O 87.5 ml, ammonium sulfate 55gm. Preserve antigens for Immunofluorescence procedures" ;
        <http://www.w3.org/2004/02/skos/core#prefLabel>
                "Michel's transport medium" .

v3-EntityCode:ROOM  a    owl:Class ;
        rdfs:label       "Room Location" ;
        rdfs:subClassOf  v3-EntityCode:_PlaceEntityType ;
        <http://www.w3.org/2004/02/skos/core#definition>
                "The location of a room" ;
        <http://www.w3.org/2004/02/skos/core#prefLabel>
                "Room Location" .

v3-EntityCode:_ResourceGroupEntityType
        a           owl:Class ;
        rdfs:label  "ResourceGroupEntityType" ;
        <http://www.w3.org/2004/02/skos/core#definition>
                "Codes to characterize a Resource Group using categories that typify its membership and/or function\r\n\n                        .\r\n\n                        \n                           Example: PractitionerGroup" ;
        <http://www.w3.org/2004/02/skos/core#prefLabel>
                "ResourceGroupEntityType" .

v3-EntityCode:_MultiUseContainerEntityType
        a                owl:Class ;
        rdfs:label       "MultiUseContainerEntityType" ;
        rdfs:subClassOf  v3-EntityCode:_RigidContainerEntityType ;
        <http://www.w3.org/2004/02/skos/core#definition>
                "A container intended to contain sufficient material for more than one use.  (I.e. Material is intended to be removed from the container at more than one discrete time period.)" ;
        <http://www.w3.org/2004/02/skos/core#prefLabel>
                "MultiUseContainerEntityType" .

v3-EntityCode:WEST  a    owl:Class ;
        rdfs:label       "Buffered Citrate" ;
        rdfs:subClassOf  v3-EntityCode:_SpecimenAdditiveEntity ;
        <http://www.w3.org/2004/02/skos/core#definition>
                "3.8% Citrate buffered to a pH of 5.5 for Westergren Sedimentation Rate" ;
        <http://www.w3.org/2004/02/skos/core#prefLabel>
                "Buffered Citrate" .

v3-EntityCode:NDA12  a   owl:Class ;
        rdfs:label       "latex" ;
        rdfs:subClassOf  v3-EntityCode:_NonDrugAgentEntity ;
        <http://www.w3.org/2004/02/skos/core#definition>
                "latex" ;
        <http://www.w3.org/2004/02/skos/core#prefLabel>
                "latex" .

v3-EntityCode:RELIG  a   owl:Class ;
        rdfs:label       "religious institution" ;
        rdfs:subClassOf  v3-EntityCode:_OrganizationEntityType ;
        <http://www.w3.org/2004/02/skos/core#definition>
                "An organization that provides religious rites of worship." ;
        <http://www.w3.org/2004/02/skos/core#prefLabel>
                "religious institution" .

v3-EntityCode:JKM  a     owl:Class ;
        rdfs:label       "Jones Kendrick Medium" ;
        rdfs:subClassOf  v3-EntityCode:_SpecimenAdditiveEntity ;
        <http://www.w3.org/2004/02/skos/core#definition>
                "A transport medium formulated to maintain Bordetella pertussis viability." ;
        <http://www.w3.org/2004/02/skos/core#prefLabel>
                "Jones Kendrick Medium" .

v3-EntityCode:_InjectionMedicalDevice
        a                owl:Class ;
        rdfs:label       "InjectionMedicalDevice" ;
        rdfs:subClassOf  v3-EntityCode:_AdministrationMedicalDevice ;
        <http://www.w3.org/2004/02/skos/core#definition>
                "A device intended to administer liquid into a subject via a" ;
        <http://www.w3.org/2004/02/skos/core#prefLabel>
                "InjectionMedicalDevice" .

v3-EntityCode:IVLINE  a  owl:Class ;
        rdfs:label       "Intraveneous Line" ;
        rdfs:subClassOf  v3-EntityCode:LINE ;
        <http://www.w3.org/2004/02/skos/core#definition>
                "A line used to administer a substance into a vein" ;
        <http://www.w3.org/2004/02/skos/core#prefLabel>
                "Intraveneous Line" .

v3-EntityCode:F10  a     owl:Class ;
        rdfs:label       "10% Formalin" ;
        rdfs:subClassOf  v3-EntityCode:_SpecimenAdditiveEntity ;
        <http://www.w3.org/2004/02/skos/core#definition>
                "A 10% v/v solution in water of formalin( a 37% solution of formaldehyde and water).  Used for tissue preservation." ;
        <http://www.w3.org/2004/02/skos/core#prefLabel>
                "10% Formalin" .

v3-EntityCode:EDTK75  a  owl:Class ;
        rdfs:label       "Potassium/K EDTA 7.5%" ;
        rdfs:subClassOf  v3-EntityCode:_SpecimenAdditiveEntity ;
        <http://www.w3.org/2004/02/skos/core#definition>
                "Potassium EDTA 7.5% solution in water" ;
        <http://www.w3.org/2004/02/skos/core#prefLabel>
                "Potassium/K EDTA 7.5%" .

v3-EntityCode:DOSET  a   owl:Class ;
        rdfs:label       "Dosette" ;
        rdfs:subClassOf  v3-EntityCode:COMPPKG ;
        <http://www.w3.org/2004/02/skos/core#definition>
                "Special packaging that will help patients take their medications on a regular basis." ;
        <http://www.w3.org/2004/02/skos/core#prefLabel>
                "Dosette" .

v3-EntityCode:TUB  a     owl:Class ;
        rdfs:label       "Tub" ;
        rdfs:subClassOf  v3-EntityCode:_MultiUseContainerEntityType ;
        <http://www.w3.org/2004/02/skos/core#definition>
                "An open flat bottomed round container." ;
        <http://www.w3.org/2004/02/skos/core#prefLabel>
                "Tub" .

v3-EntityCode:STUTM  a   owl:Class ;
        rdfs:label       "Stuart transport medium" ;
        rdfs:subClassOf  v3-EntityCode:_SpecimenAdditiveEntity ;
        <http://www.w3.org/2004/02/skos/core#definition>
                "Sodium Glycerophosphate 10.0g, Calcium Chloride 0.1g, Mercaptoacetic Acid 1.0ml, Distilled Water 1 liter" ;
        <http://www.w3.org/2004/02/skos/core#prefLabel>
                "Stuart transport medium" .

v3-EntityCode:_NonRigidContainerEntityType
        a                owl:Class ;
        rdfs:label       "NonRigidContainerEntityType" ;
        rdfs:subClassOf  v3-EntityCode:PKG ;
        <http://www.w3.org/2004/02/skos/core#definition>
                "A container having dimensions that adjust somewhat based on the amount and shape of the material placed within it." ;
        <http://www.w3.org/2004/02/skos/core#prefLabel>
                "NonRigidContainerEntityType" .

v3-EntityCode:_AdministrationMedicalDevice
        a                owl:Class ;
        rdfs:label       "AdministrationMedicalDevice" ;
        rdfs:subClassOf  v3-EntityCode:_MedicalDevice ;
        <http://www.w3.org/2004/02/skos/core#definition>
                "A device intended to administer a substance to a subject" ;
        <http://www.w3.org/2004/02/skos/core#prefLabel>
                "AdministrationMedicalDevice" .

v3-EntityCode:NDA04  a   owl:Class ;
        rdfs:label       "peanut" ;
        rdfs:subClassOf  v3-EntityCode:_NonDrugAgentEntity ;
        <http://www.w3.org/2004/02/skos/core#definition>
                "peanut" ;
        <http://www.w3.org/2004/02/skos/core#prefLabel>
                "peanut" .

v3-EntityCode:FL10  a    owl:Class ;
        rdfs:label       "Sodium Fluoride, 10mg" ;
        rdfs:subClassOf  v3-EntityCode:_SpecimenAdditiveEntity ;
        <http://www.w3.org/2004/02/skos/core#definition>
                "Sodium fluoride, 10mg added as a urine preservative." ;
        <http://www.w3.org/2004/02/skos/core#prefLabel>
                "Sodium Fluoride, 10mg" .

v3-EntityCode:HEPA  a    owl:Class ;
        rdfs:label       "Ammonium heparin" ;
        rdfs:subClassOf  v3-EntityCode:_SpecimenAdditiveEntity ;
        <http://www.w3.org/2004/02/skos/core#definition>
                "Ammonium heparin" ;
        <http://www.w3.org/2004/02/skos/core#prefLabel>
                "Ammonium heparin" .

v3-EntityCode:CARD  a    owl:Class ;
        rdfs:label       "Card" ;
        rdfs:subClassOf  v3-EntityCode:BLSTRPK ;
        <http://www.w3.org/2004/02/skos/core#definition>
                "A bubble pack card.  Multiple individual/separated doses." ;
        <http://www.w3.org/2004/02/skos/core#prefLabel>
                "Card" .

v3-EntityCode:NEBAMP  a  owl:Class ;
        rdfs:label       "Nebuamp" ;
        rdfs:subClassOf  v3-EntityCode:_IndividualPackageEntityType ;
        <http://www.w3.org/2004/02/skos/core#definition>
                "Individually dosed inhalation solution." ;
        <http://www.w3.org/2004/02/skos/core#prefLabel>
                "Nebuamp" .

v3-EntityCode:NDA17  a   owl:Class ;
        rdfs:label       "dust mites" ;
        rdfs:subClassOf  v3-EntityCode:_NonDrugAgentEntity ;
        <http://www.w3.org/2004/02/skos/core#definition>
                "dust mites" ;
        <http://www.w3.org/2004/02/skos/core#prefLabel>
                "dust mites" .

v3-EntityCode:CTAD  a    owl:Class ;
        rdfs:label       "CTAD" ;
        rdfs:subClassOf  v3-EntityCode:_SpecimenAdditiveEntity ;
        <http://www.w3.org/2004/02/skos/core#definition>
                "Buffered tri-sodium citrate solution with theophylline, adenosine and dipyridamole" ;
        <http://www.w3.org/2004/02/skos/core#prefLabel>
                "CTAD" .

v3-EntityCode:ACDA  a    owl:Class ;
        rdfs:label       "ACD Solution A" ;
        rdfs:subClassOf  v3-EntityCode:_SpecimenAdditiveEntity ;
        <http://www.w3.org/2004/02/skos/core#definition>
                "ACD Solution A of trisodium citrate, 22.0g/L; citric acid, 8.0 g/L; and dextrose 24.5 g/L. Used in Blood banking and histocompatibilty testing" ;
        <http://www.w3.org/2004/02/skos/core#prefLabel>
                "ACD Solution A" .

v3-EntityCode:THYO  a    owl:Class ;
        rdfs:label       "Thyoglycolate broth" ;
        rdfs:subClassOf  v3-EntityCode:_SpecimenAdditiveEntity ;
        <http://www.w3.org/2004/02/skos/core#definition>
                "A nutritive medium with a reducing agent  (sodium thioglycolate) which, due to a chemical reaction, removes oxygen from the broth." ;
        <http://www.w3.org/2004/02/skos/core#prefLabel>
                "Thyoglycolate broth" .

v3-EntityCode:_DrugEntity
        a                owl:Class ;
        rdfs:label       "DrugEntity" ;
        rdfs:subClassOf  v3-EntityCode:_MaterialEntityClassType ;
        <http://www.w3.org/2004/02/skos/core#definition>
                "A substance whose therapeutic effect is produced by chemical action within the body." ;
        <http://www.w3.org/2004/02/skos/core#prefLabel>
                "DrugEntity" .

v3-EntityCode:DSKS  a    owl:Class ;
        rdfs:label       "Diskus" ;
        rdfs:subClassOf  v3-EntityCode:INH ;
        <http://www.w3.org/2004/02/skos/core#definition>
                "The device used to inhale the doses of medication contained in the disk form." ;
        <http://www.w3.org/2004/02/skos/core#prefLabel>
                "Diskus" .

v3-EntityCode:BSKM  a    owl:Class ;
        rdfs:label       "Buffered skim milk" ;
        rdfs:subClassOf  v3-EntityCode:_SpecimenAdditiveEntity ;
        <http://www.w3.org/2004/02/skos/core#definition>
                "50% skim milk in 0.01 M phosphate-buffered saline.  Maintain virus viability" ;
        <http://www.w3.org/2004/02/skos/core#prefLabel>
                "Buffered skim milk" .

v3-EntityCode:HEPL  a    owl:Class ;
        rdfs:label       "Lithium/Li Heparin" ;
        rdfs:subClassOf  v3-EntityCode:_SpecimenAdditiveEntity ;
        <http://www.w3.org/2004/02/skos/core#definition>
                "Lithium heparin salt" ;
        <http://www.w3.org/2004/02/skos/core#prefLabel>
                "Lithium/Li Heparin" .

v3-EntityCode:NAT  a     owl:Class ;
        rdfs:label       "NationEntityType" ;
        rdfs:subClassOf  v3-EntityCode:_OrganizationEntityType ;
        <http://www.w3.org/2004/02/skos/core#definition>
                "Codes identifying nation states.  Allows for finer grained specification of Entity with classcode <= NAT\r\n\n                        \n                           Example:ISO3166 country codes." ;
        <http://www.w3.org/2004/02/skos/core#prefLabel>
                "NationEntityType" .

v3-EntityCode:NDA11  a   owl:Class ;
        rdfs:label       "venoms" ;
        rdfs:subClassOf  v3-EntityCode:_NonDrugAgentEntity ;
        <http://www.w3.org/2004/02/skos/core#definition>
                "venoms" ;
        <http://www.w3.org/2004/02/skos/core#prefLabel>
                "venoms" .

v3-EntityCode:PRAC  a    owl:Class ;
        rdfs:label       "PractitionerGroup" ;
        rdfs:subClassOf  v3-EntityCode:_ResourceGroupEntityType ;
        <http://www.w3.org/2004/02/skos/core#definition>
                "PractitionerGroup" ;
        <http://www.w3.org/2004/02/skos/core#prefLabel>
                "PractitionerGroup" .

v3-EntityCode:_AccessMedicalDevice
        a                owl:Class ;
        rdfs:label       "AccessMedicalDevice" ;
        rdfs:subClassOf  v3-EntityCode:_MedicalDevice ;
        <http://www.w3.org/2004/02/skos/core#definition>
                "A device used to allow access to a part of a body" ;
        <http://www.w3.org/2004/02/skos/core#prefLabel>
                "AccessMedicalDevice" .

v3-EntityCode:_SpecimenAdditiveEntity
        a                owl:Class ;
        rdfs:label       "SpecimenAdditiveEntity" ;
        rdfs:subClassOf  v3-EntityCode:_MaterialEntityClassType ;
        <http://www.w3.org/2004/02/skos/core#definition>
                "Set of codes related to specimen additives" ;
        <http://www.w3.org/2004/02/skos/core#prefLabel>
                "SpecimenAdditiveEntity" .

v3-EntityCode:NDA09  a   owl:Class ;
        rdfs:label       "solvents" ;
        rdfs:subClassOf  v3-EntityCode:_NonDrugAgentEntity ;
        <http://www.w3.org/2004/02/skos/core#definition>
                "solvents" ;
        <http://www.w3.org/2004/02/skos/core#prefLabel>
                "solvents" .

v3-EntityCode:KOX  a     owl:Class ;
        rdfs:label       "Potassium Oxalate" ;
        rdfs:subClassOf  v3-EntityCode:_SpecimenAdditiveEntity ;
        <http://www.w3.org/2004/02/skos/core#definition>
                "Potassium oxalate and sodium fluoride in a 1.25:1 ratio" ;
        <http://www.w3.org/2004/02/skos/core#prefLabel>
                "Potassium Oxalate" .

v3-EntityCode:PHENOL  a  owl:Class ;
        rdfs:label       "Phenol" ;
        rdfs:subClassOf  v3-EntityCode:_SpecimenAdditiveEntity ;
        <http://www.w3.org/2004/02/skos/core#definition>
                "Phenol. Urine preservative" ;
        <http://www.w3.org/2004/02/skos/core#prefLabel>
                "Phenol" .

v3-EntityCode:BOT  a     owl:Class ;
        rdfs:label       "Bottle" ;
        rdfs:subClassOf  v3-EntityCode:_MultiUseContainerEntityType ;
        <http://www.w3.org/2004/02/skos/core#definition>
                "A container, typically rounded, either glass or plastic with a narrow neck and capable of storing liquid." ;
        <http://www.w3.org/2004/02/skos/core#prefLabel>
                "Bottle" .

v3-EntityCode:NDA03  a   owl:Class ;
        rdfs:label       "lactose" ;
        rdfs:subClassOf  v3-EntityCode:_NonDrugAgentEntity ;
        <http://www.w3.org/2004/02/skos/core#definition>
                "lactose" ;
        <http://www.w3.org/2004/02/skos/core#prefLabel>
                "lactose" .

v3-EntityCode:_NonDrugAgentEntity
        a           owl:Class ;
        rdfs:label  "NonDrugAgentEntity" ;
        <http://www.w3.org/2004/02/skos/core#definition>
                "Indicates types of allergy and intolerance agents which are non-drugs.  (E.g. foods, latex, etc.)" ;
        <http://www.w3.org/2004/02/skos/core#prefLabel>
                "NonDrugAgentEntity" .

v3-EntityCode:RLM  a     owl:Class ;
        rdfs:label       "Reagan Lowe Medium" ;
        rdfs:subClassOf  v3-EntityCode:_SpecimenAdditiveEntity ;
        <http://www.w3.org/2004/02/skos/core#definition>
                "A transport medium formulated to maintain Bordetella pertussis viability." ;
        <http://www.w3.org/2004/02/skos/core#prefLabel>
                "Reagan Lowe Medium" .

v3-EntityCode:NONE  a    owl:Class ;
        rdfs:label       "None" ;
        rdfs:subClassOf  v3-EntityCode:_SpecimenAdditiveEntity ;
        <http://www.w3.org/2004/02/skos/core#definition>
                "No additive. Specifically identifes the specimen as having no additives." ;
        <http://www.w3.org/2004/02/skos/core#prefLabel>
                "None" .

v3-EntityCode:TRBINH  a  owl:Class ;
        rdfs:label       "Turbuhaler" ;
        rdfs:subClassOf  v3-EntityCode:INH ;
        <http://www.w3.org/2004/02/skos/core#definition>
                "Asthma medication delivery device." ;
        <http://www.w3.org/2004/02/skos/core#prefLabel>
                "Turbuhaler" .

v3-EntityCode:DISK  a    owl:Class ;
        rdfs:label       "Disk" ;
        rdfs:subClassOf  v3-EntityCode:COMPPKG ;
        <http://www.w3.org/2004/02/skos/core#definition>
                "Object that is thin, flat, and circular.  Doses of medication often contained in bubbles on the disk." ;
        <http://www.w3.org/2004/02/skos/core#prefLabel>
                "Disk" .

v3-EntityCode:BOTG  a    owl:Class ;
        rdfs:label       "Glass Bottle" ;
        rdfs:subClassOf  v3-EntityCode:BOT ;
        <http://www.w3.org/2004/02/skos/core#definition>
                "A bottle made of glass" ;
        <http://www.w3.org/2004/02/skos/core#prefLabel>
                "Glass Bottle" .

v3-EntityCode:BLDPRD  a  owl:Class ;
        rdfs:label       "Blood Product" ;
        rdfs:subClassOf  v3-EntityCode:_MaterialEntityClassType ;
        <http://www.w3.org/2004/02/skos/core#definition>
                "A manufactured product that is produced from the raw blood oi a donor with the intention of using it in a recipient transfusion." ;
        <http://www.w3.org/2004/02/skos/core#prefLabel>
                "Blood Product" .

v3-EntityCode:MINIM  a   owl:Class ;
        rdfs:label       "Minim" ;
        rdfs:subClassOf  v3-EntityCode:_IndividualPackageEntityType ;
        <http://www.w3.org/2004/02/skos/core#definition>
                "Individually dosed ophthalmic solution.  One time eye dropper dispenser." ;
        <http://www.w3.org/2004/02/skos/core#prefLabel>
                "Minim" .

v3-EntityCode:CART  a    owl:Class ;
        rdfs:label       "Cartridge" ;
        rdfs:subClassOf  v3-EntityCode:_MultiUseContainerEntityType ;
        <http://www.w3.org/2004/02/skos/core#definition>
                "A sealed container of liquid or powder intended to be loaded into a device." ;
        <http://www.w3.org/2004/02/skos/core#prefLabel>
                "Cartridge" .

v3-EntityCode:NDA16  a   owl:Class ;
        rdfs:label       "dust" ;
        rdfs:subClassOf  v3-EntityCode:_NonDrugAgentEntity ;
        <http://www.w3.org/2004/02/skos/core#definition>
                "dust" ;
        <http://www.w3.org/2004/02/skos/core#prefLabel>
                "dust" .

v3-EntityCode:PCH  a     owl:Class ;
        rdfs:label       "Pouch" ;
        rdfs:subClassOf  v3-EntityCode:_NonRigidContainerEntityType ;
        <http://www.w3.org/2004/02/skos/core#definition>
                "A small bag or container made of a soft material." ;
        <http://www.w3.org/2004/02/skos/core#prefLabel>
                "Pouch" .

v3-EntityCode:M5  a      owl:Class ;
        rdfs:label       "M5" ;
        rdfs:subClassOf  v3-EntityCode:_SpecimenAdditiveEntity ;
        <http://www.w3.org/2004/02/skos/core#definition>
                "Modified Hank's balanced salt solution supplemented with protein stabilizers, sucrose and glutamic acid. It is buffered to pH 7.3+ or - 0.2 with Hepes buffer. Phenol red is used to indicate pH. Vancomycin, Amphotericin B and Colistin are used to inhibit c" ;
        <http://www.w3.org/2004/02/skos/core#prefLabel>
                "M5" .

v3-EntityCode:COMPPKG
        a                owl:Class ;
        rdfs:label       "Compliance Package" ;
        rdfs:subClassOf  v3-EntityCode:PKG ;
        <http://www.w3.org/2004/02/skos/core#definition>
                "A container intended to contain sufficient material for more than one use, but grouped or organized to provide individual access to sufficient material for a single use.  Often used to ensure that the proper type and amount of material is consumed/expended for each use." ;
        <http://www.w3.org/2004/02/skos/core#prefLabel>
                "Compliance Package" .

v3-EntityCode:ACET  a    owl:Class ;
        rdfs:label       "Acetic Acid" ;
        rdfs:subClassOf  v3-EntityCode:_SpecimenAdditiveEntity ;
        <http://www.w3.org/2004/02/skos/core#definition>
                "50% V/V acetic acid in water.  Used as  a urine preservative" ;
        <http://www.w3.org/2004/02/skos/core#prefLabel>
                "Acetic Acid" .

v3-EntityCode:BOUIN  a   owl:Class ;
        rdfs:label       "Bouin's solution" ;
        rdfs:subClassOf  v3-EntityCode:_SpecimenAdditiveEntity ;
        <http://www.w3.org/2004/02/skos/core#definition>
                "Picric acid, saturated aqueous solution (750.0 ml), 37-40% formalin (250.0 ml), glacial acetic acid (50.0 ml). Tissue preservative." ;
        <http://www.w3.org/2004/02/skos/core#prefLabel>
                "Bouin's solution" .

v3-EntityCode:BOTA  a    owl:Class ;
        rdfs:label       "Amber Bottle" ;
        rdfs:subClassOf  v3-EntityCode:BOT ;
        <http://www.w3.org/2004/02/skos/core#definition>
                "A bottle of yellow to brown color.  Used to store light-sensitive materials" ;
        <http://www.w3.org/2004/02/skos/core#prefLabel>
                "Amber Bottle" .

v3-EntityCode:PEN  a     owl:Class ;
        rdfs:label       "Pen" ;
        rdfs:subClassOf  v3-EntityCode:_InjectionMedicalDevice ;
        <http://www.w3.org/2004/02/skos/core#definition>
                "A device which can contain a cartridge for injection purposes.  Eg. Insulin pen." ;
        <http://www.w3.org/2004/02/skos/core#prefLabel>
                "Pen" .

v3-EntityCode:NDA10  a   owl:Class ;
        rdfs:label       "oils" ;
        rdfs:subClassOf  v3-EntityCode:_NonDrugAgentEntity ;
        <http://www.w3.org/2004/02/skos/core#definition>
                "oils" ;
        <http://www.w3.org/2004/02/skos/core#prefLabel>
                "oils" .

v3-EntityCode:BLSTRPK
        a                owl:Class ;
        rdfs:label       "Blister Pack" ;
        rdfs:subClassOf  v3-EntityCode:_RigidContainerEntityType ;
        <http://www.w3.org/2004/02/skos/core#definition>
                "A bubblepack.  Medications sealed individually, separated into doses." ;
        <http://www.w3.org/2004/02/skos/core#prefLabel>
                "Blister Pack" .

v3-EntityCode:_MaterialEntityClassType
        a           owl:Class ;
        rdfs:label  "MaterialEntityClassType" ;
        <http://www.w3.org/2004/02/skos/core#definition>
                "Types of Material for EntityClass \"MAT\"" ;
        <http://www.w3.org/2004/02/skos/core#prefLabel>
                "MaterialEntityClassType" .

v3-EntityCode:PMP  a     owl:Class ;
        rdfs:label       "Pump" ;
        rdfs:subClassOf  v3-EntityCode:_AdministrationMedicalDevice ;
        <http://www.w3.org/2004/02/skos/core#definition>
                "A device that is used to raise, compress, or transfer liquids or gases and is operated by a piston or similar mechanism." ;
        <http://www.w3.org/2004/02/skos/core#prefLabel>
                "Pump" .

v3-EntityCode:EDTN  a    owl:Class ;
        rdfs:label       "Sodium/Na EDTA" ;
        rdfs:subClassOf  v3-EntityCode:_SpecimenAdditiveEntity ;
        <http://www.w3.org/2004/02/skos/core#definition>
                "Sodium fluoride and Disodium EDTA" ;
        <http://www.w3.org/2004/02/skos/core#prefLabel>
                "Sodium/Na EDTA" .

v3-EntityCode:SPS  a     owl:Class ;
        rdfs:label       "Sodium polyanethol sulfonate 0.35% in 0.85% sodium chloride" ;
        rdfs:subClassOf  v3-EntityCode:_SpecimenAdditiveEntity ;
        <http://www.w3.org/2004/02/skos/core#definition>
                "Sodium polyanethol sulfonate in saline. Anticomplementary and antiphagocytic properties. Used in blood culture collection." ;
        <http://www.w3.org/2004/02/skos/core#prefLabel>
                "Sodium polyanethol sulfonate 0.35% in 0.85% sodium chloride" .

v3-EntityCode:VIRTM  a   owl:Class ;
        rdfs:label       "Viral Transport medium" ;
        rdfs:subClassOf  v3-EntityCode:_SpecimenAdditiveEntity ;
        <http://www.w3.org/2004/02/skos/core#definition>
                "Sucrose 74.6g, Potassium hydrogenphosphate 0.52g, L-glutamic acid 0.72g, Bovine serum albumin 5.0g, Gentamicin 50mg, Potassium dihydrogenphosphate 1.25g, L-15 medium 9.9L, Water to 10L. Maintain Virus viability." ;
        <http://www.w3.org/2004/02/skos/core#prefLabel>
                "Viral Transport medium" .

v3-EntityCode:TIN  a     owl:Class ;
        rdfs:label       "Tin" ;
        rdfs:subClassOf  v3-EntityCode:_MultiUseContainerEntityType ;
        <http://www.w3.org/2004/02/skos/core#definition>
                "A lidded container made of thin sheet metal." ;
        <http://www.w3.org/2004/02/skos/core#prefLabel>
                "Tin" .

v3-EntityCode:WING  a    owl:Class ;
        rdfs:label       "Wing Location" ;
        rdfs:subClassOf  v3-EntityCode:_PlaceEntityType ;
        <http://www.w3.org/2004/02/skos/core#definition>
                "The location of a wing of a building (e.g. East Wing).  The same room number for the same floor number can be distinguished by wing number in some situations" ;
        <http://www.w3.org/2004/02/skos/core#prefLabel>
                "Wing Location" .

v3-EntityCode:NDA08  a   owl:Class ;
        rdfs:label       "isocyanates" ;
        rdfs:subClassOf  v3-EntityCode:_NonDrugAgentEntity ;
        <http://www.w3.org/2004/02/skos/core#definition>
                "isocyanates" ;
        <http://www.w3.org/2004/02/skos/core#prefLabel>
                "isocyanates" .

v3-EntityCode:CARY  a    owl:Class ;
        rdfs:label       "Cary Blair Medium" ;
        rdfs:subClassOf  v3-EntityCode:_SpecimenAdditiveEntity ;
        <http://www.w3.org/2004/02/skos/core#definition>
                "Sodium Thioglycollate 1.5 g, Disodium Hydrogen Phosphate 1.1 g, Sodium Chloride 5.0 g, Calcium Chloride 0.09 g, Agar 5.0 g, per Liter of Water" ;
        <http://www.w3.org/2004/02/skos/core#prefLabel>
                "Cary Blair Medium" .

v3-EntityCode:PACKT  a   owl:Class ;
        rdfs:label       "Packet" ;
        rdfs:subClassOf  v3-EntityCode:_NonRigidContainerEntityType ;
        <http://www.w3.org/2004/02/skos/core#definition>
                "A paper" ;
        <http://www.w3.org/2004/02/skos/core#prefLabel>
                "Packet" .
